Update ETCS_HOL.thy
Exponentiation

ETCS_HOL.thy
@@ -3491,7 +3491,7 @@ proof -
 qed
 
 lemma zero_betaN_type: 
-  shows "(zero \<circ>\<^sub>c \<beta>\<^bsub>\<nat>\<^sub>c\<^esub>): \<nat>\<^sub>c \<rightarrow> \<nat>\<^sub>c"
+  shows "(zero \<circ>\<^sub>c \<beta>\<^bsub>X\<^esub>): X \<rightarrow> \<nat>\<^sub>c"
   using comp_type terminal_func_type zero_type by blast
 
 lemma add_apply1:
@@ -3872,7 +3872,10 @@ lemma add_respects_succ2:
   shows "m +\<^sub>\<nat> (successor  \<circ>\<^sub>c n)  =  (successor\<circ>\<^sub>c m) +\<^sub>\<nat> n"
   using add_def add_uncurried_commutes_succ assms(1) assms(2) by presburger
 
-
+lemma succ_n_type: 
+  assumes "n \<in>\<^sub>c \<nat>\<^sub>c"
+  shows "successor \<circ>\<^sub>c n \<in>\<^sub>c \<nat>\<^sub>c"
+  using assms comp_type successor_type by blast
 
 lemma add_respects_succ3: 
   assumes "m \<in>\<^sub>c \<nat>\<^sub>c" "n \<in>\<^sub>c \<nat>\<^sub>c" 
@@ -4843,7 +4846,10 @@ proof -
     by (simp add: ab_type cfunc_prod_type multAddId_c_type) 
   have multAddIdABC_type: "(mult_uncurried \<circ>\<^sub>c (add_uncurried \<times>\<^sub>f id\<^sub>c \<nat>\<^sub>c)) \<circ>\<^sub>c \<langle>\<langle>a,b\<rangle>,c\<rangle> : one \<rightarrow>\<nat>\<^sub>c"
     using ABC_type fact1 by auto
-
+  have addP0_type: "add_uncurried \<circ>\<^sub>c left_cart_proj (\<nat>\<^sub>c\<times>\<^sub>c \<nat>\<^sub>c) (\<nat>\<^sub>c\<^bsup>(\<nat>\<^sub>c\<times>\<^sub>c\<nat>\<^sub>c)\<^esup>) : (\<nat>\<^sub>c\<times>\<^sub>c \<nat>\<^sub>c) \<times>\<^sub>c (\<nat>\<^sub>c\<^bsup>(\<nat>\<^sub>c\<times>\<^sub>c\<nat>\<^sub>c)\<^esup>) \<rightarrow> \<nat>\<^sub>c"
+    using add_uncurried_type comp_type left_cart_proj_type by blast
+  have evalu_type: "(eval_func \<nat>\<^sub>c (\<nat>\<^sub>c\<times>\<^sub>c \<nat>\<^sub>c)) :  (\<nat>\<^sub>c\<times>\<^sub>c \<nat>\<^sub>c)\<times>\<^sub>c(\<nat>\<^sub>c\<^bsup>(\<nat>\<^sub>c\<times>\<^sub>c\<nat>\<^sub>c)\<^esup>)\<rightarrow>\<nat>\<^sub>c"
+    using eval_func_type by auto
 
 
  (*Top of page 16*)
@@ -4905,6 +4911,22 @@ proof -
  (right_cart_proj (\<nat>\<^sub>c\<times>\<^sub>c \<nat>\<^sub>c) \<nat>\<^sub>c)\<rangle>, mult_uncurried \<circ>\<^sub>c \<langle>(right_cart_proj \<nat>\<^sub>c \<nat>\<^sub>c)\<circ>\<^sub>c
 (left_cart_proj (\<nat>\<^sub>c\<times>\<^sub>c \<nat>\<^sub>c) \<nat>\<^sub>c),(right_cart_proj (\<nat>\<^sub>c\<times>\<^sub>c \<nat>\<^sub>c) \<nat>\<^sub>c)\<rangle>\<rangle>)\<^sup>\<sharp> : \<nat>\<^sub>c \<rightarrow> \<nat>\<^sub>c \<^bsup>(\<nat>\<^sub>c\<times>\<^sub>c \<nat>\<^sub>c)\<^esup> "
      using long_type transpose_func_def by blast
+
+   have long_sharp_c_type: "(add_uncurried \<circ>\<^sub>c\<langle>mult_uncurried \<circ>\<^sub>c \<langle>(left_cart_proj \<nat>\<^sub>c \<nat>\<^sub>c) \<circ>\<^sub>c (left_cart_proj (\<nat>\<^sub>c\<times>\<^sub>c \<nat>\<^sub>c) \<nat>\<^sub>c), 
+ (right_cart_proj (\<nat>\<^sub>c\<times>\<^sub>c \<nat>\<^sub>c) \<nat>\<^sub>c)\<rangle>, mult_uncurried \<circ>\<^sub>c \<langle>(right_cart_proj \<nat>\<^sub>c \<nat>\<^sub>c)\<circ>\<^sub>c
+(left_cart_proj (\<nat>\<^sub>c\<times>\<^sub>c \<nat>\<^sub>c) \<nat>\<^sub>c),(right_cart_proj (\<nat>\<^sub>c\<times>\<^sub>c \<nat>\<^sub>c) \<nat>\<^sub>c)\<rangle>\<rangle>)\<^sup>\<sharp> \<circ>\<^sub>c c : one \<rightarrow>\<nat>\<^sub>c \<^bsup>(\<nat>\<^sub>c\<times>\<^sub>c \<nat>\<^sub>c)\<^esup> "
+     using assms(3) comp_type long_sharp_type by blast
+
+   have very_long_type: "
+ \<langle>
+\<langle>a,b\<rangle>,
+(add_uncurried \<circ>\<^sub>c\<langle>mult_uncurried \<circ>\<^sub>c \<langle>(left_cart_proj \<nat>\<^sub>c \<nat>\<^sub>c) \<circ>\<^sub>c (left_cart_proj (\<nat>\<^sub>c\<times>\<^sub>c \<nat>\<^sub>c) \<nat>\<^sub>c), 
+             (right_cart_proj (\<nat>\<^sub>c\<times>\<^sub>c \<nat>\<^sub>c) \<nat>\<^sub>c)\<rangle>, mult_uncurried \<circ>\<^sub>c \<langle>(right_cart_proj \<nat>\<^sub>c \<nat>\<^sub>c)\<circ>\<^sub>c
+            (left_cart_proj (\<nat>\<^sub>c\<times>\<^sub>c \<nat>\<^sub>c) \<nat>\<^sub>c),
+(right_cart_proj (\<nat>\<^sub>c\<times>\<^sub>c \<nat>\<^sub>c) \<nat>\<^sub>c)\<rangle>\<rangle>)\<^sup>\<sharp> \<circ>\<^sub>c
+c\<rangle> : one \<rightarrow>  (\<nat>\<^sub>c\<times>\<^sub>c \<nat>\<^sub>c)\<times>\<^sub>c (\<nat>\<^sub>c \<^bsup>(\<nat>\<^sub>c\<times>\<^sub>c \<nat>\<^sub>c)\<^esup>)"
+     using ab_type assms(3) cfunc_prod_type long_sharp_type by auto
+
 
 
 
@@ -5106,6 +5128,1123 @@ qed
 
 (*And... *)
 
+have fact7a:  "((eval_func \<nat>\<^sub>c (\<nat>\<^sub>c\<times>\<^sub>c \<nat>\<^sub>c))\<circ>\<^sub>c 
+            (id\<^sub>c (\<nat>\<^sub>c\<times>\<^sub>c \<nat>\<^sub>c) \<times>\<^sub>f(add_uncurried \<circ>\<^sub>c (add_uncurried \<times>\<^sub>f id\<^sub>c \<nat>\<^sub>c) 
+ \<circ>\<^sub>c \<langle>left_cart_proj (\<nat>\<^sub>c\<times>\<^sub>c \<nat>\<^sub>c) (\<nat>\<^sub>c\<^bsup>(\<nat>\<^sub>c\<times>\<^sub>c\<nat>\<^sub>c)\<^esup>), 
+(eval_func \<nat>\<^sub>c (\<nat>\<^sub>c\<times>\<^sub>c \<nat>\<^sub>c))\<rangle>)\<^sup>\<sharp>  \<circ>\<^sub>c (add_uncurried \<circ>\<^sub>c\<langle>mult_uncurried \<circ>\<^sub>c \<langle>(left_cart_proj \<nat>\<^sub>c \<nat>\<^sub>c) \<circ>\<^sub>c (left_cart_proj (\<nat>\<^sub>c\<times>\<^sub>c \<nat>\<^sub>c) \<nat>\<^sub>c), 
+             (right_cart_proj (\<nat>\<^sub>c\<times>\<^sub>c \<nat>\<^sub>c) \<nat>\<^sub>c)\<rangle>, mult_uncurried \<circ>\<^sub>c \<langle>(right_cart_proj \<nat>\<^sub>c \<nat>\<^sub>c)\<circ>\<^sub>c
+            (left_cart_proj (\<nat>\<^sub>c\<times>\<^sub>c \<nat>\<^sub>c) \<nat>\<^sub>c),(right_cart_proj (\<nat>\<^sub>c\<times>\<^sub>c \<nat>\<^sub>c) \<nat>\<^sub>c)\<rangle>\<rangle>)\<^sup>\<sharp>))
+\<circ>\<^sub>c \<langle>\<langle>a,b\<rangle>,c\<rangle> = (a \<cdot>\<^sub>\<nat> (successor \<circ>\<^sub>c c)) +\<^sub>\<nat> (b \<cdot>\<^sub>\<nat> (successor \<circ>\<^sub>c c))"
+
+
+proof - 
+  have "((eval_func \<nat>\<^sub>c (\<nat>\<^sub>c\<times>\<^sub>c \<nat>\<^sub>c))\<circ>\<^sub>c 
+            (id\<^sub>c (\<nat>\<^sub>c\<times>\<^sub>c \<nat>\<^sub>c) \<times>\<^sub>f(add_uncurried \<circ>\<^sub>c (add_uncurried \<times>\<^sub>f id\<^sub>c \<nat>\<^sub>c) 
+ \<circ>\<^sub>c \<langle>left_cart_proj (\<nat>\<^sub>c\<times>\<^sub>c \<nat>\<^sub>c) (\<nat>\<^sub>c\<^bsup>(\<nat>\<^sub>c\<times>\<^sub>c\<nat>\<^sub>c)\<^esup>), 
+(eval_func \<nat>\<^sub>c (\<nat>\<^sub>c\<times>\<^sub>c \<nat>\<^sub>c))\<rangle>)\<^sup>\<sharp>  \<circ>\<^sub>c (add_uncurried \<circ>\<^sub>c\<langle>mult_uncurried \<circ>\<^sub>c \<langle>(left_cart_proj \<nat>\<^sub>c \<nat>\<^sub>c) \<circ>\<^sub>c (left_cart_proj (\<nat>\<^sub>c\<times>\<^sub>c \<nat>\<^sub>c) \<nat>\<^sub>c), 
+             (right_cart_proj (\<nat>\<^sub>c\<times>\<^sub>c \<nat>\<^sub>c) \<nat>\<^sub>c)\<rangle>, mult_uncurried \<circ>\<^sub>c \<langle>(right_cart_proj \<nat>\<^sub>c \<nat>\<^sub>c)\<circ>\<^sub>c
+            (left_cart_proj (\<nat>\<^sub>c\<times>\<^sub>c \<nat>\<^sub>c) \<nat>\<^sub>c),(right_cart_proj (\<nat>\<^sub>c\<times>\<^sub>c \<nat>\<^sub>c) \<nat>\<^sub>c)\<rangle>\<rangle>)\<^sup>\<sharp>))
+\<circ>\<^sub>c \<langle>\<langle>a,b\<rangle>,c\<rangle> =
+((eval_func \<nat>\<^sub>c (\<nat>\<^sub>c\<times>\<^sub>c \<nat>\<^sub>c))\<circ>\<^sub>c 
+            (id\<^sub>c (\<nat>\<^sub>c\<times>\<^sub>c \<nat>\<^sub>c) \<times>\<^sub>f(add_uncurried \<circ>\<^sub>c (add_uncurried \<times>\<^sub>f id\<^sub>c \<nat>\<^sub>c) 
+ \<circ>\<^sub>c \<langle>left_cart_proj (\<nat>\<^sub>c\<times>\<^sub>c \<nat>\<^sub>c) (\<nat>\<^sub>c\<^bsup>(\<nat>\<^sub>c\<times>\<^sub>c\<nat>\<^sub>c)\<^esup>), 
+(eval_func \<nat>\<^sub>c (\<nat>\<^sub>c\<times>\<^sub>c \<nat>\<^sub>c))\<rangle>)\<^sup>\<sharp>  ) \<circ>\<^sub>c  
+ (id\<^sub>c (\<nat>\<^sub>c\<times>\<^sub>c \<nat>\<^sub>c) \<times>\<^sub>f (add_uncurried \<circ>\<^sub>c\<langle>mult_uncurried \<circ>\<^sub>c \<langle>(left_cart_proj \<nat>\<^sub>c \<nat>\<^sub>c) \<circ>\<^sub>c (left_cart_proj (\<nat>\<^sub>c\<times>\<^sub>c \<nat>\<^sub>c) \<nat>\<^sub>c), 
+             (right_cart_proj (\<nat>\<^sub>c\<times>\<^sub>c \<nat>\<^sub>c) \<nat>\<^sub>c)\<rangle>, mult_uncurried \<circ>\<^sub>c \<langle>(right_cart_proj \<nat>\<^sub>c \<nat>\<^sub>c)\<circ>\<^sub>c
+            (left_cart_proj (\<nat>\<^sub>c\<times>\<^sub>c \<nat>\<^sub>c) \<nat>\<^sub>c),
+(right_cart_proj (\<nat>\<^sub>c\<times>\<^sub>c \<nat>\<^sub>c) \<nat>\<^sub>c)\<rangle>\<rangle>)\<^sup>\<sharp>)) \<circ>\<^sub>c \<langle>\<langle>a,b\<rangle>,c\<rangle> "
+    using addAddIdPiEvalSharp_type identity_distributes_across_composition long_sharp_type by auto
+  also have "... = ((add_uncurried \<circ>\<^sub>c (add_uncurried \<times>\<^sub>f id\<^sub>c \<nat>\<^sub>c) 
+ \<circ>\<^sub>c \<langle>left_cart_proj (\<nat>\<^sub>c\<times>\<^sub>c \<nat>\<^sub>c) (\<nat>\<^sub>c\<^bsup>(\<nat>\<^sub>c\<times>\<^sub>c\<nat>\<^sub>c)\<^esup>), 
+(eval_func \<nat>\<^sub>c (\<nat>\<^sub>c\<times>\<^sub>c \<nat>\<^sub>c))\<rangle>) \<circ>\<^sub>c
+(id\<^sub>c (\<nat>\<^sub>c\<times>\<^sub>c \<nat>\<^sub>c) \<times>\<^sub>f (add_uncurried \<circ>\<^sub>c\<langle>mult_uncurried \<circ>\<^sub>c \<langle>(left_cart_proj \<nat>\<^sub>c \<nat>\<^sub>c) \<circ>\<^sub>c (left_cart_proj (\<nat>\<^sub>c\<times>\<^sub>c \<nat>\<^sub>c) \<nat>\<^sub>c), 
+             (right_cart_proj (\<nat>\<^sub>c\<times>\<^sub>c \<nat>\<^sub>c) \<nat>\<^sub>c)\<rangle>, mult_uncurried \<circ>\<^sub>c \<langle>(right_cart_proj \<nat>\<^sub>c \<nat>\<^sub>c)\<circ>\<^sub>c
+            (left_cart_proj (\<nat>\<^sub>c\<times>\<^sub>c \<nat>\<^sub>c) \<nat>\<^sub>c),
+(right_cart_proj (\<nat>\<^sub>c\<times>\<^sub>c \<nat>\<^sub>c) \<nat>\<^sub>c)\<rangle>\<rangle>)\<^sup>\<sharp>)) \<circ>\<^sub>c \<langle>\<langle>a,b\<rangle>,c\<rangle> "
+    using addAddIdPiEval_type comp_associative transpose_func_def by auto
+  also have "... =  (add_uncurried \<circ>\<^sub>c (add_uncurried \<times>\<^sub>f id\<^sub>c \<nat>\<^sub>c) 
+ \<circ>\<^sub>c \<langle>left_cart_proj (\<nat>\<^sub>c\<times>\<^sub>c \<nat>\<^sub>c) (\<nat>\<^sub>c\<^bsup>(\<nat>\<^sub>c\<times>\<^sub>c\<nat>\<^sub>c)\<^esup>), 
+(eval_func \<nat>\<^sub>c (\<nat>\<^sub>c\<times>\<^sub>c \<nat>\<^sub>c))\<rangle>) \<circ>\<^sub>c
+(id\<^sub>c (\<nat>\<^sub>c\<times>\<^sub>c \<nat>\<^sub>c) \<times>\<^sub>f (add_uncurried \<circ>\<^sub>c\<langle>mult_uncurried \<circ>\<^sub>c \<langle>(left_cart_proj \<nat>\<^sub>c \<nat>\<^sub>c) \<circ>\<^sub>c (left_cart_proj (\<nat>\<^sub>c\<times>\<^sub>c \<nat>\<^sub>c) \<nat>\<^sub>c), 
+             (right_cart_proj (\<nat>\<^sub>c\<times>\<^sub>c \<nat>\<^sub>c) \<nat>\<^sub>c)\<rangle>, mult_uncurried \<circ>\<^sub>c \<langle>(right_cart_proj \<nat>\<^sub>c \<nat>\<^sub>c)\<circ>\<^sub>c
+            (left_cart_proj (\<nat>\<^sub>c\<times>\<^sub>c \<nat>\<^sub>c) \<nat>\<^sub>c),
+(right_cart_proj (\<nat>\<^sub>c\<times>\<^sub>c \<nat>\<^sub>c) \<nat>\<^sub>c)\<rangle>\<rangle>)\<^sup>\<sharp>) \<circ>\<^sub>c \<langle>\<langle>a,b\<rangle>,c\<rangle> "
+    using comp_associative by auto
+  also have "... = (add_uncurried \<circ>\<^sub>c (add_uncurried \<times>\<^sub>f id\<^sub>c \<nat>\<^sub>c) 
+ \<circ>\<^sub>c \<langle>left_cart_proj (\<nat>\<^sub>c\<times>\<^sub>c \<nat>\<^sub>c) (\<nat>\<^sub>c\<^bsup>(\<nat>\<^sub>c\<times>\<^sub>c\<nat>\<^sub>c)\<^esup>), 
+(eval_func \<nat>\<^sub>c (\<nat>\<^sub>c\<times>\<^sub>c \<nat>\<^sub>c))\<rangle>)  \<circ>\<^sub>c \<langle>id\<^sub>c (\<nat>\<^sub>c\<times>\<^sub>c \<nat>\<^sub>c)\<circ>\<^sub>c \<langle>a,b\<rangle>,
+(add_uncurried \<circ>\<^sub>c\<langle>mult_uncurried \<circ>\<^sub>c \<langle>(left_cart_proj \<nat>\<^sub>c \<nat>\<^sub>c) \<circ>\<^sub>c (left_cart_proj (\<nat>\<^sub>c\<times>\<^sub>c \<nat>\<^sub>c) \<nat>\<^sub>c), 
+             (right_cart_proj (\<nat>\<^sub>c\<times>\<^sub>c \<nat>\<^sub>c) \<nat>\<^sub>c)\<rangle>, mult_uncurried \<circ>\<^sub>c \<langle>(right_cart_proj \<nat>\<^sub>c \<nat>\<^sub>c)\<circ>\<^sub>c
+            (left_cart_proj (\<nat>\<^sub>c\<times>\<^sub>c \<nat>\<^sub>c) \<nat>\<^sub>c),
+(right_cart_proj (\<nat>\<^sub>c\<times>\<^sub>c \<nat>\<^sub>c) \<nat>\<^sub>c)\<rangle>\<rangle>)\<^sup>\<sharp> \<circ>\<^sub>c
+c\<rangle> "
+    using ab_type assms(3) cfunc_cross_prod_comp_cfunc_prod id_type long_sharp_type by fastforce
+  also have "... =  (add_uncurried \<circ>\<^sub>c (add_uncurried \<times>\<^sub>f id\<^sub>c \<nat>\<^sub>c) 
+ \<circ>\<^sub>c \<langle>left_cart_proj (\<nat>\<^sub>c\<times>\<^sub>c \<nat>\<^sub>c) (\<nat>\<^sub>c\<^bsup>(\<nat>\<^sub>c\<times>\<^sub>c\<nat>\<^sub>c)\<^esup>), 
+(eval_func \<nat>\<^sub>c (\<nat>\<^sub>c\<times>\<^sub>c \<nat>\<^sub>c))\<rangle>)  \<circ>\<^sub>c \<langle>\<langle>a,b\<rangle>,
+(add_uncurried \<circ>\<^sub>c\<langle>mult_uncurried \<circ>\<^sub>c \<langle>(left_cart_proj \<nat>\<^sub>c \<nat>\<^sub>c) \<circ>\<^sub>c (left_cart_proj (\<nat>\<^sub>c\<times>\<^sub>c \<nat>\<^sub>c) \<nat>\<^sub>c), 
+             (right_cart_proj (\<nat>\<^sub>c\<times>\<^sub>c \<nat>\<^sub>c) \<nat>\<^sub>c)\<rangle>, mult_uncurried \<circ>\<^sub>c \<langle>(right_cart_proj \<nat>\<^sub>c \<nat>\<^sub>c)\<circ>\<^sub>c
+            (left_cart_proj (\<nat>\<^sub>c\<times>\<^sub>c \<nat>\<^sub>c) \<nat>\<^sub>c),
+(right_cart_proj (\<nat>\<^sub>c\<times>\<^sub>c \<nat>\<^sub>c) \<nat>\<^sub>c)\<rangle>\<rangle>)\<^sup>\<sharp> \<circ>\<^sub>c
+c\<rangle> "
+    using ab_type id_left_unit2 by auto
+  also have "... =  add_uncurried \<circ>\<^sub>c (
+(add_uncurried \<times>\<^sub>f id\<^sub>c \<nat>\<^sub>c) 
+ \<circ>\<^sub>c \<langle>left_cart_proj (\<nat>\<^sub>c\<times>\<^sub>c \<nat>\<^sub>c) (\<nat>\<^sub>c\<^bsup>(\<nat>\<^sub>c\<times>\<^sub>c\<nat>\<^sub>c)\<^esup>), 
+(eval_func \<nat>\<^sub>c (\<nat>\<^sub>c\<times>\<^sub>c \<nat>\<^sub>c))\<rangle> ) \<circ>\<^sub>c \<langle>
+\<langle>a,b\<rangle>,
+(add_uncurried \<circ>\<^sub>c\<langle>mult_uncurried \<circ>\<^sub>c \<langle>(left_cart_proj \<nat>\<^sub>c \<nat>\<^sub>c) \<circ>\<^sub>c (left_cart_proj (\<nat>\<^sub>c\<times>\<^sub>c \<nat>\<^sub>c) \<nat>\<^sub>c), 
+             (right_cart_proj (\<nat>\<^sub>c\<times>\<^sub>c \<nat>\<^sub>c) \<nat>\<^sub>c)\<rangle>, mult_uncurried \<circ>\<^sub>c \<langle>(right_cart_proj \<nat>\<^sub>c \<nat>\<^sub>c)\<circ>\<^sub>c
+            (left_cart_proj (\<nat>\<^sub>c\<times>\<^sub>c \<nat>\<^sub>c) \<nat>\<^sub>c),
+(right_cart_proj (\<nat>\<^sub>c\<times>\<^sub>c \<nat>\<^sub>c) \<nat>\<^sub>c)\<rangle>\<rangle>)\<^sup>\<sharp> \<circ>\<^sub>c
+c\<rangle> "
+    by (simp add: comp_associative)
+  also have "... = 
+ add_uncurried \<circ>\<^sub>c \<langle>
+add_uncurried \<circ>\<^sub>c left_cart_proj (\<nat>\<^sub>c\<times>\<^sub>c \<nat>\<^sub>c) (\<nat>\<^sub>c\<^bsup>(\<nat>\<^sub>c\<times>\<^sub>c\<nat>\<^sub>c)\<^esup>),  id\<^sub>c \<nat>\<^sub>c \<circ>\<^sub>c(eval_func \<nat>\<^sub>c (\<nat>\<^sub>c\<times>\<^sub>c \<nat>\<^sub>c))  \<rangle>  
+ \<circ>\<^sub>c \<langle>
+\<langle>a,b\<rangle>,
+(add_uncurried \<circ>\<^sub>c\<langle>mult_uncurried \<circ>\<^sub>c \<langle>(left_cart_proj \<nat>\<^sub>c \<nat>\<^sub>c) \<circ>\<^sub>c (left_cart_proj (\<nat>\<^sub>c\<times>\<^sub>c \<nat>\<^sub>c) \<nat>\<^sub>c), 
+             (right_cart_proj (\<nat>\<^sub>c\<times>\<^sub>c \<nat>\<^sub>c) \<nat>\<^sub>c)\<rangle>, mult_uncurried \<circ>\<^sub>c \<langle>(right_cart_proj \<nat>\<^sub>c \<nat>\<^sub>c)\<circ>\<^sub>c
+            (left_cart_proj (\<nat>\<^sub>c\<times>\<^sub>c \<nat>\<^sub>c) \<nat>\<^sub>c),
+(right_cart_proj (\<nat>\<^sub>c\<times>\<^sub>c \<nat>\<^sub>c) \<nat>\<^sub>c)\<rangle>\<rangle>)\<^sup>\<sharp> \<circ>\<^sub>c
+c\<rangle> "
+    by (smt add_uncurried_type cfunc_cross_prod_comp_cfunc_prod eval_func_type id_type left_cart_proj_type)
+  also have "... = 
+ add_uncurried \<circ>\<^sub>c \<langle>
+add_uncurried \<circ>\<^sub>c left_cart_proj (\<nat>\<^sub>c\<times>\<^sub>c \<nat>\<^sub>c) (\<nat>\<^sub>c\<^bsup>(\<nat>\<^sub>c\<times>\<^sub>c\<nat>\<^sub>c)\<^esup>),  (eval_func \<nat>\<^sub>c (\<nat>\<^sub>c\<times>\<^sub>c \<nat>\<^sub>c))  \<rangle>  
+ \<circ>\<^sub>c \<langle>
+\<langle>a,b\<rangle>,
+(add_uncurried \<circ>\<^sub>c\<langle>mult_uncurried \<circ>\<^sub>c \<langle>(left_cart_proj \<nat>\<^sub>c \<nat>\<^sub>c) \<circ>\<^sub>c (left_cart_proj (\<nat>\<^sub>c\<times>\<^sub>c \<nat>\<^sub>c) \<nat>\<^sub>c), 
+             (right_cart_proj (\<nat>\<^sub>c\<times>\<^sub>c \<nat>\<^sub>c) \<nat>\<^sub>c)\<rangle>, mult_uncurried \<circ>\<^sub>c \<langle>(right_cart_proj \<nat>\<^sub>c \<nat>\<^sub>c)\<circ>\<^sub>c
+            (left_cart_proj (\<nat>\<^sub>c\<times>\<^sub>c \<nat>\<^sub>c) \<nat>\<^sub>c),
+(right_cart_proj (\<nat>\<^sub>c\<times>\<^sub>c \<nat>\<^sub>c) \<nat>\<^sub>c)\<rangle>\<rangle>)\<^sup>\<sharp> \<circ>\<^sub>c
+c\<rangle> "
+    by (metis eval_func_type id_left_unit2)
+  also have "... =  
+add_uncurried \<circ>\<^sub>c \<langle>
+add_uncurried \<circ>\<^sub>c left_cart_proj (\<nat>\<^sub>c\<times>\<^sub>c \<nat>\<^sub>c) (\<nat>\<^sub>c\<^bsup>(\<nat>\<^sub>c\<times>\<^sub>c\<nat>\<^sub>c)\<^esup>)
+ \<circ>\<^sub>c \<langle>
+\<langle>a,b\<rangle>,
+(add_uncurried \<circ>\<^sub>c\<langle>mult_uncurried \<circ>\<^sub>c \<langle>(left_cart_proj \<nat>\<^sub>c \<nat>\<^sub>c) \<circ>\<^sub>c (left_cart_proj (\<nat>\<^sub>c\<times>\<^sub>c \<nat>\<^sub>c) \<nat>\<^sub>c), 
+             (right_cart_proj (\<nat>\<^sub>c\<times>\<^sub>c \<nat>\<^sub>c) \<nat>\<^sub>c)\<rangle>, mult_uncurried \<circ>\<^sub>c \<langle>(right_cart_proj \<nat>\<^sub>c \<nat>\<^sub>c)\<circ>\<^sub>c
+            (left_cart_proj (\<nat>\<^sub>c\<times>\<^sub>c \<nat>\<^sub>c) \<nat>\<^sub>c),
+(right_cart_proj (\<nat>\<^sub>c\<times>\<^sub>c \<nat>\<^sub>c) \<nat>\<^sub>c)\<rangle>\<rangle>)\<^sup>\<sharp> \<circ>\<^sub>c
+c\<rangle>
+,  (eval_func \<nat>\<^sub>c (\<nat>\<^sub>c\<times>\<^sub>c \<nat>\<^sub>c)) 
+ \<circ>\<^sub>c \<langle>
+\<langle>a,b\<rangle>,
+(add_uncurried \<circ>\<^sub>c\<langle>mult_uncurried \<circ>\<^sub>c \<langle>(left_cart_proj \<nat>\<^sub>c \<nat>\<^sub>c) \<circ>\<^sub>c (left_cart_proj (\<nat>\<^sub>c\<times>\<^sub>c \<nat>\<^sub>c) \<nat>\<^sub>c), 
+             (right_cart_proj (\<nat>\<^sub>c\<times>\<^sub>c \<nat>\<^sub>c) \<nat>\<^sub>c)\<rangle>, mult_uncurried \<circ>\<^sub>c \<langle>(right_cart_proj \<nat>\<^sub>c \<nat>\<^sub>c)\<circ>\<^sub>c
+            (left_cart_proj (\<nat>\<^sub>c\<times>\<^sub>c \<nat>\<^sub>c) \<nat>\<^sub>c),
+(right_cart_proj (\<nat>\<^sub>c\<times>\<^sub>c \<nat>\<^sub>c) \<nat>\<^sub>c)\<rangle>\<rangle>)\<^sup>\<sharp> \<circ>\<^sub>c
+c\<rangle>
+ \<rangle>"
+    using cfunc_prod_comp addP0_type comp_associative evalu_type very_long_type by auto
+  also have "... =add_uncurried \<circ>\<^sub>c \<langle>
+add_uncurried \<circ>\<^sub>c \<langle>a,b\<rangle>
+,  (eval_func \<nat>\<^sub>c (\<nat>\<^sub>c\<times>\<^sub>c \<nat>\<^sub>c)) 
+ \<circ>\<^sub>c \<langle>\<langle>a,b\<rangle>,
+(add_uncurried \<circ>\<^sub>c\<langle>mult_uncurried \<circ>\<^sub>c \<langle>(left_cart_proj \<nat>\<^sub>c \<nat>\<^sub>c) \<circ>\<^sub>c (left_cart_proj (\<nat>\<^sub>c\<times>\<^sub>c \<nat>\<^sub>c) \<nat>\<^sub>c), 
+             (right_cart_proj (\<nat>\<^sub>c\<times>\<^sub>c \<nat>\<^sub>c) \<nat>\<^sub>c)\<rangle>, mult_uncurried \<circ>\<^sub>c 
+\<langle>(right_cart_proj \<nat>\<^sub>c \<nat>\<^sub>c)\<circ>\<^sub>c
+            (left_cart_proj (\<nat>\<^sub>c\<times>\<^sub>c \<nat>\<^sub>c) \<nat>\<^sub>c),
+(right_cart_proj (\<nat>\<^sub>c\<times>\<^sub>c \<nat>\<^sub>c) \<nat>\<^sub>c)\<rangle>\<rangle>)\<^sup>\<sharp> \<circ>\<^sub>c
+c\<rangle>
+ \<rangle>" 
+    using left_cart_proj_cfunc_prod ab_type long_sharp_c_type by auto
+  also have "... = add_uncurried \<circ>\<^sub>c \<langle>
+add_uncurried \<circ>\<^sub>c \<langle>a,b\<rangle>
+,  (eval_func \<nat>\<^sub>c (\<nat>\<^sub>c\<times>\<^sub>c \<nat>\<^sub>c)) 
+ \<circ>\<^sub>c \<langle>id\<^sub>c (\<nat>\<^sub>c\<times>\<^sub>c \<nat>\<^sub>c) \<circ>\<^sub>c \<langle>a,b\<rangle>,
+(add_uncurried \<circ>\<^sub>c\<langle>mult_uncurried \<circ>\<^sub>c \<langle>(left_cart_proj \<nat>\<^sub>c \<nat>\<^sub>c) \<circ>\<^sub>c (left_cart_proj (\<nat>\<^sub>c\<times>\<^sub>c \<nat>\<^sub>c) \<nat>\<^sub>c), 
+             (right_cart_proj (\<nat>\<^sub>c\<times>\<^sub>c \<nat>\<^sub>c) \<nat>\<^sub>c)\<rangle>, mult_uncurried \<circ>\<^sub>c 
+\<langle>(right_cart_proj \<nat>\<^sub>c \<nat>\<^sub>c)\<circ>\<^sub>c
+            (left_cart_proj (\<nat>\<^sub>c\<times>\<^sub>c \<nat>\<^sub>c) \<nat>\<^sub>c),
+(right_cart_proj (\<nat>\<^sub>c\<times>\<^sub>c \<nat>\<^sub>c) \<nat>\<^sub>c)\<rangle>\<rangle>)\<^sup>\<sharp> \<circ>\<^sub>c
+c\<rangle>
+ \<rangle>"
+    using ab_type id_left_unit2 by auto
+  also have "... = 
+add_uncurried \<circ>\<^sub>c \<langle>
+add_uncurried \<circ>\<^sub>c \<langle>a,b\<rangle>
+,  (eval_func \<nat>\<^sub>c (\<nat>\<^sub>c\<times>\<^sub>c \<nat>\<^sub>c)) 
+ \<circ>\<^sub>c (id\<^sub>c (\<nat>\<^sub>c\<times>\<^sub>c \<nat>\<^sub>c) \<times>\<^sub>f (add_uncurried \<circ>\<^sub>c\<langle>mult_uncurried \<circ>\<^sub>c \<langle>(left_cart_proj \<nat>\<^sub>c \<nat>\<^sub>c) \<circ>\<^sub>c (left_cart_proj (\<nat>\<^sub>c\<times>\<^sub>c \<nat>\<^sub>c) \<nat>\<^sub>c), 
+             (right_cart_proj (\<nat>\<^sub>c\<times>\<^sub>c \<nat>\<^sub>c) \<nat>\<^sub>c)\<rangle>, mult_uncurried \<circ>\<^sub>c 
+\<langle>(right_cart_proj \<nat>\<^sub>c \<nat>\<^sub>c)\<circ>\<^sub>c
+            (left_cart_proj (\<nat>\<^sub>c\<times>\<^sub>c \<nat>\<^sub>c) \<nat>\<^sub>c),
+(right_cart_proj (\<nat>\<^sub>c\<times>\<^sub>c \<nat>\<^sub>c) \<nat>\<^sub>c)\<rangle>\<rangle>)\<^sup>\<sharp>) \<circ>\<^sub>c \<langle> \<langle>a,b\<rangle>,c\<rangle> \<rangle>"
+    using ab_type assms(3) cfunc_cross_prod_comp_cfunc_prod id_type long_sharp_type by fastforce
+  also have "... = 
+add_uncurried \<circ>\<^sub>c \<langle>
+add_uncurried \<circ>\<^sub>c \<langle>a,b\<rangle>
+,  (add_uncurried \<circ>\<^sub>c\<langle>mult_uncurried \<circ>\<^sub>c \<langle>(left_cart_proj \<nat>\<^sub>c \<nat>\<^sub>c) \<circ>\<^sub>c (left_cart_proj (\<nat>\<^sub>c\<times>\<^sub>c \<nat>\<^sub>c) \<nat>\<^sub>c), 
+             (right_cart_proj (\<nat>\<^sub>c\<times>\<^sub>c \<nat>\<^sub>c) \<nat>\<^sub>c)\<rangle>, mult_uncurried \<circ>\<^sub>c 
+\<langle>(right_cart_proj \<nat>\<^sub>c \<nat>\<^sub>c)\<circ>\<^sub>c
+            (left_cart_proj (\<nat>\<^sub>c\<times>\<^sub>c \<nat>\<^sub>c) \<nat>\<^sub>c),
+(right_cart_proj (\<nat>\<^sub>c\<times>\<^sub>c \<nat>\<^sub>c) \<nat>\<^sub>c)\<rangle>\<rangle>) \<circ>\<^sub>c \<langle> \<langle>a,b\<rangle>,c\<rangle> \<rangle>"
+    using comp_associative long_type transpose_func_def by presburger
+  also have "... = add_uncurried \<circ>\<^sub>c \<langle>
+add_uncurried \<circ>\<^sub>c \<langle>a,b\<rangle>
+,  add_uncurried \<circ>\<^sub>c\<langle>mult_uncurried \<circ>\<^sub>c \<langle>(left_cart_proj \<nat>\<^sub>c \<nat>\<^sub>c) \<circ>\<^sub>c (left_cart_proj (\<nat>\<^sub>c\<times>\<^sub>c \<nat>\<^sub>c) \<nat>\<^sub>c), 
+             (right_cart_proj (\<nat>\<^sub>c\<times>\<^sub>c \<nat>\<^sub>c) \<nat>\<^sub>c)\<rangle>
+
+, mult_uncurried \<circ>\<^sub>c
+\<langle>(right_cart_proj \<nat>\<^sub>c \<nat>\<^sub>c)\<circ>\<^sub>c
+            (left_cart_proj (\<nat>\<^sub>c\<times>\<^sub>c \<nat>\<^sub>c) \<nat>\<^sub>c),
+(right_cart_proj (\<nat>\<^sub>c\<times>\<^sub>c \<nat>\<^sub>c) \<nat>\<^sub>c)\<rangle>\<rangle> \<circ>\<^sub>c \<langle> \<langle>a,b\<rangle>,c\<rangle> \<rangle>"
+    by (simp add: comp_associative)
+ also have "... = add_uncurried \<circ>\<^sub>c \<langle>
+add_uncurried \<circ>\<^sub>c \<langle>a,b\<rangle>
+,  add_uncurried \<circ>\<^sub>c\<langle>mult_uncurried \<circ>\<^sub>c \<langle>(left_cart_proj \<nat>\<^sub>c \<nat>\<^sub>c) \<circ>\<^sub>c (left_cart_proj (\<nat>\<^sub>c\<times>\<^sub>c \<nat>\<^sub>c) \<nat>\<^sub>c), 
+             (right_cart_proj (\<nat>\<^sub>c\<times>\<^sub>c \<nat>\<^sub>c) \<nat>\<^sub>c)\<rangle> \<circ>\<^sub>c \<langle> \<langle>a,b\<rangle>,c\<rangle>
+
+, mult_uncurried \<circ>\<^sub>c
+\<langle>(right_cart_proj \<nat>\<^sub>c \<nat>\<^sub>c)\<circ>\<^sub>c
+            (left_cart_proj (\<nat>\<^sub>c\<times>\<^sub>c \<nat>\<^sub>c) \<nat>\<^sub>c),
+(right_cart_proj (\<nat>\<^sub>c\<times>\<^sub>c \<nat>\<^sub>c) \<nat>\<^sub>c)\<rangle>   \<circ>\<^sub>c \<langle> \<langle>a,b\<rangle>,c\<rangle> \<rangle>  \<rangle>"
+   using ABC_type cfunc_prod_comp comp_associative multp1p1p2_type right_type by auto
+  also have "... =add_uncurried \<circ>\<^sub>c \<langle>
+add_uncurried \<circ>\<^sub>c \<langle>a,b\<rangle>
+,  add_uncurried \<circ>\<^sub>c\<langle>mult_uncurried \<circ>\<^sub>c \<langle>(left_cart_proj \<nat>\<^sub>c \<nat>\<^sub>c) \<circ>\<^sub>c (left_cart_proj (\<nat>\<^sub>c\<times>\<^sub>c \<nat>\<^sub>c) \<nat>\<^sub>c), 
+             (right_cart_proj (\<nat>\<^sub>c\<times>\<^sub>c \<nat>\<^sub>c) \<nat>\<^sub>c)\<rangle> \<circ>\<^sub>c \<langle> \<langle>a,b\<rangle>,c\<rangle>
+
+, mult_uncurried \<circ>\<^sub>c
+\<langle>(right_cart_proj \<nat>\<^sub>c \<nat>\<^sub>c)\<circ>\<^sub>c
+            (left_cart_proj (\<nat>\<^sub>c\<times>\<^sub>c \<nat>\<^sub>c) \<nat>\<^sub>c) \<circ>\<^sub>c \<langle> \<langle>a,b\<rangle>,c\<rangle> ,
+(right_cart_proj (\<nat>\<^sub>c\<times>\<^sub>c \<nat>\<^sub>c) \<nat>\<^sub>c) \<circ>\<^sub>c \<langle> \<langle>a,b\<rangle>,c\<rangle>\<rangle>   \<rangle>  \<rangle>"
+    by (smt ABC_type cfunc_prod_comp comp_associative p2p1_type right_cart_proj_type)
+  also have "... = 
+add_uncurried \<circ>\<^sub>c \<langle>
+add_uncurried \<circ>\<^sub>c \<langle>a,b\<rangle>
+,  add_uncurried \<circ>\<^sub>c\<langle>mult_uncurried \<circ>\<^sub>c \<langle>(left_cart_proj \<nat>\<^sub>c \<nat>\<^sub>c) \<circ>\<^sub>c (left_cart_proj (\<nat>\<^sub>c\<times>\<^sub>c \<nat>\<^sub>c) \<nat>\<^sub>c) \<circ>\<^sub>c \<langle> \<langle>a,b\<rangle>,c\<rangle>, 
+             (right_cart_proj (\<nat>\<^sub>c\<times>\<^sub>c \<nat>\<^sub>c) \<nat>\<^sub>c) \<circ>\<^sub>c \<langle> \<langle>a,b\<rangle>,c\<rangle>\<rangle>
+
+, mult_uncurried \<circ>\<^sub>c
+\<langle>(right_cart_proj \<nat>\<^sub>c \<nat>\<^sub>c)\<circ>\<^sub>c
+            \<langle>a,b\<rangle>,
+c\<rangle>   \<rangle>  \<rangle>"
+    by (smt ABC_type ab_type assms(3) cfunc_prod_comp comp_associative left_cart_proj_cfunc_prod p1p1_type right_cart_proj_cfunc_prod right_cart_proj_type)
+  also have "... = 
+add_uncurried \<circ>\<^sub>c \<langle>
+add_uncurried \<circ>\<^sub>c \<langle>a,b\<rangle>
+,  add_uncurried \<circ>\<^sub>c\<langle>mult_uncurried \<circ>\<^sub>c 
+\<langle>(left_cart_proj \<nat>\<^sub>c \<nat>\<^sub>c) \<circ>\<^sub>c   \<langle>a,b\<rangle>, c\<rangle>,
+ mult_uncurried \<circ>\<^sub>c\<langle>b,c\<rangle>\<rangle>\<rangle>"
+    using ab_type assms(1) assms(2) assms(3) left_cart_proj_cfunc_prod right_cart_proj_cfunc_prod by auto
+  also have "... =
+add_uncurried \<circ>\<^sub>c \<langle>
+add_uncurried \<circ>\<^sub>c \<langle>a,b\<rangle>
+,  add_uncurried \<circ>\<^sub>c\<langle>mult_uncurried \<circ>\<^sub>c \<langle>a, c\<rangle>, mult_uncurried \<circ>\<^sub>c\<langle>b,c\<rangle>\<rangle>\<rangle>"
+    using assms(1) assms(2) left_cart_proj_cfunc_prod by auto
+  also have "... = (a +\<^sub>\<nat> b) +\<^sub>\<nat> (a \<cdot>\<^sub>\<nat> c +\<^sub>\<nat> b \<cdot>\<^sub>\<nat> c)"
+    by (simp add: add_def mult_def)
+  also have "... = a +\<^sub>\<nat> (b +\<^sub>\<nat> (a \<cdot>\<^sub>\<nat> c +\<^sub>\<nat> b \<cdot>\<^sub>\<nat> c))"
+    oops
+(*
+    also have "... = a +\<^sub>\<nat> ((b +\<^sub>\<nat> a \<cdot>\<^sub>\<nat> c) +\<^sub>\<nat> b \<cdot>\<^sub>\<nat> c)"
+
+ also have "... = a +\<^sub>\<nat> ((a \<cdot>\<^sub>\<nat> c  +\<^sub>\<nat> b) +\<^sub>\<nat> b \<cdot>\<^sub>\<nat> c)"
+ also have "... = a +\<^sub>\<nat> (a \<cdot>\<^sub>\<nat> c  +\<^sub>\<nat> (b +\<^sub>\<nat> b \<cdot>\<^sub>\<nat> c))"
+   also have "... = (a +\<^sub>\<nat> a \<cdot>\<^sub>\<nat> c)  +\<^sub>\<nat> (b +\<^sub>\<nat> b \<cdot>\<^sub>\<nat> c)"
+     also have "... = (a \<cdot>\<^sub>\<nat> (successor \<circ>\<^sub>c c)) +\<^sub>\<nat> (b \<cdot>\<^sub>\<nat> (successor \<circ>\<^sub>c c))"
+       
+*)
+
+lemma mult_commutative:
+  assumes "a \<in>\<^sub>c  \<nat>\<^sub>c"  "b\<in>\<^sub>c  \<nat>\<^sub>c" 
+  shows "a \<cdot>\<^sub>\<nat> b = b \<cdot>\<^sub>\<nat> a"
+
+proof - 
+  have a0_type: "\<langle>a,zero\<rangle>: one \<rightarrow>(\<nat>\<^sub>c\<times>\<^sub>c\<nat>\<^sub>c)"
+    by (simp add: assms(1) cfunc_prod_type zero_type)
+  have a1_type: "\<langle>a,id\<^sub>c one\<rangle>: one \<rightarrow>(\<nat>\<^sub>c\<times>\<^sub>c one)"
+    by (simp add: assms(1) cfunc_prod_type id_type)
+  have ab_typ: "\<langle>a,b\<rangle>: one \<rightarrow>(\<nat>\<^sub>c\<times>\<^sub>c\<nat>\<^sub>c)"
+    by (simp add: assms(1) assms(2) cfunc_prod_type)
+  have p1p0_type:  "\<langle>right_cart_proj \<nat>\<^sub>c \<nat>\<^sub>c,left_cart_proj \<nat>\<^sub>c \<nat>\<^sub>c\<rangle>: (\<nat>\<^sub>c\<times>\<^sub>c\<nat>\<^sub>c) \<rightarrow>  (\<nat>\<^sub>c\<times>\<^sub>c\<nat>\<^sub>c)"
+    by (simp add: cfunc_prod_type left_cart_proj_type right_cart_proj_type)
+  have multp1p0_tye: "mult_uncurried \<circ>\<^sub>c \<langle>right_cart_proj \<nat>\<^sub>c \<nat>\<^sub>c,left_cart_proj \<nat>\<^sub>c \<nat>\<^sub>c\<rangle>: (\<nat>\<^sub>c\<times>\<^sub>c\<nat>\<^sub>c) \<rightarrow> \<nat>\<^sub>c"
+    using comp_type mult_uncurried_type p1p0_type by blast 
+  have multp1p0sharp_type: "(mult_uncurried \<circ>\<^sub>c \<langle>right_cart_proj \<nat>\<^sub>c \<nat>\<^sub>c,left_cart_proj \<nat>\<^sub>c \<nat>\<^sub>c\<rangle>)\<^sup>\<sharp>: \<nat>\<^sub>c \<rightarrow> \<nat>\<^sub>c\<^bsup>\<nat>\<^sub>c\<^esup>"
+    by (simp add: multp1p0_tye transpose_func_def)
+  have  multp1p0sharp0_type: "(mult_uncurried \<circ>\<^sub>c \<langle>right_cart_proj \<nat>\<^sub>c \<nat>\<^sub>c,left_cart_proj \<nat>\<^sub>c \<nat>\<^sub>c\<rangle>)\<^sup>\<sharp>\<circ>\<^sub>c zero: one \<rightarrow> \<nat>\<^sub>c\<^bsup>\<nat>\<^sub>c\<^esup>"
+    using multp1p0sharp_type zero_type by auto
+  have  pi0eval_type: "\<langle>left_cart_proj \<nat>\<^sub>c (\<nat>\<^sub>c\<^bsup>\<nat>\<^sub>c\<^esup>), eval_func \<nat>\<^sub>c \<nat>\<^sub>c\<rangle>: \<nat>\<^sub>c\<times>\<^sub>c(\<nat>\<^sub>c\<^bsup>\<nat>\<^sub>c\<^esup>) \<rightarrow> (\<nat>\<^sub>c\<times>\<^sub>c\<nat>\<^sub>c)"
+    by (simp add: cfunc_prod_type eval_func_type left_cart_proj_type)
+  have addpi0eval_type: "add_uncurried \<circ>\<^sub>c \<langle>left_cart_proj \<nat>\<^sub>c (\<nat>\<^sub>c\<^bsup>\<nat>\<^sub>c\<^esup>), eval_func \<nat>\<^sub>c \<nat>\<^sub>c\<rangle>: \<nat>\<^sub>c\<times>\<^sub>c(\<nat>\<^sub>c\<^bsup>\<nat>\<^sub>c\<^esup>) \<rightarrow> \<nat>\<^sub>c"
+    by (simp add: f_mult_flat_type)
+  have addpi0evalsharp_type:  "(add_uncurried \<circ>\<^sub>c \<langle>left_cart_proj \<nat>\<^sub>c (\<nat>\<^sub>c\<^bsup>\<nat>\<^sub>c\<^esup>), eval_func \<nat>\<^sub>c \<nat>\<^sub>c\<rangle>)\<^sup>\<sharp>: (\<nat>\<^sub>c\<^bsup>\<nat>\<^sub>c\<^esup>) \<rightarrow> (\<nat>\<^sub>c\<^bsup>\<nat>\<^sub>c\<^esup>)"
+    by (simp add: f_mult_type)
+  have long_type: "(id\<^sub>c \<nat>\<^sub>c \<times>\<^sub>f (mult_uncurried \<circ>\<^sub>c \<langle>right_cart_proj \<nat>\<^sub>c \<nat>\<^sub>c,left_cart_proj \<nat>\<^sub>c \<nat>\<^sub>c\<rangle>)\<^sup>\<sharp>) \<circ>\<^sub>c \<langle>a,b\<rangle>: one \<rightarrow> \<nat>\<^sub>c\<times>\<^sub>c(\<nat>\<^sub>c\<^bsup>\<nat>\<^sub>c\<^esup>)"
+    using ab_typ cfunc_cross_prod_type id_type multp1p0sharp_type by auto
+
+
+  have f1: "(eval_func \<nat>\<^sub>c \<nat>\<^sub>c \<circ>\<^sub>c (id\<^sub>c \<nat>\<^sub>c \<times>\<^sub>f (mult_uncurried \<circ>\<^sub>c
+ \<langle>right_cart_proj \<nat>\<^sub>c \<nat>\<^sub>c,left_cart_proj \<nat>\<^sub>c \<nat>\<^sub>c\<rangle>)\<^sup>\<sharp>\<circ>\<^sub>c zero))\<circ>\<^sub>c \<langle>a,id\<^sub>c one\<rangle> = zero"
+  proof - 
+    have "(eval_func \<nat>\<^sub>c \<nat>\<^sub>c \<circ>\<^sub>c (id\<^sub>c \<nat>\<^sub>c \<times>\<^sub>f (mult_uncurried \<circ>\<^sub>c
+ \<langle>right_cart_proj \<nat>\<^sub>c \<nat>\<^sub>c,left_cart_proj \<nat>\<^sub>c \<nat>\<^sub>c\<rangle>)\<^sup>\<sharp>\<circ>\<^sub>c zero))\<circ>\<^sub>c \<langle>a,id\<^sub>c one\<rangle> = 
+eval_func \<nat>\<^sub>c \<nat>\<^sub>c \<circ>\<^sub>c (id\<^sub>c \<nat>\<^sub>c \<times>\<^sub>f (mult_uncurried \<circ>\<^sub>c
+ \<langle>right_cart_proj \<nat>\<^sub>c \<nat>\<^sub>c,left_cart_proj \<nat>\<^sub>c \<nat>\<^sub>c\<rangle>)\<^sup>\<sharp>\<circ>\<^sub>c zero)\<circ>\<^sub>c \<langle>a,id\<^sub>c one\<rangle>"
+      by (simp add: comp_associative)
+    also have "... = eval_func \<nat>\<^sub>c \<nat>\<^sub>c \<circ>\<^sub>c (id\<^sub>c \<nat>\<^sub>c \<times>\<^sub>f (mult_uncurried \<circ>\<^sub>c
+ \<langle>right_cart_proj \<nat>\<^sub>c \<nat>\<^sub>c,left_cart_proj \<nat>\<^sub>c \<nat>\<^sub>c\<rangle>)\<^sup>\<sharp>) \<circ>\<^sub>c (id\<^sub>c \<nat>\<^sub>c \<times>\<^sub>f zero)\<circ>\<^sub>c \<langle>a,id\<^sub>c one\<rangle>"
+      using comp_associative identity_distributes_across_composition multp1p0sharp_type zero_type by auto
+    also have "... = (mult_uncurried \<circ>\<^sub>c
+ \<langle>right_cart_proj \<nat>\<^sub>c \<nat>\<^sub>c,left_cart_proj \<nat>\<^sub>c \<nat>\<^sub>c\<rangle>)\<circ>\<^sub>c (id\<^sub>c \<nat>\<^sub>c \<times>\<^sub>f zero)\<circ>\<^sub>c \<langle>a,id\<^sub>c one\<rangle>"
+      using comp_associative flat_cancels_sharp inv_transpose_func_def2 multp1p0_tye multp1p0sharp_type by fastforce
+    also have "... = (mult_uncurried \<circ>\<^sub>c
+ \<langle>right_cart_proj \<nat>\<^sub>c \<nat>\<^sub>c,left_cart_proj \<nat>\<^sub>c \<nat>\<^sub>c\<rangle>) \<circ>\<^sub>c \<langle>id\<^sub>c \<nat>\<^sub>c\<circ>\<^sub>c  a, zero \<circ>\<^sub>c id\<^sub>c one\<rangle>"
+      by (smt assms(1) cfunc_cross_prod_comp_cfunc_prod id_type zero_type)
+    also have "... =  mult_uncurried \<circ>\<^sub>c
+ \<langle>right_cart_proj \<nat>\<^sub>c \<nat>\<^sub>c,left_cart_proj \<nat>\<^sub>c \<nat>\<^sub>c\<rangle> \<circ>\<^sub>c \<langle>a, zero\<rangle>"
+      using assms(1) comp_associative id_left_unit2 id_right_unit2 zero_type by auto
+    also have "... =  mult_uncurried \<circ>\<^sub>c
+ \<langle>right_cart_proj \<nat>\<^sub>c \<nat>\<^sub>c \<circ>\<^sub>c \<langle>a, zero\<rangle> ,left_cart_proj \<nat>\<^sub>c \<nat>\<^sub>c \<circ>\<^sub>c \<langle>a, zero\<rangle> \<rangle>"
+      using ETCS_HOL.swap_def assms(1) left_cart_proj_cfunc_prod right_cart_proj_cfunc_prod swap_ap zero_type by auto
+    also have "... =  mult_uncurried \<circ>\<^sub>c \<langle>zero , a\<rangle>"
+      using assms(1) left_cart_proj_cfunc_prod right_cart_proj_cfunc_prod zero_type by auto
+    also have "... = zero"
+      using assms(1) mult_def mult_respects_zero_left by auto
+then show ?thesis using calculation by auto
+qed
+(*
+  have f2: "(eval_func \<nat>\<^sub>c \<nat>\<^sub>c \<circ>\<^sub>c (id\<^sub>c \<nat>\<^sub>c \<times>\<^sub>f ((add_uncurried \<circ>\<^sub>c \<langle>left_cart_proj \<nat>\<^sub>c (\<nat>\<^sub>c\<^bsup>\<nat>\<^sub>c\<^esup>), eval_func \<nat>\<^sub>c \<nat>\<^sub>c\<rangle>)\<^sup>\<sharp>\<circ>\<^sub>c
+(mult_uncurried \<circ>\<^sub>c \<langle>right_cart_proj \<nat>\<^sub>c \<nat>\<^sub>c,left_cart_proj \<nat>\<^sub>c \<nat>\<^sub>c\<rangle>)\<^sup>\<sharp>)))\<circ>\<^sub>c \<langle>a,b\<rangle> = (successor \<circ>\<^sub>c a)  \<cdot>\<^sub>\<nat> b"
+  proof - 
+    have "(eval_func \<nat>\<^sub>c \<nat>\<^sub>c \<circ>\<^sub>c (id\<^sub>c \<nat>\<^sub>c \<times>\<^sub>f ((add_uncurried \<circ>\<^sub>c \<langle>left_cart_proj \<nat>\<^sub>c (\<nat>\<^sub>c\<^bsup>\<nat>\<^sub>c\<^esup>), eval_func \<nat>\<^sub>c \<nat>\<^sub>c\<rangle>)\<^sup>\<sharp>\<circ>\<^sub>c
+(mult_uncurried \<circ>\<^sub>c \<langle>right_cart_proj \<nat>\<^sub>c \<nat>\<^sub>c,left_cart_proj \<nat>\<^sub>c \<nat>\<^sub>c\<rangle>)\<^sup>\<sharp>)))\<circ>\<^sub>c \<langle>a,b\<rangle> = 
+  eval_func \<nat>\<^sub>c \<nat>\<^sub>c \<circ>\<^sub>c (id\<^sub>c \<nat>\<^sub>c \<times>\<^sub>f ((add_uncurried \<circ>\<^sub>c \<langle>left_cart_proj \<nat>\<^sub>c (\<nat>\<^sub>c\<^bsup>\<nat>\<^sub>c\<^esup>), eval_func \<nat>\<^sub>c \<nat>\<^sub>c\<rangle>)\<^sup>\<sharp>\<circ>\<^sub>c
+(mult_uncurried \<circ>\<^sub>c \<langle>right_cart_proj \<nat>\<^sub>c \<nat>\<^sub>c,left_cart_proj \<nat>\<^sub>c \<nat>\<^sub>c\<rangle>)\<^sup>\<sharp>))\<circ>\<^sub>c \<langle>a,b\<rangle>"
+      using comp_associative by auto
+    also have "... = eval_func \<nat>\<^sub>c \<nat>\<^sub>c \<circ>\<^sub>c (id\<^sub>c \<nat>\<^sub>c \<times>\<^sub>f ((add_uncurried \<circ>\<^sub>c \<langle>left_cart_proj \<nat>\<^sub>c (\<nat>\<^sub>c\<^bsup>\<nat>\<^sub>c\<^esup>), eval_func \<nat>\<^sub>c \<nat>\<^sub>c\<rangle>)\<^sup>\<sharp>))
+\<circ>\<^sub>c (id\<^sub>c \<nat>\<^sub>c \<times>\<^sub>f (mult_uncurried \<circ>\<^sub>c \<langle>right_cart_proj \<nat>\<^sub>c \<nat>\<^sub>c,left_cart_proj \<nat>\<^sub>c \<nat>\<^sub>c\<rangle>)\<^sup>\<sharp>) \<circ>\<^sub>c \<langle>a,b\<rangle>"
+      using comp_associative f_mult_type identity_distributes_across_composition multp1p0sharp_type by auto
+    also have "... = add_uncurried \<circ>\<^sub>c \<langle>left_cart_proj \<nat>\<^sub>c (\<nat>\<^sub>c\<^bsup>\<nat>\<^sub>c\<^esup>), eval_func \<nat>\<^sub>c \<nat>\<^sub>c\<rangle>
+\<circ>\<^sub>c (id\<^sub>c \<nat>\<^sub>c \<times>\<^sub>f (mult_uncurried \<circ>\<^sub>c \<langle>right_cart_proj \<nat>\<^sub>c \<nat>\<^sub>c,left_cart_proj \<nat>\<^sub>c \<nat>\<^sub>c\<rangle>)\<^sup>\<sharp>) \<circ>\<^sub>c \<langle>a,b\<rangle>"
+      using comp_associative f_mult_flat_type f_mult_type flat_cancels_sharp inv_transpose_func_def2 by fastforce
+    also have "... =  add_uncurried \<circ>\<^sub>c
+ \<langle>left_cart_proj \<nat>\<^sub>c (\<nat>\<^sub>c\<^bsup>\<nat>\<^sub>c\<^esup>)\<circ>\<^sub>c (id\<^sub>c \<nat>\<^sub>c \<times>\<^sub>f (mult_uncurried \<circ>\<^sub>c \<langle>right_cart_proj \<nat>\<^sub>c \<nat>\<^sub>c,left_cart_proj \<nat>\<^sub>c \<nat>\<^sub>c\<rangle>)\<^sup>\<sharp>) \<circ>\<^sub>c \<langle>a,b\<rangle> ,
+            eval_func \<nat>\<^sub>c \<nat>\<^sub>c \<circ>\<^sub>c (id\<^sub>c \<nat>\<^sub>c \<times>\<^sub>f (mult_uncurried \<circ>\<^sub>c \<langle>right_cart_proj \<nat>\<^sub>c \<nat>\<^sub>c,left_cart_proj \<nat>\<^sub>c \<nat>\<^sub>c\<rangle>)\<^sup>\<sharp>) \<circ>\<^sub>c \<langle>a,b\<rangle> \<rangle>"
+      using cfunc_prod_comp eval_func_type left_cart_proj_type long_type by fastforce
+    also have "... = add_uncurried \<circ>\<^sub>c
+ \<langle>left_cart_proj \<nat>\<^sub>c (\<nat>\<^sub>c\<^bsup>\<nat>\<^sub>c\<^esup>)\<circ>\<^sub>c (id\<^sub>c \<nat>\<^sub>c \<times>\<^sub>f (mult_uncurried \<circ>\<^sub>c \<langle>right_cart_proj \<nat>\<^sub>c \<nat>\<^sub>c,left_cart_proj \<nat>\<^sub>c \<nat>\<^sub>c\<rangle>)\<^sup>\<sharp>)  ,
+            eval_func \<nat>\<^sub>c \<nat>\<^sub>c \<circ>\<^sub>c (id\<^sub>c \<nat>\<^sub>c \<times>\<^sub>f (mult_uncurried \<circ>\<^sub>c \<langle>right_cart_proj \<nat>\<^sub>c \<nat>\<^sub>c,left_cart_proj \<nat>\<^sub>c \<nat>\<^sub>c\<rangle>)\<^sup>\<sharp>) \<rangle> \<circ>\<^sub>c \<langle>a,b\<rangle>"
+      by (smt ab_typ cfunc_prod_comp comp_associative id_left_unit2 id_type left_cart_proj_cfunc_cross_prod left_cart_proj_type multp1p0_tye transpose_func_def)
+    also have "... =  add_uncurried \<circ>\<^sub>c
+ \<langle>id\<^sub>c \<nat>\<^sub>c \<circ>\<^sub>c left_cart_proj \<nat>\<^sub>c \<nat>\<^sub>c , 
+    eval_func \<nat>\<^sub>c \<nat>\<^sub>c \<circ>\<^sub>c (id\<^sub>c \<nat>\<^sub>c \<times>\<^sub>f (mult_uncurried \<circ>\<^sub>c \<langle>right_cart_proj \<nat>\<^sub>c \<nat>\<^sub>c,left_cart_proj \<nat>\<^sub>c \<nat>\<^sub>c\<rangle>)\<^sup>\<sharp>)\<rangle>  \<circ>\<^sub>c \<langle>a,b\<rangle> "
+    proof -
+      have "left_cart_proj \<nat>\<^sub>c (\<nat>\<^sub>c\<^bsup>\<nat>\<^sub>c\<^esup>) \<circ>\<^sub>c id\<^sub>c \<nat>\<^sub>c \<times>\<^sub>f (mult_uncurried \<circ>\<^sub>c \<langle>right_cart_proj \<nat>\<^sub>c \<nat>\<^sub>c,left_cart_proj \<nat>\<^sub>c \<nat>\<^sub>c\<rangle>)\<^sup>\<sharp> = id\<^sub>c \<nat>\<^sub>c \<circ>\<^sub>c left_cart_proj \<nat>\<^sub>c \<nat>\<^sub>c"
+        by (simp add: id_type left_cart_proj_cfunc_cross_prod multp1p0sharp_type)
+      then show ?thesis
+        by presburger
+    qed
+    also have "... = add_uncurried \<circ>\<^sub>c
+ \<langle>id\<^sub>c \<nat>\<^sub>c \<circ>\<^sub>c left_cart_proj \<nat>\<^sub>c \<nat>\<^sub>c , 
+    mult_uncurried \<circ>\<^sub>c \<langle>right_cart_proj \<nat>\<^sub>c \<nat>\<^sub>c,left_cart_proj \<nat>\<^sub>c \<nat>\<^sub>c\<rangle>\<rangle>  \<circ>\<^sub>c \<langle>a,b\<rangle> "
+      using multp1p0_tye transpose_func_def by auto
+    also have "... =  add_uncurried \<circ>\<^sub>c
+ \<langle>id\<^sub>c \<nat>\<^sub>c \<circ>\<^sub>c left_cart_proj \<nat>\<^sub>c \<nat>\<^sub>c  \<circ>\<^sub>c \<langle>a,b\<rangle>, 
+    mult_uncurried \<circ>\<^sub>c \<langle>right_cart_proj \<nat>\<^sub>c \<nat>\<^sub>c,left_cart_proj \<nat>\<^sub>c \<nat>\<^sub>c\<rangle> \<circ>\<^sub>c \<langle>a,b\<rangle> \<rangle>  "
+      by (smt ab_typ cfunc_prod_comp comp_associative id_left_unit2 left_cart_proj_type multp1p0_tye)
+    also have "... =  add_uncurried \<circ>\<^sub>c\<langle>a,  mult_uncurried \<circ>\<^sub>c \<langle>right_cart_proj \<nat>\<^sub>c \<nat>\<^sub>c \<circ>\<^sub>c \<langle>a,b\<rangle>,left_cart_proj \<nat>\<^sub>c \<nat>\<^sub>c \<circ>\<^sub>c \<langle>a,b\<rangle>\<rangle>  \<rangle>  "
+      using ETCS_HOL.swap_def assms(1) assms(2) id_left_unit2 left_cart_proj_cfunc_prod right_cart_proj_cfunc_prod swap_ap by auto
+    also have "... =  add_uncurried \<circ>\<^sub>c\<langle>a,  mult_uncurried \<circ>\<^sub>c \<langle>b,a\<rangle>  \<rangle>  "
+      using assms(1) assms(2) left_cart_proj_cfunc_prod right_cart_proj_cfunc_prod by auto
+    also have "... = a +\<^sub>\<nat> (b \<cdot>\<^sub>\<nat> a)"
+      by (simp add: add_def mult_def)
+    also have "... = (successor \<circ>\<^sub>c a) \<cdot>\<^sub>\<nat> b"
+      oops (*need respects successor to the left, and for that we need "left" distributivity.*)
+ 
+*)   
+
+     
+      have f3: "(eval_func \<nat>\<^sub>c \<nat>\<^sub>c \<circ>\<^sub>c (id\<^sub>c \<nat>\<^sub>c \<times>\<^sub>f ((mult_uncurried \<circ>\<^sub>c \<langle>right_cart_proj \<nat>\<^sub>c \<nat>\<^sub>c,left_cart_proj \<nat>\<^sub>c \<nat>\<^sub>c\<rangle>)\<^sup>\<sharp>\<circ>\<^sub>c zero)))
+\<circ>\<^sub>c \<langle>a, id\<^sub>c one\<rangle> = zero"
+      proof - 
+        have "(eval_func \<nat>\<^sub>c \<nat>\<^sub>c \<circ>\<^sub>c (id\<^sub>c \<nat>\<^sub>c \<times>\<^sub>f ((mult_uncurried \<circ>\<^sub>c \<langle>right_cart_proj \<nat>\<^sub>c \<nat>\<^sub>c,left_cart_proj \<nat>\<^sub>c \<nat>\<^sub>c\<rangle>)\<^sup>\<sharp>\<circ>\<^sub>c zero)))
+\<circ>\<^sub>c \<langle>a, id\<^sub>c one\<rangle> = 
+    eval_func \<nat>\<^sub>c \<nat>\<^sub>c \<circ>\<^sub>c (id\<^sub>c \<nat>\<^sub>c \<times>\<^sub>f ((mult_uncurried \<circ>\<^sub>c \<langle>right_cart_proj \<nat>\<^sub>c \<nat>\<^sub>c,left_cart_proj \<nat>\<^sub>c \<nat>\<^sub>c\<rangle>)\<^sup>\<sharp>\<circ>\<^sub>c zero))
+    \<circ>\<^sub>c \<langle>a, id\<^sub>c one\<rangle>"
+          by (simp add: comp_associative)
+        also have "... =  eval_func \<nat>\<^sub>c \<nat>\<^sub>c \<circ>\<^sub>c (id\<^sub>c \<nat>\<^sub>c \<times>\<^sub>f ((mult_uncurried \<circ>\<^sub>c \<langle>right_cart_proj \<nat>\<^sub>c \<nat>\<^sub>c,left_cart_proj \<nat>\<^sub>c \<nat>\<^sub>c\<rangle>)\<^sup>\<sharp>))
+                                          \<circ>\<^sub>c  (id\<^sub>c \<nat>\<^sub>c \<times>\<^sub>f  zero) \<circ>\<^sub>c \<langle>a, id\<^sub>c one\<rangle>"
+          by (metis comp_associative inv_transpose_func_def2 inv_transpose_of_composition multp1p0sharp0_type multp1p0sharp_type zero_type)
+        also have "... = (mult_uncurried \<circ>\<^sub>c \<langle>right_cart_proj \<nat>\<^sub>c \<nat>\<^sub>c,left_cart_proj \<nat>\<^sub>c \<nat>\<^sub>c\<rangle>) \<circ>\<^sub>c  (id\<^sub>c \<nat>\<^sub>c \<times>\<^sub>f  zero) \<circ>\<^sub>c \<langle>a, id\<^sub>c one\<rangle>"
+          using comp_associative flat_cancels_sharp inv_transpose_func_def2 multp1p0_tye multp1p0sharp_type by fastforce
+        also have "... = mult_uncurried \<circ>\<^sub>c \<langle>right_cart_proj \<nat>\<^sub>c \<nat>\<^sub>c,left_cart_proj \<nat>\<^sub>c \<nat>\<^sub>c\<rangle> \<circ>\<^sub>c  (id\<^sub>c \<nat>\<^sub>c \<times>\<^sub>f  zero) \<circ>\<^sub>c \<langle>a, id\<^sub>c one\<rangle>"
+          by (simp add: comp_associative)
+        also have "... = mult_uncurried \<circ>\<^sub>c \<langle>right_cart_proj \<nat>\<^sub>c \<nat>\<^sub>c,left_cart_proj \<nat>\<^sub>c \<nat>\<^sub>c\<rangle>  \<circ>\<^sub>c \<langle>id\<^sub>c \<nat>\<^sub>c \<circ>\<^sub>c a, zero \<circ>\<^sub>c id\<^sub>c one\<rangle>"
+          using ETCS_HOL.swap_def assms(1) calculation f1 id_left_unit2 id_right_unit2 mult_def mult_respects_zero_left swap_ap zero_type by auto
+        also have "... =  mult_uncurried \<circ>\<^sub>c \<langle>right_cart_proj \<nat>\<^sub>c \<nat>\<^sub>c \<circ>\<^sub>c \<langle>a, zero\<rangle> ,left_cart_proj \<nat>\<^sub>c \<nat>\<^sub>c  \<circ>\<^sub>c \<langle>a, zero\<rangle> \<rangle>  "
+          using assms(1) calculation f1 left_cart_proj_cfunc_prod mult_def mult_respects_zero_left right_cart_proj_cfunc_prod zero_type by auto
+        also have "... =  mult_uncurried \<circ>\<^sub>c \<langle>zero ,a \<rangle>"
+          using assms(1) left_cart_proj_cfunc_prod right_cart_proj_cfunc_prod zero_type by auto
+        also have "... = zero"
+          using calculation f1 by auto
+then show ?thesis using calculation by auto
+qed
+
+  oops
+
+         
+(*
+
+lemma mult_associative:
+  assumes "a \<in>\<^sub>c  \<nat>\<^sub>c"  "b\<in>\<^sub>c  \<nat>\<^sub>c"  "c\<in>\<^sub>c  \<nat>\<^sub>c"
+  shows "a \<cdot>\<^sub>\<nat> ( b \<cdot>\<^sub>\<nat> c)   = (a \<cdot>\<^sub>\<nat> b) \<cdot>\<^sub>\<nat> c"
+proof -
+  have ab_type: "\<langle>a,b\<rangle> : one \<rightarrow>(\<nat>\<^sub>c\<times>\<^sub>c\<nat>\<^sub>c)"
+    by (simp add: assms(1) assms(2) cfunc_prod_type)
+  have id_ab_type: "id\<^sub>c (\<nat>\<^sub>c\<times>\<^sub>c\<nat>\<^sub>c)\<circ>\<^sub>c  \<langle>a,b\<rangle>: one \<rightarrow>(\<nat>\<^sub>c\<times>\<^sub>c\<nat>\<^sub>c)"
+    using ab_type id_left_unit2 by auto
+  have b0_type: "\<langle>b,zero\<rangle> : one \<rightarrow>(\<nat>\<^sub>c\<times>\<^sub>c\<nat>\<^sub>c)"
+    using assms(2) cfunc_prod_type zero_type by blast
+  have abc_type: "\<langle>\<langle>a,b\<rangle>,c\<rangle>:  one \<rightarrow>(\<nat>\<^sub>c\<times>\<^sub>c\<nat>\<^sub>c)\<times>\<^sub>c\<nat>\<^sub>c"
+    by (simp add: ab_type assms(3) cfunc_prod_type)
+  have sc_type: "successor \<circ>\<^sub>c c : one \<rightarrow> \<nat>\<^sub>c"
+    using assms(3) successor_type by auto
+  have abz_type: "\<langle>\<langle>a,b\<rangle>,zero\<rangle>:  one \<rightarrow>(\<nat>\<^sub>c\<times>\<^sub>c\<nat>\<^sub>c)\<times>\<^sub>c\<nat>\<^sub>c"
+    by (simp add: ab_type cfunc_prod_type zero_type)
+  have abId_type: "\<langle>\<langle>a,b\<rangle>,id one\<rangle>:  one \<rightarrow>(\<nat>\<^sub>c\<times>\<^sub>c\<nat>\<^sub>c)\<times>\<^sub>c one"
+    by (simp add: ab_type cfunc_prod_type id_type)
+  have abSc_type: "\<langle>\<langle>a,b\<rangle>,successor  \<circ>\<^sub>c c\<rangle>: one \<rightarrow>(\<nat>\<^sub>c\<times>\<^sub>c\<nat>\<^sub>c)\<times>\<^sub>c \<nat>\<^sub>c"
+    by (simp add: ab_type cfunc_prod_type sc_type)
+  have bSc_type: "\<langle>b,successor  \<circ>\<^sub>c c\<rangle>: one \<rightarrow> (\<nat>\<^sub>c\<times>\<^sub>c\<nat>\<^sub>c)"
+    by (simp add: assms(2) cfunc_prod_type sc_type)
+  have multId_type: "mult_uncurried \<times>\<^sub>f id\<^sub>c \<nat>\<^sub>c : (\<nat>\<^sub>c\<times>\<^sub>c \<nat>\<^sub>c)\<times>\<^sub>c \<nat>\<^sub>c\<rightarrow> (\<nat>\<^sub>c\<times>\<^sub>c \<nat>\<^sub>c)"
+    by (simp add: cfunc_cross_prod_type id_type mult_uncurried_type)
+  have multab_type: "mult_uncurried \<circ>\<^sub>c \<langle>a,b\<rangle>: one \<rightarrow> \<nat>\<^sub>c"
+    using ab_type comp_type mult_uncurried_type by blast
+  have multmultId_type: "mult_uncurried \<circ>\<^sub>c (mult_uncurried \<times>\<^sub>f id\<^sub>c \<nat>\<^sub>c) : (\<nat>\<^sub>c\<times>\<^sub>c \<nat>\<^sub>c)\<times>\<^sub>c \<nat>\<^sub>c\<rightarrow> \<nat>\<^sub>c"
+    using comp_type multId_type mult_uncurried_type by blast
+  have multIdmult_type: "(mult_uncurried \<circ>\<^sub>c (id\<^sub>c \<nat>\<^sub>c  \<times>\<^sub>f mult_uncurried)): \<nat>\<^sub>c\<times>\<^sub>c( \<nat>\<^sub>c\<times>\<^sub>c \<nat>\<^sub>c)\<rightarrow> \<nat>\<^sub>c"
+    by (smt comp_type flat_type inv_transpose_func_def2 inv_transpose_of_composition mult_curried_type mult_uncurried_def)
+  have multmultIdSharp_type: "(mult_uncurried \<circ>\<^sub>c (mult_uncurried \<times>\<^sub>f id\<^sub>c \<nat>\<^sub>c))\<^sup>\<sharp> :  \<nat>\<^sub>c\<rightarrow> \<nat>\<^sub>c\<^bsup>(\<nat>\<^sub>c\<times>\<^sub>c \<nat>\<^sub>c)\<^esup>"
+    by (simp add: multmultId_type transpose_func_def)
+  have mmIdSharp0_type: "(mult_uncurried \<circ>\<^sub>c (mult_uncurried \<times>\<^sub>f id\<^sub>c \<nat>\<^sub>c))\<^sup>\<sharp>\<circ>\<^sub>c zero : one \<rightarrow> \<nat>\<^sub>c\<^bsup>(\<nat>\<^sub>c\<times>\<^sub>c \<nat>\<^sub>c)\<^esup>"
+    using comp_type multmultIdSharp_type zero_type by blast
+  have mmIdSharpS_type: "(mult_uncurried \<circ>\<^sub>c (mult_uncurried \<times>\<^sub>f id\<^sub>c \<nat>\<^sub>c))\<^sup>\<sharp>\<circ>\<^sub>c successor : \<nat>\<^sub>c \<rightarrow> \<nat>\<^sub>c\<^bsup>(\<nat>\<^sub>c\<times>\<^sub>c \<nat>\<^sub>c)\<^esup>"
+    using multmultIdSharp_type successor_type by auto
+  have p0rho0_type: "(left_cart_proj \<nat>\<^sub>c \<nat>\<^sub>c) \<circ>\<^sub>c (left_cart_proj (\<nat>\<^sub>c\<times>\<^sub>c \<nat>\<^sub>c) \<nat>\<^sub>c) : (\<nat>\<^sub>c\<times>\<^sub>c \<nat>\<^sub>c)\<times>\<^sub>c \<nat>\<^sub>c\<rightarrow> \<nat>\<^sub>c"
+    using comp_type left_cart_proj_type by blast
+  have p1rho0_type: "(right_cart_proj \<nat>\<^sub>c \<nat>\<^sub>c) \<circ>\<^sub>c (left_cart_proj (\<nat>\<^sub>c\<times>\<^sub>c \<nat>\<^sub>c) \<nat>\<^sub>c) : (\<nat>\<^sub>c\<times>\<^sub>c \<nat>\<^sub>c)\<times>\<^sub>c \<nat>\<^sub>c\<rightarrow> \<nat>\<^sub>c"
+    using comp_type left_cart_proj_type right_cart_proj_type by blast
+  have p1rho0rho1_type: "\<langle>(right_cart_proj \<nat>\<^sub>c \<nat>\<^sub>c) \<circ>\<^sub>c (left_cart_proj (\<nat>\<^sub>c\<times>\<^sub>c \<nat>\<^sub>c) \<nat>\<^sub>c), (right_cart_proj (\<nat>\<^sub>c\<times>\<^sub>c \<nat>\<^sub>c) \<nat>\<^sub>c)\<rangle> :  (\<nat>\<^sub>c\<times>\<^sub>c \<nat>\<^sub>c)\<times>\<^sub>c \<nat>\<^sub>c \<rightarrow>  (\<nat>\<^sub>c\<times>\<^sub>c \<nat>\<^sub>c)"
+    by (simp add: cfunc_prod_type p1rho0_type right_cart_proj_type)
+  have p0p0p1p0p1_type: "\<langle>(left_cart_proj \<nat>\<^sub>c \<nat>\<^sub>c) \<circ>\<^sub>c (left_cart_proj (\<nat>\<^sub>c\<times>\<^sub>c \<nat>\<^sub>c) \<nat>\<^sub>c),
+\<langle>(right_cart_proj \<nat>\<^sub>c \<nat>\<^sub>c) \<circ>\<^sub>c (left_cart_proj (\<nat>\<^sub>c\<times>\<^sub>c \<nat>\<^sub>c) \<nat>\<^sub>c), (right_cart_proj (\<nat>\<^sub>c\<times>\<^sub>c \<nat>\<^sub>c) \<nat>\<^sub>c)\<rangle>\<rangle>: (\<nat>\<^sub>c\<times>\<^sub>c \<nat>\<^sub>c)\<times>\<^sub>c \<nat>\<^sub>c \<rightarrow>   \<nat>\<^sub>c \<times>\<^sub>c(\<nat>\<^sub>c\<times>\<^sub>c \<nat>\<^sub>c)"
+    by (simp add: cfunc_prod_type p0rho0_type p1rho0rho1_type)
+  have multIdxMultp0p0p1p0p1_type: "mult_uncurried \<circ>\<^sub>c (id\<^sub>c \<nat>\<^sub>c  \<times>\<^sub>f mult_uncurried) \<circ>\<^sub>c \<langle>(left_cart_proj \<nat>\<^sub>c \<nat>\<^sub>c) \<circ>\<^sub>c (left_cart_proj (\<nat>\<^sub>c\<times>\<^sub>c \<nat>\<^sub>c) \<nat>\<^sub>c),
+\<langle>(right_cart_proj \<nat>\<^sub>c \<nat>\<^sub>c) \<circ>\<^sub>c (left_cart_proj (\<nat>\<^sub>c\<times>\<^sub>c \<nat>\<^sub>c) \<nat>\<^sub>c), (right_cart_proj (\<nat>\<^sub>c\<times>\<^sub>c \<nat>\<^sub>c) \<nat>\<^sub>c)\<rangle>\<rangle> : (\<nat>\<^sub>c\<times>\<^sub>c \<nat>\<^sub>c)\<times>\<^sub>c \<nat>\<^sub>c \<rightarrow>\<nat>\<^sub>c"
+    using comp_associative multIdmult_type p0p0p1p0p1_type by auto
+  have multIdxMultp0p0p1p0p1_Sharp_type: "(mult_uncurried \<circ>\<^sub>c (id\<^sub>c \<nat>\<^sub>c  \<times>\<^sub>f mult_uncurried) \<circ>\<^sub>c \<langle>(left_cart_proj \<nat>\<^sub>c \<nat>\<^sub>c) \<circ>\<^sub>c (left_cart_proj (\<nat>\<^sub>c\<times>\<^sub>c \<nat>\<^sub>c) \<nat>\<^sub>c),
+\<langle>(right_cart_proj \<nat>\<^sub>c \<nat>\<^sub>c) \<circ>\<^sub>c (left_cart_proj (\<nat>\<^sub>c\<times>\<^sub>c \<nat>\<^sub>c) \<nat>\<^sub>c), (right_cart_proj (\<nat>\<^sub>c\<times>\<^sub>c \<nat>\<^sub>c) \<nat>\<^sub>c)\<rangle>\<rangle>)\<^sup>\<sharp>: \<nat>\<^sub>c\<rightarrow> \<nat>\<^sub>c\<^bsup>(\<nat>\<^sub>c\<times>\<^sub>c\<nat>\<^sub>c)\<^esup>"
+    using multIdxMultp0p0p1p0p1_type transpose_func_def by blast
+  then have multIdxMultp0p0p1p0p0_Sharp0_type: "(mult_uncurried \<circ>\<^sub>c (id\<^sub>c \<nat>\<^sub>c  \<times>\<^sub>f mult_uncurried) \<circ>\<^sub>c \<langle>(left_cart_proj \<nat>\<^sub>c \<nat>\<^sub>c) \<circ>\<^sub>c (left_cart_proj (\<nat>\<^sub>c\<times>\<^sub>c \<nat>\<^sub>c) \<nat>\<^sub>c),
+\<langle>(right_cart_proj \<nat>\<^sub>c \<nat>\<^sub>c) \<circ>\<^sub>c (left_cart_proj (\<nat>\<^sub>c\<times>\<^sub>c \<nat>\<^sub>c) \<nat>\<^sub>c), (right_cart_proj (\<nat>\<^sub>c\<times>\<^sub>c \<nat>\<^sub>c) \<nat>\<^sub>c)\<rangle>\<rangle>)\<^sup>\<sharp> \<circ>\<^sub>c zero :  one \<rightarrow> \<nat>\<^sub>c\<^bsup>(\<nat>\<^sub>c\<times>\<^sub>c\<nat>\<^sub>c)\<^esup>"
+    using comp_type zero_type by blast
+  have multIdxMultp0p0p1p0p0_SharpSucc_type: "(mult_uncurried \<circ>\<^sub>c (id\<^sub>c \<nat>\<^sub>c  \<times>\<^sub>f mult_uncurried) \<circ>\<^sub>c \<langle>(left_cart_proj \<nat>\<^sub>c \<nat>\<^sub>c) \<circ>\<^sub>c (left_cart_proj (\<nat>\<^sub>c\<times>\<^sub>c \<nat>\<^sub>c) \<nat>\<^sub>c),
+\<langle>(right_cart_proj \<nat>\<^sub>c \<nat>\<^sub>c) \<circ>\<^sub>c (left_cart_proj (\<nat>\<^sub>c\<times>\<^sub>c \<nat>\<^sub>c) \<nat>\<^sub>c), (right_cart_proj (\<nat>\<^sub>c\<times>\<^sub>c \<nat>\<^sub>c) \<nat>\<^sub>c)\<rangle>\<rangle>)\<^sup>\<sharp> \<circ>\<^sub>c successor :  \<nat>\<^sub>c \<rightarrow> \<nat>\<^sub>c\<^bsup>(\<nat>\<^sub>c\<times>\<^sub>c\<nat>\<^sub>c)\<^esup>"
+    using comp_type multIdxMultp0p0p1p0p1_Sharp_type successor_type by blast
+  have zbsharp_type: "(zero \<circ>\<^sub>c \<beta>\<^bsub>(\<nat>\<^sub>c\<times>\<^sub>c \<nat>\<^sub>c)\<times>\<^sub>cone\<^esub>)\<^sup>\<sharp>: one \<rightarrow> \<nat>\<^sub>c\<^bsup>(\<nat>\<^sub>c\<times>\<^sub>c\<nat>\<^sub>c)\<^esup>"
+    by (simp add: transpose_func_def zero_betaN_type)
+  have multsigma0_type: "mult_uncurried \<circ>\<^sub>c (left_cart_proj (\<nat>\<^sub>c\<times>\<^sub>c\<nat>\<^sub>c) (\<nat>\<^sub>c\<^bsup>(\<nat>\<^sub>c\<times>\<^sub>c\<nat>\<^sub>c)\<^esup>)):  ((\<nat>\<^sub>c\<times>\<^sub>c \<nat>\<^sub>c)\<times>\<^sub>c(\<nat>\<^sub>c\<^bsup>(\<nat>\<^sub>c\<times>\<^sub>c\<nat>\<^sub>c)\<^esup>))\<rightarrow> \<nat>\<^sub>c"
+    using comp_type left_cart_proj_type mult_uncurried_type by blast
+  have multsigma0Eval_type: "\<langle>mult_uncurried \<circ>\<^sub>c (left_cart_proj (\<nat>\<^sub>c\<times>\<^sub>c\<nat>\<^sub>c) (\<nat>\<^sub>c\<^bsup>(\<nat>\<^sub>c\<times>\<^sub>c\<nat>\<^sub>c)\<^esup>)),eval_func \<nat>\<^sub>c (\<nat>\<^sub>c\<times>\<^sub>c\<nat>\<^sub>c)\<rangle> : ((\<nat>\<^sub>c\<times>\<^sub>c \<nat>\<^sub>c)\<times>\<^sub>c(\<nat>\<^sub>c\<^bsup>(\<nat>\<^sub>c\<times>\<^sub>c\<nat>\<^sub>c)\<^esup>))\<rightarrow> (\<nat>\<^sub>c\<times>\<^sub>c\<nat>\<^sub>c)"
+    by (simp add: cfunc_prod_type eval_func_type multsigma0_type)
+  then have addMultSigma0Eval_type: "add_uncurried \<circ>\<^sub>c \<langle>mult_uncurried \<circ>\<^sub>c (left_cart_proj (\<nat>\<^sub>c\<times>\<^sub>c\<nat>\<^sub>c) (\<nat>\<^sub>c\<^bsup>(\<nat>\<^sub>c\<times>\<^sub>c\<nat>\<^sub>c)\<^esup>)),eval_func \<nat>\<^sub>c (\<nat>\<^sub>c\<times>\<^sub>c\<nat>\<^sub>c)\<rangle> : ((\<nat>\<^sub>c\<times>\<^sub>c \<nat>\<^sub>c)\<times>\<^sub>c(\<nat>\<^sub>c\<^bsup>(\<nat>\<^sub>c\<times>\<^sub>c\<nat>\<^sub>c)\<^esup>))\<rightarrow> \<nat>\<^sub>c"
+    using add_uncurried_type comp_type by blast
+  then have addMultSigma0EvalSharp_type: "(add_uncurried \<circ>\<^sub>c \<langle>mult_uncurried \<circ>\<^sub>c (left_cart_proj (\<nat>\<^sub>c\<times>\<^sub>c\<nat>\<^sub>c) (\<nat>\<^sub>c\<^bsup>(\<nat>\<^sub>c\<times>\<^sub>c\<nat>\<^sub>c)\<^esup>)),eval_func \<nat>\<^sub>c (\<nat>\<^sub>c\<times>\<^sub>c\<nat>\<^sub>c)\<rangle>)\<^sup>\<sharp> : (\<nat>\<^sub>c\<^bsup>(\<nat>\<^sub>c\<times>\<^sub>c\<nat>\<^sub>c)\<^esup>)\<rightarrow> (\<nat>\<^sub>c\<^bsup>(\<nat>\<^sub>c\<times>\<^sub>c\<nat>\<^sub>c)\<^esup>)"
+    by (simp add: transpose_func_def)
+  have id_multmultidsharp_type: "(id\<^sub>c (\<nat>\<^sub>c\<times>\<^sub>c\<nat>\<^sub>c) \<times>\<^sub>f ((mult_uncurried \<circ>\<^sub>c (mult_uncurried \<times>\<^sub>f id\<^sub>c \<nat>\<^sub>c))\<^sup>\<sharp>)): (\<nat>\<^sub>c\<times>\<^sub>c\<nat>\<^sub>c) \<times>\<^sub>c \<nat>\<^sub>c \<rightarrow> (\<nat>\<^sub>c\<times>\<^sub>c\<nat>\<^sub>c) \<times>\<^sub>c \<nat>\<^sub>c\<^bsup>(\<nat>\<^sub>c\<times>\<^sub>c \<nat>\<^sub>c)\<^esup>"
+    by (meson cfunc_cross_prod_type id_type multmultIdSharp_type)
+  have f1: "((eval_func \<nat>\<^sub>c (\<nat>\<^sub>c\<times>\<^sub>c\<nat>\<^sub>c))\<circ>\<^sub>c 
+(id\<^sub>c (\<nat>\<^sub>c\<times>\<^sub>c\<nat>\<^sub>c) \<times>\<^sub>f ((mult_uncurried \<circ>\<^sub>c (mult_uncurried \<times>\<^sub>f id\<^sub>c \<nat>\<^sub>c))\<^sup>\<sharp>\<circ>\<^sub>c zero)))\<circ>\<^sub>c \<langle>\<langle>a,b\<rangle>,id\<^sub>c one\<rangle> = zero" 
+  proof - 
+    have "((eval_func \<nat>\<^sub>c (\<nat>\<^sub>c\<times>\<^sub>c\<nat>\<^sub>c))\<circ>\<^sub>c 
+(id\<^sub>c (\<nat>\<^sub>c\<times>\<^sub>c\<nat>\<^sub>c) \<times>\<^sub>f ((mult_uncurried \<circ>\<^sub>c (mult_uncurried \<times>\<^sub>f id\<^sub>c \<nat>\<^sub>c))\<^sup>\<sharp>\<circ>\<^sub>c zero)))\<circ>\<^sub>c \<langle>\<langle>a,b\<rangle>,id\<^sub>c one\<rangle> = 
+(eval_func \<nat>\<^sub>c (\<nat>\<^sub>c\<times>\<^sub>c\<nat>\<^sub>c))\<circ>\<^sub>c 
+(id\<^sub>c (\<nat>\<^sub>c\<times>\<^sub>c\<nat>\<^sub>c) \<times>\<^sub>f ((mult_uncurried \<circ>\<^sub>c (mult_uncurried \<times>\<^sub>f id\<^sub>c \<nat>\<^sub>c))\<^sup>\<sharp>\<circ>\<^sub>c zero))\<circ>\<^sub>c \<langle>\<langle>a,b\<rangle>,id\<^sub>c one\<rangle>"
+      by (simp add: comp_associative)
+    also have "... = (eval_func \<nat>\<^sub>c (\<nat>\<^sub>c\<times>\<^sub>c\<nat>\<^sub>c))\<circ>\<^sub>c 
+(id\<^sub>c (\<nat>\<^sub>c\<times>\<^sub>c\<nat>\<^sub>c) \<times>\<^sub>f ((mult_uncurried \<circ>\<^sub>c (mult_uncurried \<times>\<^sub>f id\<^sub>c \<nat>\<^sub>c))\<^sup>\<sharp>))\<circ>\<^sub>c ((id\<^sub>c (\<nat>\<^sub>c\<times>\<^sub>c\<nat>\<^sub>c) \<times>\<^sub>f zero)) \<circ>\<^sub>c \<langle>\<langle>a,b\<rangle>,id\<^sub>c one\<rangle>"
+      using comp_associative identity_distributes_across_composition multmultIdSharp_type zero_type by auto
+    also have "... = (mult_uncurried \<circ>\<^sub>c (mult_uncurried \<times>\<^sub>f id\<^sub>c \<nat>\<^sub>c)) \<circ>\<^sub>c   \<langle> id\<^sub>c (\<nat>\<^sub>c\<times>\<^sub>c\<nat>\<^sub>c) \<circ>\<^sub>c \<langle>a,b\<rangle>, zero \<circ>\<^sub>c id\<^sub>c one\<rangle>"
+      by (smt ab_type cfunc_cross_prod_comp_cfunc_prod comp_associative flat_cancels_sharp id_type inv_transpose_func_def2 multmultIdSharp_type multmultId_type zero_type)
+    also have "... = mult_uncurried \<circ>\<^sub>c (mult_uncurried \<times>\<^sub>f id\<^sub>c \<nat>\<^sub>c)  \<circ>\<^sub>c   \<langle>\<langle>a,b\<rangle>, zero\<rangle>"
+      using ab_type comp_associative id_left_unit2 id_right_unit2 zero_type by auto
+    also have "... = mult_uncurried \<circ>\<^sub>c \<langle>mult_uncurried \<circ>\<^sub>c \<langle>a,b\<rangle>, zero\<rangle> "
+      using ab_type cfunc_cross_prod_comp_cfunc_prod id_left_unit2 id_type mult_uncurried_type zero_type by fastforce
+    also have "... = zero"
+      using mult_def mult_respects_zero_right multab_type by auto
+then show ?thesis using calculation by auto
+qed
+
+
+  have f2: "((eval_func \<nat>\<^sub>c (\<nat>\<^sub>c\<times>\<^sub>c\<nat>\<^sub>c))\<circ>\<^sub>c 
+(id\<^sub>c (\<nat>\<^sub>c\<times>\<^sub>c\<nat>\<^sub>c) \<times>\<^sub>f ((mult_uncurried \<circ>\<^sub>c (id\<^sub>c \<nat>\<^sub>c  \<times>\<^sub>f mult_uncurried) \<circ>\<^sub>c \<langle>(left_cart_proj \<nat>\<^sub>c \<nat>\<^sub>c) \<circ>\<^sub>c (left_cart_proj (\<nat>\<^sub>c\<times>\<^sub>c \<nat>\<^sub>c) \<nat>\<^sub>c),
+\<langle>(right_cart_proj \<nat>\<^sub>c \<nat>\<^sub>c) \<circ>\<^sub>c (left_cart_proj (\<nat>\<^sub>c\<times>\<^sub>c \<nat>\<^sub>c) \<nat>\<^sub>c), (right_cart_proj (\<nat>\<^sub>c\<times>\<^sub>c \<nat>\<^sub>c) \<nat>\<^sub>c)\<rangle>\<rangle>)\<^sup>\<sharp> \<circ>\<^sub>c zero))) \<circ>\<^sub>c \<langle>\<langle>a,b\<rangle>,id\<^sub>c one\<rangle> = zero" 
+  proof - 
+    have "((eval_func \<nat>\<^sub>c (\<nat>\<^sub>c\<times>\<^sub>c\<nat>\<^sub>c))\<circ>\<^sub>c 
+(id\<^sub>c (\<nat>\<^sub>c\<times>\<^sub>c\<nat>\<^sub>c) \<times>\<^sub>f ((mult_uncurried \<circ>\<^sub>c (id\<^sub>c \<nat>\<^sub>c  \<times>\<^sub>f mult_uncurried) \<circ>\<^sub>c \<langle>(left_cart_proj \<nat>\<^sub>c \<nat>\<^sub>c) \<circ>\<^sub>c (left_cart_proj (\<nat>\<^sub>c\<times>\<^sub>c \<nat>\<^sub>c) \<nat>\<^sub>c),
+\<langle>(right_cart_proj \<nat>\<^sub>c \<nat>\<^sub>c) \<circ>\<^sub>c (left_cart_proj (\<nat>\<^sub>c\<times>\<^sub>c \<nat>\<^sub>c) \<nat>\<^sub>c), (right_cart_proj (\<nat>\<^sub>c\<times>\<^sub>c \<nat>\<^sub>c) \<nat>\<^sub>c)\<rangle>\<rangle>)\<^sup>\<sharp> \<circ>\<^sub>c zero))) \<circ>\<^sub>c \<langle>\<langle>a,b\<rangle>,id\<^sub>c one\<rangle> = 
+   (eval_func \<nat>\<^sub>c (\<nat>\<^sub>c\<times>\<^sub>c\<nat>\<^sub>c))\<circ>\<^sub>c 
+(id\<^sub>c (\<nat>\<^sub>c\<times>\<^sub>c\<nat>\<^sub>c) \<times>\<^sub>f ((mult_uncurried \<circ>\<^sub>c (id\<^sub>c \<nat>\<^sub>c  \<times>\<^sub>f mult_uncurried) \<circ>\<^sub>c \<langle>(left_cart_proj \<nat>\<^sub>c \<nat>\<^sub>c) \<circ>\<^sub>c (left_cart_proj (\<nat>\<^sub>c\<times>\<^sub>c \<nat>\<^sub>c) \<nat>\<^sub>c),
+\<langle>(right_cart_proj \<nat>\<^sub>c \<nat>\<^sub>c) \<circ>\<^sub>c (left_cart_proj (\<nat>\<^sub>c\<times>\<^sub>c \<nat>\<^sub>c) \<nat>\<^sub>c), (right_cart_proj (\<nat>\<^sub>c\<times>\<^sub>c \<nat>\<^sub>c) \<nat>\<^sub>c)\<rangle>\<rangle>)\<^sup>\<sharp> \<circ>\<^sub>c zero)) \<circ>\<^sub>c \<langle>\<langle>a,b\<rangle>,id\<^sub>c one\<rangle>"
+      by (simp add: comp_associative)
+    also have "... = (eval_func \<nat>\<^sub>c (\<nat>\<^sub>c\<times>\<^sub>c\<nat>\<^sub>c))\<circ>\<^sub>c 
+(id\<^sub>c (\<nat>\<^sub>c\<times>\<^sub>c\<nat>\<^sub>c) \<times>\<^sub>f ((mult_uncurried \<circ>\<^sub>c (id\<^sub>c \<nat>\<^sub>c  \<times>\<^sub>f mult_uncurried) \<circ>\<^sub>c \<langle>(left_cart_proj \<nat>\<^sub>c \<nat>\<^sub>c) \<circ>\<^sub>c (left_cart_proj (\<nat>\<^sub>c\<times>\<^sub>c \<nat>\<^sub>c) \<nat>\<^sub>c),
+\<langle>(right_cart_proj \<nat>\<^sub>c \<nat>\<^sub>c) \<circ>\<^sub>c (left_cart_proj (\<nat>\<^sub>c\<times>\<^sub>c \<nat>\<^sub>c) \<nat>\<^sub>c), (right_cart_proj (\<nat>\<^sub>c\<times>\<^sub>c \<nat>\<^sub>c) \<nat>\<^sub>c)\<rangle>\<rangle>)\<^sup>\<sharp> )) \<circ>\<^sub>c (id\<^sub>c (\<nat>\<^sub>c\<times>\<^sub>c\<nat>\<^sub>c) \<times>\<^sub>f zero)  \<circ>\<^sub>c \<langle>\<langle>a,b\<rangle>,id\<^sub>c one\<rangle>"
+      using comp_associative identity_distributes_across_composition multIdxMultp0p0p1p0p1_Sharp_type zero_type by auto
+    also have "... = (mult_uncurried \<circ>\<^sub>c (id\<^sub>c \<nat>\<^sub>c  \<times>\<^sub>f mult_uncurried) \<circ>\<^sub>c \<langle>(left_cart_proj \<nat>\<^sub>c \<nat>\<^sub>c) \<circ>\<^sub>c (left_cart_proj (\<nat>\<^sub>c\<times>\<^sub>c \<nat>\<^sub>c) \<nat>\<^sub>c),
+\<langle>(right_cart_proj \<nat>\<^sub>c \<nat>\<^sub>c) \<circ>\<^sub>c (left_cart_proj (\<nat>\<^sub>c\<times>\<^sub>c \<nat>\<^sub>c) \<nat>\<^sub>c), (right_cart_proj (\<nat>\<^sub>c\<times>\<^sub>c \<nat>\<^sub>c) \<nat>\<^sub>c)\<rangle>\<rangle>)\<circ>\<^sub>c (id\<^sub>c (\<nat>\<^sub>c\<times>\<^sub>c\<nat>\<^sub>c) \<times>\<^sub>f zero)  \<circ>\<^sub>c \<langle>\<langle>a,b\<rangle>,id\<^sub>c one\<rangle>"
+      using comp_associative multIdxMultp0p0p1p0p1_type transpose_func_def by presburger
+    also have "... = mult_uncurried \<circ>\<^sub>c (id\<^sub>c \<nat>\<^sub>c  \<times>\<^sub>f mult_uncurried) \<circ>\<^sub>c \<langle>(left_cart_proj \<nat>\<^sub>c \<nat>\<^sub>c) \<circ>\<^sub>c (left_cart_proj (\<nat>\<^sub>c\<times>\<^sub>c \<nat>\<^sub>c) \<nat>\<^sub>c),
+\<langle>(right_cart_proj \<nat>\<^sub>c \<nat>\<^sub>c) \<circ>\<^sub>c (left_cart_proj (\<nat>\<^sub>c\<times>\<^sub>c \<nat>\<^sub>c) \<nat>\<^sub>c), (right_cart_proj (\<nat>\<^sub>c\<times>\<^sub>c \<nat>\<^sub>c) \<nat>\<^sub>c)\<rangle>\<rangle>\<circ>\<^sub>c \<langle>id\<^sub>c (\<nat>\<^sub>c\<times>\<^sub>c\<nat>\<^sub>c) \<circ>\<^sub>c \<langle>a,b\<rangle>,zero \<circ>\<^sub>cid\<^sub>c one\<rangle>"
+      by (smt ab_type cfunc_cross_prod_comp_cfunc_prod comp_associative id_type zero_type)
+    also have "... = mult_uncurried \<circ>\<^sub>c (id\<^sub>c \<nat>\<^sub>c  \<times>\<^sub>f mult_uncurried) \<circ>\<^sub>c \<langle>(left_cart_proj \<nat>\<^sub>c \<nat>\<^sub>c) \<circ>\<^sub>c (left_cart_proj (\<nat>\<^sub>c\<times>\<^sub>c \<nat>\<^sub>c) \<nat>\<^sub>c),
+\<langle>(right_cart_proj \<nat>\<^sub>c \<nat>\<^sub>c) \<circ>\<^sub>c (left_cart_proj (\<nat>\<^sub>c\<times>\<^sub>c \<nat>\<^sub>c) \<nat>\<^sub>c), (right_cart_proj (\<nat>\<^sub>c\<times>\<^sub>c \<nat>\<^sub>c) \<nat>\<^sub>c)\<rangle>\<rangle>\<circ>\<^sub>c \<langle>\<langle>a,b\<rangle>,zero\<rangle>"
+      using ab_type id_left_unit2 id_right_unit2 zero_type by auto
+    also have "... = mult_uncurried \<circ>\<^sub>c (id\<^sub>c \<nat>\<^sub>c  \<times>\<^sub>f mult_uncurried) \<circ>\<^sub>c \<langle>(left_cart_proj \<nat>\<^sub>c \<nat>\<^sub>c) \<circ>\<^sub>c (left_cart_proj (\<nat>\<^sub>c\<times>\<^sub>c \<nat>\<^sub>c) \<nat>\<^sub>c) \<circ>\<^sub>c \<langle>\<langle>a,b\<rangle>,zero\<rangle>,
+\<langle>(right_cart_proj \<nat>\<^sub>c \<nat>\<^sub>c) \<circ>\<^sub>c (left_cart_proj (\<nat>\<^sub>c\<times>\<^sub>c \<nat>\<^sub>c) \<nat>\<^sub>c), (right_cart_proj (\<nat>\<^sub>c\<times>\<^sub>c \<nat>\<^sub>c) \<nat>\<^sub>c)\<rangle> \<circ>\<^sub>c \<langle>\<langle>a,b\<rangle>,zero\<rangle>  \<rangle>"
+      using abz_type cfunc_prod_comp comp_associative p0rho0_type p1rho0rho1_type by auto
+   also have "... = mult_uncurried \<circ>\<^sub>c (id\<^sub>c \<nat>\<^sub>c  \<times>\<^sub>f mult_uncurried) \<circ>\<^sub>c \<langle>(left_cart_proj \<nat>\<^sub>c \<nat>\<^sub>c) \<circ>\<^sub>c (left_cart_proj (\<nat>\<^sub>c\<times>\<^sub>c \<nat>\<^sub>c) \<nat>\<^sub>c) \<circ>\<^sub>c \<langle>\<langle>a,b\<rangle>,zero\<rangle>,
+\<langle>(right_cart_proj \<nat>\<^sub>c \<nat>\<^sub>c) \<circ>\<^sub>c (left_cart_proj (\<nat>\<^sub>c\<times>\<^sub>c \<nat>\<^sub>c) \<nat>\<^sub>c) \<circ>\<^sub>c \<langle>\<langle>a,b\<rangle>,zero\<rangle>  , (right_cart_proj (\<nat>\<^sub>c\<times>\<^sub>c \<nat>\<^sub>c) \<nat>\<^sub>c) \<circ>\<^sub>c \<langle>\<langle>a,b\<rangle>,zero\<rangle>  \<rangle>  \<rangle>"
+     using \<open>mult_uncurried \<circ>\<^sub>c (id\<^sub>c \<nat>\<^sub>c \<times>\<^sub>f mult_uncurried) \<circ>\<^sub>c \<langle>left_cart_proj \<nat>\<^sub>c \<nat>\<^sub>c \<circ>\<^sub>c left_cart_proj (\<nat>\<^sub>c \<times>\<^sub>c \<nat>\<^sub>c) \<nat>\<^sub>c,\<langle>right_cart_proj \<nat>\<^sub>c \<nat>\<^sub>c \<circ>\<^sub>c left_cart_proj (\<nat>\<^sub>c \<times>\<^sub>c \<nat>\<^sub>c) \<nat>\<^sub>c,right_cart_proj (\<nat>\<^sub>c \<times>\<^sub>c \<nat>\<^sub>c) \<nat>\<^sub>c\<rangle>\<rangle> \<circ>\<^sub>c \<langle>\<langle>a,b\<rangle>,zero\<rangle> = mult_uncurried \<circ>\<^sub>c (id\<^sub>c \<nat>\<^sub>c \<times>\<^sub>f mult_uncurried) \<circ>\<^sub>c \<langle>left_cart_proj \<nat>\<^sub>c \<nat>\<^sub>c \<circ>\<^sub>c left_cart_proj (\<nat>\<^sub>c \<times>\<^sub>c \<nat>\<^sub>c) \<nat>\<^sub>c \<circ>\<^sub>c \<langle>\<langle>a,b\<rangle>,zero\<rangle>,\<langle>right_cart_proj \<nat>\<^sub>c \<nat>\<^sub>c \<circ>\<^sub>c left_cart_proj (\<nat>\<^sub>c \<times>\<^sub>c \<nat>\<^sub>c) \<nat>\<^sub>c,right_cart_proj (\<nat>\<^sub>c \<times>\<^sub>c \<nat>\<^sub>c) \<nat>\<^sub>c\<rangle> \<circ>\<^sub>c \<langle>\<langle>a,b\<rangle>,zero\<rangle>\<rangle>\<close> ab_type assms(1) assms(2) associate_right_ap associate_right_def left_cart_proj_cfunc_prod right_cart_proj_cfunc_prod zero_type by auto
+   also have "... = mult_uncurried \<circ>\<^sub>c (id\<^sub>c \<nat>\<^sub>c  \<times>\<^sub>f mult_uncurried) \<circ>\<^sub>c \<langle>(left_cart_proj \<nat>\<^sub>c \<nat>\<^sub>c) \<circ>\<^sub>c  \<langle>a,b\<rangle>,
+\<langle>(right_cart_proj \<nat>\<^sub>c \<nat>\<^sub>c) \<circ>\<^sub>c  \<langle>a,b\<rangle>  ,zero  \<rangle>  \<rangle>"
+     using ab_type left_cart_proj_cfunc_prod right_cart_proj_cfunc_prod zero_type by auto
+   also have "... = mult_uncurried \<circ>\<^sub>c (id\<^sub>c \<nat>\<^sub>c  \<times>\<^sub>f mult_uncurried) \<circ>\<^sub>c \<langle>a , \<langle>b,zero\<rangle>  \<rangle>"
+     using assms(1) assms(2) left_cart_proj_cfunc_prod right_cart_proj_cfunc_prod by auto
+   also have "... = mult_uncurried \<circ>\<^sub>c  \<langle>id\<^sub>c \<nat>\<^sub>c \<circ>\<^sub>c a ,mult_uncurried \<circ>\<^sub>c \<langle>b,zero\<rangle>  \<rangle>"
+     using assms(1) b0_type id_type mult_uncurried_type cfunc_cross_prod_comp_cfunc_prod by fastforce
+   also have "... = zero"
+     using assms(1) assms(2) id_left_unit2 mult_def mult_respects_zero_right by auto
+        then show ?thesis using calculation by auto
+qed
+
+ (*Moreover,...*)
+
+     have f3: "((eval_func \<nat>\<^sub>c (\<nat>\<^sub>c\<times>\<^sub>c\<nat>\<^sub>c))\<circ>\<^sub>c 
+(id\<^sub>c (\<nat>\<^sub>c\<times>\<^sub>c\<nat>\<^sub>c) \<times>\<^sub>f (zero \<circ>\<^sub>c \<beta>\<^bsub>(\<nat>\<^sub>c\<times>\<^sub>c \<nat>\<^sub>c)\<times>\<^sub>cone\<^esub>)\<^sup>\<sharp>))  \<circ>\<^sub>c \<langle>\<langle>a,b\<rangle>,id\<^sub>c one\<rangle> = zero"
+     proof - 
+       have "((eval_func \<nat>\<^sub>c (\<nat>\<^sub>c\<times>\<^sub>c\<nat>\<^sub>c))\<circ>\<^sub>c 
+(id\<^sub>c (\<nat>\<^sub>c\<times>\<^sub>c\<nat>\<^sub>c) \<times>\<^sub>f (zero \<circ>\<^sub>c \<beta>\<^bsub>(\<nat>\<^sub>c\<times>\<^sub>c \<nat>\<^sub>c)\<times>\<^sub>cone\<^esub>)\<^sup>\<sharp>))  \<circ>\<^sub>c \<langle>\<langle>a,b\<rangle>,id\<^sub>c one\<rangle> =
+(eval_func \<nat>\<^sub>c (\<nat>\<^sub>c\<times>\<^sub>c\<nat>\<^sub>c))\<circ>\<^sub>c 
+(id\<^sub>c (\<nat>\<^sub>c\<times>\<^sub>c\<nat>\<^sub>c) \<times>\<^sub>f (zero \<circ>\<^sub>c \<beta>\<^bsub>(\<nat>\<^sub>c\<times>\<^sub>c \<nat>\<^sub>c)\<times>\<^sub>cone\<^esub>)\<^sup>\<sharp>)  \<circ>\<^sub>c \<langle>\<langle>a,b\<rangle>,id\<^sub>c one\<rangle>"
+         by (simp add: comp_associative)
+       also have "... =  (zero \<circ>\<^sub>c \<beta>\<^bsub>(\<nat>\<^sub>c\<times>\<^sub>c \<nat>\<^sub>c)\<times>\<^sub>cone\<^esub>) \<circ>\<^sub>c \<langle>\<langle>a,b\<rangle>,id\<^sub>c one\<rangle>"
+         by (metis calculation transpose_func_def zero_betaN_type)
+       also have "... = zero \<circ>\<^sub>c (\<beta>\<^bsub>(\<nat>\<^sub>c\<times>\<^sub>c \<nat>\<^sub>c)\<times>\<^sub>cone\<^esub> \<circ>\<^sub>c \<langle>\<langle>a,b\<rangle>,id\<^sub>c one\<rangle>)"
+         by (simp add: comp_associative)
+       also have "... = zero"
+         using abId_type beta_N_succ_mEqs_Id1 comp_associative id_right_unit2 successor_type terminal_func_comp zero_type by auto
+      then show ?thesis using calculation by auto
+qed
+
+(*Equation before "Likewise..." on page 19*)
+  have f4: "((eval_func \<nat>\<^sub>c (\<nat>\<^sub>c\<times>\<^sub>c\<nat>\<^sub>c))\<circ>\<^sub>c 
+(id\<^sub>c (\<nat>\<^sub>c\<times>\<^sub>c\<nat>\<^sub>c) \<times>\<^sub>f (mult_uncurried \<circ>\<^sub>c (mult_uncurried \<times>\<^sub>f id\<^sub>c \<nat>\<^sub>c))\<^sup>\<sharp>\<circ>\<^sub>c successor) )
+\<circ>\<^sub>c \<langle>\<langle>a,b\<rangle>,c\<rangle> = (a \<cdot>\<^sub>\<nat> b)  \<cdot>\<^sub>\<nat> (successor  \<circ>\<^sub>c c)"
+  proof - 
+    have "((eval_func \<nat>\<^sub>c (\<nat>\<^sub>c\<times>\<^sub>c\<nat>\<^sub>c))\<circ>\<^sub>c 
+(id\<^sub>c (\<nat>\<^sub>c\<times>\<^sub>c\<nat>\<^sub>c) \<times>\<^sub>f (mult_uncurried \<circ>\<^sub>c (mult_uncurried \<times>\<^sub>f id\<^sub>c \<nat>\<^sub>c))\<^sup>\<sharp>\<circ>\<^sub>c successor) )
+\<circ>\<^sub>c \<langle>\<langle>a,b\<rangle>,c\<rangle> = (eval_func \<nat>\<^sub>c (\<nat>\<^sub>c\<times>\<^sub>c\<nat>\<^sub>c))\<circ>\<^sub>c 
+(id\<^sub>c (\<nat>\<^sub>c\<times>\<^sub>c\<nat>\<^sub>c) \<times>\<^sub>f (mult_uncurried \<circ>\<^sub>c (mult_uncurried \<times>\<^sub>f id\<^sub>c \<nat>\<^sub>c))\<^sup>\<sharp>\<circ>\<^sub>c successor) 
+\<circ>\<^sub>c \<langle>\<langle>a,b\<rangle>,c\<rangle>"
+      by (simp add: comp_associative)
+    also have "... = (eval_func \<nat>\<^sub>c (\<nat>\<^sub>c\<times>\<^sub>c\<nat>\<^sub>c))\<circ>\<^sub>c 
+(id\<^sub>c (\<nat>\<^sub>c\<times>\<^sub>c\<nat>\<^sub>c) \<times>\<^sub>f (mult_uncurried \<circ>\<^sub>c (mult_uncurried \<times>\<^sub>f id\<^sub>c \<nat>\<^sub>c))\<^sup>\<sharp>)\<circ>\<^sub>c (id\<^sub>c (\<nat>\<^sub>c\<times>\<^sub>c\<nat>\<^sub>c) \<times>\<^sub>f successor) 
+\<circ>\<^sub>c \<langle>\<langle>a,b\<rangle>,c\<rangle>"
+      using comp_associative identity_distributes_across_composition multmultIdSharp_type successor_type by auto
+    also have "... = mult_uncurried \<circ>\<^sub>c (mult_uncurried \<times>\<^sub>f id\<^sub>c \<nat>\<^sub>c) \<circ>\<^sub>c (id\<^sub>c (\<nat>\<^sub>c\<times>\<^sub>c\<nat>\<^sub>c) \<times>\<^sub>f successor) \<circ>\<^sub>c \<langle>\<langle>a,b\<rangle>,c\<rangle>"
+      using comp_associative flat_cancels_sharp inv_transpose_func_def2 multmultIdSharp_type multmultId_type by fastforce
+    also have "... = mult_uncurried \<circ>\<^sub>c (mult_uncurried \<times>\<^sub>f id\<^sub>c \<nat>\<^sub>c) \<circ>\<^sub>c \<langle>id\<^sub>c (\<nat>\<^sub>c\<times>\<^sub>c\<nat>\<^sub>c)\<circ>\<^sub>c  \<langle>a,b\<rangle>,successor \<circ>\<^sub>c c\<rangle>"
+      using ab_type assms(3) cfunc_cross_prod_comp_cfunc_prod id_type successor_type by fastforce
+    also have "... = mult_uncurried \<circ>\<^sub>c \<langle>mult_uncurried \<circ>\<^sub>c  (id\<^sub>c (\<nat>\<^sub>c\<times>\<^sub>c\<nat>\<^sub>c)\<circ>\<^sub>c  \<langle>a,b\<rangle>),id\<^sub>c \<nat>\<^sub>c \<circ>\<^sub>c (successor \<circ>\<^sub>c c)\<rangle>"
+      using id_ab_type sc_type mult_uncurried_type id_type cfunc_cross_prod_comp_cfunc_prod by fastforce
+    also have "... =  mult_uncurried \<circ>\<^sub>c \<langle>mult_uncurried \<circ>\<^sub>c  (\<langle>a,b\<rangle>),(successor \<circ>\<^sub>c c)\<rangle>"
+      using ab_type id_left_unit2 sc_type by auto
+    also have "... = (a \<cdot>\<^sub>\<nat> b)  \<cdot>\<^sub>\<nat> (successor  \<circ>\<^sub>c c)"
+      by (simp add: mult_def)
+then show ?thesis using calculation by auto
+qed
+
+(*Likewise ...*)
+
+  have f5: "((eval_func \<nat>\<^sub>c (\<nat>\<^sub>c\<times>\<^sub>c\<nat>\<^sub>c))\<circ>\<^sub>c 
+(id\<^sub>c (\<nat>\<^sub>c\<times>\<^sub>c\<nat>\<^sub>c) \<times>\<^sub>f ((mult_uncurried \<circ>\<^sub>c (id\<^sub>c \<nat>\<^sub>c  \<times>\<^sub>f mult_uncurried) \<circ>\<^sub>c \<langle>(left_cart_proj \<nat>\<^sub>c \<nat>\<^sub>c) \<circ>\<^sub>c (left_cart_proj (\<nat>\<^sub>c\<times>\<^sub>c \<nat>\<^sub>c) \<nat>\<^sub>c),
+\<langle>(right_cart_proj \<nat>\<^sub>c \<nat>\<^sub>c) \<circ>\<^sub>c (left_cart_proj (\<nat>\<^sub>c\<times>\<^sub>c \<nat>\<^sub>c) \<nat>\<^sub>c), (right_cart_proj (\<nat>\<^sub>c\<times>\<^sub>c \<nat>\<^sub>c) \<nat>\<^sub>c)\<rangle>\<rangle>)\<^sup>\<sharp> \<circ>\<^sub>c successor)))
+\<circ>\<^sub>c \<langle>\<langle>a,b\<rangle>,c\<rangle> = a \<cdot>\<^sub>\<nat> (b  \<cdot>\<^sub>\<nat> (successor  \<circ>\<^sub>c c))"
+  proof - 
+    have "((eval_func \<nat>\<^sub>c (\<nat>\<^sub>c\<times>\<^sub>c\<nat>\<^sub>c))\<circ>\<^sub>c 
+(id\<^sub>c (\<nat>\<^sub>c\<times>\<^sub>c\<nat>\<^sub>c) \<times>\<^sub>f ((mult_uncurried \<circ>\<^sub>c (id\<^sub>c \<nat>\<^sub>c  \<times>\<^sub>f mult_uncurried) \<circ>\<^sub>c \<langle>(left_cart_proj \<nat>\<^sub>c \<nat>\<^sub>c) \<circ>\<^sub>c (left_cart_proj (\<nat>\<^sub>c\<times>\<^sub>c \<nat>\<^sub>c) \<nat>\<^sub>c),
+\<langle>(right_cart_proj \<nat>\<^sub>c \<nat>\<^sub>c) \<circ>\<^sub>c (left_cart_proj (\<nat>\<^sub>c\<times>\<^sub>c \<nat>\<^sub>c) \<nat>\<^sub>c), (right_cart_proj (\<nat>\<^sub>c\<times>\<^sub>c \<nat>\<^sub>c) \<nat>\<^sub>c)\<rangle>\<rangle>)\<^sup>\<sharp> \<circ>\<^sub>c successor)))
+\<circ>\<^sub>c \<langle>\<langle>a,b\<rangle>,c\<rangle> =(eval_func \<nat>\<^sub>c (\<nat>\<^sub>c\<times>\<^sub>c\<nat>\<^sub>c))\<circ>\<^sub>c 
+(id\<^sub>c (\<nat>\<^sub>c\<times>\<^sub>c\<nat>\<^sub>c) \<times>\<^sub>f ((mult_uncurried \<circ>\<^sub>c (id\<^sub>c \<nat>\<^sub>c  \<times>\<^sub>f mult_uncurried) \<circ>\<^sub>c \<langle>(left_cart_proj \<nat>\<^sub>c \<nat>\<^sub>c) \<circ>\<^sub>c (left_cart_proj (\<nat>\<^sub>c\<times>\<^sub>c \<nat>\<^sub>c) \<nat>\<^sub>c),
+\<langle>(right_cart_proj \<nat>\<^sub>c \<nat>\<^sub>c) \<circ>\<^sub>c (left_cart_proj (\<nat>\<^sub>c\<times>\<^sub>c \<nat>\<^sub>c) \<nat>\<^sub>c), (right_cart_proj (\<nat>\<^sub>c\<times>\<^sub>c \<nat>\<^sub>c) \<nat>\<^sub>c)\<rangle>\<rangle>)\<^sup>\<sharp> \<circ>\<^sub>c successor))
+\<circ>\<^sub>c \<langle>\<langle>a,b\<rangle>,c\<rangle>"
+      using comp_associative by auto
+    also have "... = (eval_func \<nat>\<^sub>c (\<nat>\<^sub>c\<times>\<^sub>c\<nat>\<^sub>c))\<circ>\<^sub>c 
+(id\<^sub>c (\<nat>\<^sub>c\<times>\<^sub>c\<nat>\<^sub>c) \<times>\<^sub>f ((mult_uncurried \<circ>\<^sub>c (id\<^sub>c \<nat>\<^sub>c  \<times>\<^sub>f mult_uncurried) \<circ>\<^sub>c \<langle>(left_cart_proj \<nat>\<^sub>c \<nat>\<^sub>c) \<circ>\<^sub>c (left_cart_proj (\<nat>\<^sub>c\<times>\<^sub>c \<nat>\<^sub>c) \<nat>\<^sub>c),
+\<langle>(right_cart_proj \<nat>\<^sub>c \<nat>\<^sub>c) \<circ>\<^sub>c (left_cart_proj (\<nat>\<^sub>c\<times>\<^sub>c \<nat>\<^sub>c) \<nat>\<^sub>c), (right_cart_proj (\<nat>\<^sub>c\<times>\<^sub>c \<nat>\<^sub>c) \<nat>\<^sub>c)\<rangle>\<rangle>)\<^sup>\<sharp>))
+\<circ>\<^sub>c (id\<^sub>c (\<nat>\<^sub>c\<times>\<^sub>c\<nat>\<^sub>c) \<times>\<^sub>f  successor)
+\<circ>\<^sub>c \<langle>\<langle>a,b\<rangle>,c\<rangle>"
+      using comp_associative identity_distributes_across_composition multIdxMultp0p0p1p0p1_Sharp_type successor_type by auto
+    also have "... = (mult_uncurried \<circ>\<^sub>c (id\<^sub>c \<nat>\<^sub>c  \<times>\<^sub>f mult_uncurried) \<circ>\<^sub>c \<langle>(left_cart_proj \<nat>\<^sub>c \<nat>\<^sub>c) \<circ>\<^sub>c (left_cart_proj (\<nat>\<^sub>c\<times>\<^sub>c \<nat>\<^sub>c) \<nat>\<^sub>c),
+\<langle>(right_cart_proj \<nat>\<^sub>c \<nat>\<^sub>c) \<circ>\<^sub>c (left_cart_proj (\<nat>\<^sub>c\<times>\<^sub>c \<nat>\<^sub>c) \<nat>\<^sub>c), (right_cart_proj (\<nat>\<^sub>c\<times>\<^sub>c \<nat>\<^sub>c) \<nat>\<^sub>c)\<rangle>\<rangle>)
+\<circ>\<^sub>c (id\<^sub>c (\<nat>\<^sub>c\<times>\<^sub>c\<nat>\<^sub>c) \<times>\<^sub>f  successor)
+\<circ>\<^sub>c \<langle>\<langle>a,b\<rangle>,c\<rangle>"
+      using comp_associative flat_cancels_sharp inv_transpose_func_def2 multIdxMultp0p0p1p0p1_Sharp_type multIdxMultp0p0p1p0p1_type by fastforce
+    also have "... = (mult_uncurried \<circ>\<^sub>c (id\<^sub>c \<nat>\<^sub>c  \<times>\<^sub>f mult_uncurried) \<circ>\<^sub>c \<langle>(left_cart_proj \<nat>\<^sub>c \<nat>\<^sub>c) \<circ>\<^sub>c (left_cart_proj (\<nat>\<^sub>c\<times>\<^sub>c \<nat>\<^sub>c) \<nat>\<^sub>c),
+\<langle>(right_cart_proj \<nat>\<^sub>c \<nat>\<^sub>c) \<circ>\<^sub>c (left_cart_proj (\<nat>\<^sub>c\<times>\<^sub>c \<nat>\<^sub>c) \<nat>\<^sub>c), (right_cart_proj (\<nat>\<^sub>c\<times>\<^sub>c \<nat>\<^sub>c) \<nat>\<^sub>c)\<rangle>\<rangle>)
+\<circ>\<^sub>c \<langle>id\<^sub>c (\<nat>\<^sub>c\<times>\<^sub>c\<nat>\<^sub>c) \<circ>\<^sub>c \<langle>a,b\<rangle>,successor  \<circ>\<^sub>c c\<rangle>"
+      using ab_type assms(3) cfunc_cross_prod_comp_cfunc_prod id_type successor_type by fastforce
+    also have "... = (mult_uncurried \<circ>\<^sub>c (id\<^sub>c \<nat>\<^sub>c  \<times>\<^sub>f mult_uncurried) \<circ>\<^sub>c \<langle>(left_cart_proj \<nat>\<^sub>c \<nat>\<^sub>c) \<circ>\<^sub>c (left_cart_proj (\<nat>\<^sub>c\<times>\<^sub>c \<nat>\<^sub>c) \<nat>\<^sub>c),
+\<langle>(right_cart_proj \<nat>\<^sub>c \<nat>\<^sub>c) \<circ>\<^sub>c (left_cart_proj (\<nat>\<^sub>c\<times>\<^sub>c \<nat>\<^sub>c) \<nat>\<^sub>c), (right_cart_proj (\<nat>\<^sub>c\<times>\<^sub>c \<nat>\<^sub>c) \<nat>\<^sub>c)\<rangle>\<rangle>)
+\<circ>\<^sub>c \<langle>\<langle>a,b\<rangle>,successor  \<circ>\<^sub>c c\<rangle>"
+      using ab_type id_left_unit2 by auto
+    also have "... = mult_uncurried \<circ>\<^sub>c (id\<^sub>c \<nat>\<^sub>c  \<times>\<^sub>f mult_uncurried) \<circ>\<^sub>c \<langle>(left_cart_proj \<nat>\<^sub>c \<nat>\<^sub>c) \<circ>\<^sub>c (left_cart_proj (\<nat>\<^sub>c\<times>\<^sub>c \<nat>\<^sub>c) \<nat>\<^sub>c),
+\<langle>(right_cart_proj \<nat>\<^sub>c \<nat>\<^sub>c) \<circ>\<^sub>c (left_cart_proj (\<nat>\<^sub>c\<times>\<^sub>c \<nat>\<^sub>c) \<nat>\<^sub>c), (right_cart_proj (\<nat>\<^sub>c\<times>\<^sub>c \<nat>\<^sub>c) \<nat>\<^sub>c)\<rangle>\<rangle>
+\<circ>\<^sub>c \<langle>\<langle>a,b\<rangle>,successor  \<circ>\<^sub>c c\<rangle>"
+      using comp_associative by force
+    also have "... = mult_uncurried \<circ>\<^sub>c (id\<^sub>c \<nat>\<^sub>c  \<times>\<^sub>f mult_uncurried) \<circ>\<^sub>c \<langle>(left_cart_proj \<nat>\<^sub>c \<nat>\<^sub>c) \<circ>\<^sub>c (left_cart_proj (\<nat>\<^sub>c\<times>\<^sub>c \<nat>\<^sub>c) \<nat>\<^sub>c)\<circ>\<^sub>c \<langle>\<langle>a,b\<rangle>,successor  \<circ>\<^sub>c c\<rangle> ,
+\<langle>(right_cart_proj \<nat>\<^sub>c \<nat>\<^sub>c) \<circ>\<^sub>c (left_cart_proj (\<nat>\<^sub>c\<times>\<^sub>c \<nat>\<^sub>c) \<nat>\<^sub>c), (right_cart_proj (\<nat>\<^sub>c\<times>\<^sub>c \<nat>\<^sub>c) \<nat>\<^sub>c)\<rangle>    \<circ>\<^sub>c \<langle>\<langle>a,b\<rangle>,successor  \<circ>\<^sub>c c\<rangle>   \<rangle>"
+      using abSc_type cfunc_prod_comp comp_associative p0rho0_type p1rho0rho1_type by auto
+    also have "... = mult_uncurried \<circ>\<^sub>c (id\<^sub>c \<nat>\<^sub>c  \<times>\<^sub>f mult_uncurried) \<circ>\<^sub>c \<langle>(left_cart_proj \<nat>\<^sub>c \<nat>\<^sub>c) \<circ>\<^sub>c \<langle>a,b\<rangle> ,
+\<langle>(right_cart_proj \<nat>\<^sub>c \<nat>\<^sub>c) \<circ>\<^sub>c (left_cart_proj (\<nat>\<^sub>c\<times>\<^sub>c \<nat>\<^sub>c) \<nat>\<^sub>c)\<circ>\<^sub>c \<langle>\<langle>a,b\<rangle>,successor  \<circ>\<^sub>c c\<rangle>  , (right_cart_proj (\<nat>\<^sub>c\<times>\<^sub>c \<nat>\<^sub>c) \<nat>\<^sub>c) \<circ>\<^sub>c \<langle>\<langle>a,b\<rangle>,successor  \<circ>\<^sub>c c\<rangle>\<rangle>\<rangle>"
+      by (smt abSc_type ab_type cfunc_prod_comp comp_associative left_cart_proj_cfunc_prod p1rho0_type right_cart_proj_type sc_type)
+    also have "... = mult_uncurried \<circ>\<^sub>c (id\<^sub>c \<nat>\<^sub>c  \<times>\<^sub>f mult_uncurried) \<circ>\<^sub>c \<langle>a ,
+\<langle>(right_cart_proj \<nat>\<^sub>c \<nat>\<^sub>c) \<circ>\<^sub>c \<langle>a,b\<rangle>  , successor  \<circ>\<^sub>c c  \<rangle>  \<rangle>"
+      using ab_type assms(1) assms(2) left_cart_proj_cfunc_prod right_cart_proj_cfunc_prod sc_type by auto
+    also have "... = mult_uncurried \<circ>\<^sub>c (id\<^sub>c \<nat>\<^sub>c  \<times>\<^sub>f mult_uncurried) \<circ>\<^sub>c \<langle>a,\<langle>b,successor  \<circ>\<^sub>c c\<rangle>\<rangle>"
+      using assms(1) assms(2) right_cart_proj_cfunc_prod by auto
+    also have "... = mult_uncurried \<circ>\<^sub>c  \<langle>id\<^sub>c \<nat>\<^sub>c \<circ>\<^sub>c a, mult_uncurried \<circ>\<^sub>c \<langle>b,successor  \<circ>\<^sub>c c\<rangle>\<rangle>"
+      using assms(1) bSc_type id_type mult_uncurried_type cfunc_cross_prod_comp_cfunc_prod by fastforce
+    also have "... =   a \<cdot>\<^sub>\<nat> (b  \<cdot>\<^sub>\<nat> (successor  \<circ>\<^sub>c c))"
+      using assms(1) id_left_unit2 mult_def by auto
+then show ?thesis using calculation by auto
+qed
+
+(*Now we compute this pair... *)
+
+  have f6: "((eval_func \<nat>\<^sub>c (\<nat>\<^sub>c\<times>\<^sub>c\<nat>\<^sub>c))\<circ>\<^sub>c 
+(id\<^sub>c (\<nat>\<^sub>c\<times>\<^sub>c\<nat>\<^sub>c) \<times>\<^sub>f ((add_uncurried \<circ>\<^sub>c \<langle>mult_uncurried \<circ>\<^sub>c (left_cart_proj (\<nat>\<^sub>c\<times>\<^sub>c\<nat>\<^sub>c) (\<nat>\<^sub>c\<^bsup>(\<nat>\<^sub>c\<times>\<^sub>c\<nat>\<^sub>c)\<^esup>)),eval_func \<nat>\<^sub>c (\<nat>\<^sub>c\<times>\<^sub>c\<nat>\<^sub>c)\<rangle>)\<^sup>\<sharp>)
+\<circ>\<^sub>c ((mult_uncurried \<circ>\<^sub>c (mult_uncurried \<times>\<^sub>f id\<^sub>c \<nat>\<^sub>c))\<^sup>\<sharp>)
+))  \<circ>\<^sub>c \<langle>\<langle>a,b\<rangle>,c\<rangle> = (a \<cdot>\<^sub>\<nat> b)  \<cdot>\<^sub>\<nat> (successor  \<circ>\<^sub>c c)"
+  proof - 
+    have "((eval_func \<nat>\<^sub>c (\<nat>\<^sub>c\<times>\<^sub>c\<nat>\<^sub>c))\<circ>\<^sub>c 
+(id\<^sub>c (\<nat>\<^sub>c\<times>\<^sub>c\<nat>\<^sub>c) \<times>\<^sub>f ((add_uncurried \<circ>\<^sub>c \<langle>mult_uncurried \<circ>\<^sub>c (left_cart_proj (\<nat>\<^sub>c\<times>\<^sub>c\<nat>\<^sub>c) (\<nat>\<^sub>c\<^bsup>(\<nat>\<^sub>c\<times>\<^sub>c\<nat>\<^sub>c)\<^esup>)),eval_func \<nat>\<^sub>c (\<nat>\<^sub>c\<times>\<^sub>c\<nat>\<^sub>c)\<rangle>)\<^sup>\<sharp>)
+\<circ>\<^sub>c ((mult_uncurried \<circ>\<^sub>c (mult_uncurried \<times>\<^sub>f id\<^sub>c \<nat>\<^sub>c))\<^sup>\<sharp>)
+))  \<circ>\<^sub>c \<langle>\<langle>a,b\<rangle>,c\<rangle> = 
+ (eval_func \<nat>\<^sub>c (\<nat>\<^sub>c\<times>\<^sub>c\<nat>\<^sub>c))\<circ>\<^sub>c 
+(id\<^sub>c (\<nat>\<^sub>c\<times>\<^sub>c\<nat>\<^sub>c) \<times>\<^sub>f ((add_uncurried \<circ>\<^sub>c \<langle>mult_uncurried \<circ>\<^sub>c (left_cart_proj (\<nat>\<^sub>c\<times>\<^sub>c\<nat>\<^sub>c) (\<nat>\<^sub>c\<^bsup>(\<nat>\<^sub>c\<times>\<^sub>c\<nat>\<^sub>c)\<^esup>)),eval_func \<nat>\<^sub>c (\<nat>\<^sub>c\<times>\<^sub>c\<nat>\<^sub>c)\<rangle>)\<^sup>\<sharp>)
+\<circ>\<^sub>c ((mult_uncurried \<circ>\<^sub>c (mult_uncurried \<times>\<^sub>f id\<^sub>c \<nat>\<^sub>c))\<^sup>\<sharp>)
+)  \<circ>\<^sub>c \<langle>\<langle>a,b\<rangle>,c\<rangle>"
+      by (simp add: comp_associative)
+    also have "... = (eval_func \<nat>\<^sub>c (\<nat>\<^sub>c\<times>\<^sub>c\<nat>\<^sub>c))\<circ>\<^sub>c 
+(id\<^sub>c (\<nat>\<^sub>c\<times>\<^sub>c\<nat>\<^sub>c) \<times>\<^sub>f ((add_uncurried \<circ>\<^sub>c \<langle>mult_uncurried \<circ>\<^sub>c (left_cart_proj (\<nat>\<^sub>c\<times>\<^sub>c\<nat>\<^sub>c) (\<nat>\<^sub>c\<^bsup>(\<nat>\<^sub>c\<times>\<^sub>c\<nat>\<^sub>c)\<^esup>)),eval_func \<nat>\<^sub>c (\<nat>\<^sub>c\<times>\<^sub>c\<nat>\<^sub>c)\<rangle>)\<^sup>\<sharp>)) \<circ>\<^sub>c 
+(id\<^sub>c (\<nat>\<^sub>c\<times>\<^sub>c\<nat>\<^sub>c) \<times>\<^sub>f ((mult_uncurried \<circ>\<^sub>c (mult_uncurried \<times>\<^sub>f id\<^sub>c \<nat>\<^sub>c))\<^sup>\<sharp>))\<circ>\<^sub>c
+\<langle>\<langle>a,b\<rangle>,c\<rangle>"
+      using addMultSigma0EvalSharp_type comp_associative identity_distributes_across_composition multmultIdSharp_type by auto
+    also have "... = (add_uncurried \<circ>\<^sub>c \<langle>mult_uncurried \<circ>\<^sub>c (left_cart_proj (\<nat>\<^sub>c\<times>\<^sub>c\<nat>\<^sub>c) (\<nat>\<^sub>c\<^bsup>(\<nat>\<^sub>c\<times>\<^sub>c\<nat>\<^sub>c)\<^esup>)),eval_func \<nat>\<^sub>c (\<nat>\<^sub>c\<times>\<^sub>c\<nat>\<^sub>c)\<rangle>) \<circ>\<^sub>c 
+(id\<^sub>c (\<nat>\<^sub>c\<times>\<^sub>c\<nat>\<^sub>c) \<times>\<^sub>f ((mult_uncurried \<circ>\<^sub>c (mult_uncurried \<times>\<^sub>f id\<^sub>c \<nat>\<^sub>c))\<^sup>\<sharp>))\<circ>\<^sub>c
+\<langle>\<langle>a,b\<rangle>,c\<rangle>"
+      using addMultSigma0Eval_type comp_associative transpose_func_def by presburger
+    also have "... = ((add_uncurried \<circ>\<^sub>c
+\<langle>mult_uncurried \<circ>\<^sub>c (left_cart_proj (\<nat>\<^sub>c\<times>\<^sub>c\<nat>\<^sub>c) (\<nat>\<^sub>c\<^bsup>(\<nat>\<^sub>c\<times>\<^sub>c\<nat>\<^sub>c)\<^esup>)),
+eval_func \<nat>\<^sub>c (\<nat>\<^sub>c\<times>\<^sub>c\<nat>\<^sub>c)\<rangle>) 
+\<circ>\<^sub>c (id\<^sub>c (\<nat>\<^sub>c\<times>\<^sub>c\<nat>\<^sub>c) \<times>\<^sub>f ((mult_uncurried \<circ>\<^sub>c (mult_uncurried \<times>\<^sub>f id\<^sub>c \<nat>\<^sub>c))\<^sup>\<sharp>)))
+\<circ>\<^sub>c\<langle>\<langle>a,b\<rangle>,c\<rangle>"
+      by (simp add: comp_associative)
+    also have "... = (
+add_uncurried \<circ>\<^sub>c
+\<langle>mult_uncurried \<circ>\<^sub>c (left_cart_proj (\<nat>\<^sub>c\<times>\<^sub>c\<nat>\<^sub>c) (\<nat>\<^sub>c\<^bsup>(\<nat>\<^sub>c\<times>\<^sub>c\<nat>\<^sub>c)\<^esup>))
+\<circ>\<^sub>c (id\<^sub>c (\<nat>\<^sub>c\<times>\<^sub>c\<nat>\<^sub>c) \<times>\<^sub>f ((mult_uncurried \<circ>\<^sub>c (mult_uncurried \<times>\<^sub>f id\<^sub>c \<nat>\<^sub>c))\<^sup>\<sharp>)),
+eval_func \<nat>\<^sub>c (\<nat>\<^sub>c\<times>\<^sub>c\<nat>\<^sub>c)
+\<circ>\<^sub>c (id\<^sub>c (\<nat>\<^sub>c\<times>\<^sub>c\<nat>\<^sub>c) \<times>\<^sub>f ((mult_uncurried \<circ>\<^sub>c (mult_uncurried \<times>\<^sub>f id\<^sub>c \<nat>\<^sub>c))\<^sup>\<sharp>))\<rangle> 
+)
+\<circ>\<^sub>c\<langle>\<langle>a,b\<rangle>,c\<rangle>"
+      by (smt cfunc_prod_comp comp_associative eval_func_type id_multmultidsharp_type multsigma0_type)
+    also have "... = (
+add_uncurried \<circ>\<^sub>c
+\<langle>mult_uncurried \<circ>\<^sub>c (id\<^sub>c (\<nat>\<^sub>c\<times>\<^sub>c\<nat>\<^sub>c) \<circ>\<^sub>c left_cart_proj (\<nat>\<^sub>c\<times>\<^sub>c\<nat>\<^sub>c) \<nat>\<^sub>c) ,
+eval_func \<nat>\<^sub>c (\<nat>\<^sub>c\<times>\<^sub>c\<nat>\<^sub>c)
+\<circ>\<^sub>c (id\<^sub>c (\<nat>\<^sub>c\<times>\<^sub>c\<nat>\<^sub>c) \<times>\<^sub>f ((mult_uncurried \<circ>\<^sub>c (mult_uncurried \<times>\<^sub>f id\<^sub>c \<nat>\<^sub>c))\<^sup>\<sharp>))\<rangle> 
+)
+\<circ>\<^sub>c\<langle>\<langle>a,b\<rangle>,c\<rangle>"
+      by (smt id_type left_cart_proj_cfunc_cross_prod multmultIdSharp_type)
+    also have "... = 
+add_uncurried \<circ>\<^sub>c
+\<langle>mult_uncurried \<circ>\<^sub>c left_cart_proj (\<nat>\<^sub>c\<times>\<^sub>c\<nat>\<^sub>c) \<nat>\<^sub>c ,
+eval_func \<nat>\<^sub>c (\<nat>\<^sub>c\<times>\<^sub>c\<nat>\<^sub>c)
+\<circ>\<^sub>c (id\<^sub>c (\<nat>\<^sub>c\<times>\<^sub>c\<nat>\<^sub>c) \<times>\<^sub>f ((mult_uncurried \<circ>\<^sub>c (mult_uncurried \<times>\<^sub>f id\<^sub>c \<nat>\<^sub>c))\<^sup>\<sharp>))\<rangle> 
+\<circ>\<^sub>c\<langle>\<langle>a,b\<rangle>,c\<rangle>"
+      using comp_associative id_right_unit2 mult_uncurried_type by auto
+also have "... = add_uncurried \<circ>\<^sub>c
+\<langle>mult_uncurried \<circ>\<^sub>c left_cart_proj (\<nat>\<^sub>c\<times>\<^sub>c\<nat>\<^sub>c) \<nat>\<^sub>c \<circ>\<^sub>c\<langle>\<langle>a,b\<rangle>,c\<rangle> ,
+eval_func \<nat>\<^sub>c (\<nat>\<^sub>c\<times>\<^sub>c\<nat>\<^sub>c)
+\<circ>\<^sub>c (id\<^sub>c (\<nat>\<^sub>c\<times>\<^sub>c\<nat>\<^sub>c) \<times>\<^sub>f ((mult_uncurried \<circ>\<^sub>c (mult_uncurried \<times>\<^sub>f id\<^sub>c \<nat>\<^sub>c))\<^sup>\<sharp>))\<circ>\<^sub>c\<langle>\<langle>a,b\<rangle>,c\<rangle>   \<rangle>"
+         apply(subst cfunc_prod_comp[where X = "one", where Y= "(\<nat>\<^sub>c\<times>\<^sub>c\<nat>\<^sub>c)\<times>\<^sub>c\<nat>\<^sub>c",
+                    where A = "\<nat>\<^sub>c", where B= "\<nat>\<^sub>c"])
+          using abc_type apply force
+          using comp_type left_cart_proj_type mult_uncurried_type apply blast
+          using multmultId_type transpose_func_def apply auto[1]
+          using comp_associative by presburger
+also have "... =  add_uncurried \<circ>\<^sub>c\<langle>mult_uncurried \<circ>\<^sub>c  \<langle>a,b\<rangle> ,(mult_uncurried \<circ>\<^sub>c (mult_uncurried \<times>\<^sub>f id\<^sub>c \<nat>\<^sub>c)) \<circ>\<^sub>c\<langle>\<langle>a,b\<rangle>,c\<rangle>   \<rangle>"
+    using ab_type assms(3) comp_associative left_cart_proj_cfunc_prod multmultId_type transpose_func_def by auto
+  also have "... = add_uncurried \<circ>\<^sub>c\<langle>mult_uncurried \<circ>\<^sub>c  \<langle>a,b\<rangle> ,mult_uncurried  \<circ>\<^sub>c\<langle>mult_uncurried \<circ>\<^sub>c\<langle>a,b\<rangle>,id\<^sub>c \<nat>\<^sub>c \<circ>\<^sub>c c\<rangle>   \<rangle>"
+    by (smt ab_type assms(3) cfunc_cross_prod_comp_cfunc_prod comp_associative id_type mult_uncurried_type)
+  also have "... = (a \<cdot>\<^sub>\<nat> b) +\<^sub>\<nat> ((a \<cdot>\<^sub>\<nat> b)\<cdot>\<^sub>\<nat> c)"
+    using add_def assms(3) id_left_unit2 mult_def by auto
+  also have "... =  (a \<cdot>\<^sub>\<nat> b)  \<cdot>\<^sub>\<nat> (successor  \<circ>\<^sub>c c)"
+    using assms(3) mult_def mult_respects_succ_right multab_type by auto
+then show ?thesis using calculation by auto
+qed
+
+
+(*Next to last on page 20*)
+
+
+(*
+  have f7: "((eval_func \<nat>\<^sub>c (\<nat>\<^sub>c\<times>\<^sub>c\<nat>\<^sub>c))\<circ>\<^sub>c 
+(id\<^sub>c (\<nat>\<^sub>c\<times>\<^sub>c\<nat>\<^sub>c) \<times>\<^sub>f ((add_uncurried \<circ>\<^sub>c \<langle>mult_uncurried \<circ>\<^sub>c (left_cart_proj (\<nat>\<^sub>c\<times>\<^sub>c\<nat>\<^sub>c) (\<nat>\<^sub>c\<^bsup>(\<nat>\<^sub>c\<times>\<^sub>c\<nat>\<^sub>c)\<^esup>)),eval_func \<nat>\<^sub>c (\<nat>\<^sub>c\<times>\<^sub>c\<nat>\<^sub>c)\<rangle>)\<^sup>\<sharp>)
+\<circ>\<^sub>c  (mult_uncurried \<circ>\<^sub>c (id\<^sub>c \<nat>\<^sub>c  \<times>\<^sub>f mult_uncurried) \<circ>\<^sub>c \<langle>(left_cart_proj \<nat>\<^sub>c \<nat>\<^sub>c) \<circ>\<^sub>c (left_cart_proj (\<nat>\<^sub>c\<times>\<^sub>c \<nat>\<^sub>c) \<nat>\<^sub>c),
+\<langle>(right_cart_proj \<nat>\<^sub>c \<nat>\<^sub>c) \<circ>\<^sub>c (left_cart_proj (\<nat>\<^sub>c\<times>\<^sub>c \<nat>\<^sub>c) \<nat>\<^sub>c), (right_cart_proj (\<nat>\<^sub>c\<times>\<^sub>c \<nat>\<^sub>c) \<nat>\<^sub>c)\<rangle>\<rangle>)\<^sup>\<sharp>
+))  \<circ>\<^sub>c \<langle>\<langle>a,b\<rangle>,c\<rangle> = a \<cdot>\<^sub>\<nat> (b  \<cdot>\<^sub>\<nat> (successor  \<circ>\<^sub>c c))"
+  proof - 
+    have "((eval_func \<nat>\<^sub>c (\<nat>\<^sub>c\<times>\<^sub>c\<nat>\<^sub>c))\<circ>\<^sub>c 
+(id\<^sub>c (\<nat>\<^sub>c\<times>\<^sub>c\<nat>\<^sub>c) \<times>\<^sub>f ((add_uncurried \<circ>\<^sub>c \<langle>mult_uncurried \<circ>\<^sub>c (left_cart_proj (\<nat>\<^sub>c\<times>\<^sub>c\<nat>\<^sub>c) (\<nat>\<^sub>c\<^bsup>(\<nat>\<^sub>c\<times>\<^sub>c\<nat>\<^sub>c)\<^esup>)),eval_func \<nat>\<^sub>c (\<nat>\<^sub>c\<times>\<^sub>c\<nat>\<^sub>c)\<rangle>)\<^sup>\<sharp>)
+\<circ>\<^sub>c  (mult_uncurried \<circ>\<^sub>c (id\<^sub>c \<nat>\<^sub>c  \<times>\<^sub>f mult_uncurried) \<circ>\<^sub>c \<langle>(left_cart_proj \<nat>\<^sub>c \<nat>\<^sub>c) \<circ>\<^sub>c (left_cart_proj (\<nat>\<^sub>c\<times>\<^sub>c \<nat>\<^sub>c) \<nat>\<^sub>c),
+\<langle>(right_cart_proj \<nat>\<^sub>c \<nat>\<^sub>c) \<circ>\<^sub>c (left_cart_proj (\<nat>\<^sub>c\<times>\<^sub>c \<nat>\<^sub>c) \<nat>\<^sub>c), (right_cart_proj (\<nat>\<^sub>c\<times>\<^sub>c \<nat>\<^sub>c) \<nat>\<^sub>c)\<rangle>\<rangle>)\<^sup>\<sharp>
+))  \<circ>\<^sub>c \<langle>\<langle>a,b\<rangle>,c\<rangle> =   
+((eval_func \<nat>\<^sub>c (\<nat>\<^sub>c\<times>\<^sub>c\<nat>\<^sub>c))\<circ>\<^sub>c 
+(id\<^sub>c (\<nat>\<^sub>c\<times>\<^sub>c\<nat>\<^sub>c) \<times>\<^sub>f ((add_uncurried \<circ>\<^sub>c \<langle>mult_uncurried \<circ>\<^sub>c (left_cart_proj (\<nat>\<^sub>c\<times>\<^sub>c\<nat>\<^sub>c) (\<nat>\<^sub>c\<^bsup>(\<nat>\<^sub>c\<times>\<^sub>c\<nat>\<^sub>c)\<^esup>)),eval_func \<nat>\<^sub>c (\<nat>\<^sub>c\<times>\<^sub>c\<nat>\<^sub>c)\<rangle>)\<^sup>\<sharp>)
+))
+\<circ>\<^sub>c ( id\<^sub>c (\<nat>\<^sub>c\<times>\<^sub>c\<nat>\<^sub>c) \<times>\<^sub>f  (mult_uncurried \<circ>\<^sub>c (id\<^sub>c \<nat>\<^sub>c  \<times>\<^sub>f mult_uncurried) \<circ>\<^sub>c \<langle>(left_cart_proj \<nat>\<^sub>c \<nat>\<^sub>c) \<circ>\<^sub>c (left_cart_proj (\<nat>\<^sub>c\<times>\<^sub>c \<nat>\<^sub>c) \<nat>\<^sub>c),
+\<langle>(right_cart_proj \<nat>\<^sub>c \<nat>\<^sub>c) \<circ>\<^sub>c (left_cart_proj (\<nat>\<^sub>c\<times>\<^sub>c \<nat>\<^sub>c) \<nat>\<^sub>c), (right_cart_proj (\<nat>\<^sub>c\<times>\<^sub>c \<nat>\<^sub>c) \<nat>\<^sub>c)\<rangle>\<rangle>)\<^sup>\<sharp>)
+\<circ>\<^sub>c \<langle>\<langle>a,b\<rangle>,c\<rangle>"
+      using addMultSigma0EvalSharp_type comp_associative identity_distributes_across_composition multIdxMultp0p0p1p0p1_Sharp_type by auto
+    also have "... = add_uncurried \<circ>\<^sub>c \<langle>mult_uncurried \<circ>\<^sub>c (left_cart_proj (\<nat>\<^sub>c\<times>\<^sub>c\<nat>\<^sub>c) (\<nat>\<^sub>c\<^bsup>(\<nat>\<^sub>c\<times>\<^sub>c\<nat>\<^sub>c)\<^esup>))
+, eval_func \<nat>\<^sub>c (\<nat>\<^sub>c\<times>\<^sub>c\<nat>\<^sub>c)
+\<rangle>
+\<circ>\<^sub>c ( id\<^sub>c (\<nat>\<^sub>c\<times>\<^sub>c\<nat>\<^sub>c) \<times>\<^sub>f  (mult_uncurried \<circ>\<^sub>c (id\<^sub>c \<nat>\<^sub>c  \<times>\<^sub>f mult_uncurried) \<circ>\<^sub>c \<langle>(left_cart_proj \<nat>\<^sub>c \<nat>\<^sub>c) \<circ>\<^sub>c (left_cart_proj (\<nat>\<^sub>c\<times>\<^sub>c \<nat>\<^sub>c) \<nat>\<^sub>c),
+\<langle>(right_cart_proj \<nat>\<^sub>c \<nat>\<^sub>c) \<circ>\<^sub>c (left_cart_proj (\<nat>\<^sub>c\<times>\<^sub>c \<nat>\<^sub>c) \<nat>\<^sub>c), (right_cart_proj (\<nat>\<^sub>c\<times>\<^sub>c \<nat>\<^sub>c) \<nat>\<^sub>c)\<rangle>\<rangle>)\<^sup>\<sharp>)
+\<circ>\<^sub>c \<langle>\<langle>a,b\<rangle>,c\<rangle>"
+      using comp_associative addMultSigma0Eval_type transpose_func_def by auto
+    also have "...  = (add_uncurried \<circ>\<^sub>c \<langle>mult_uncurried \<circ>\<^sub>c (left_cart_proj (\<nat>\<^sub>c\<times>\<^sub>c\<nat>\<^sub>c) (\<nat>\<^sub>c\<^bsup>(\<nat>\<^sub>c\<times>\<^sub>c\<nat>\<^sub>c)\<^esup>))
+, eval_func \<nat>\<^sub>c (\<nat>\<^sub>c\<times>\<^sub>c\<nat>\<^sub>c)
+\<rangle>
+\<circ>\<^sub>c ( id\<^sub>c (\<nat>\<^sub>c\<times>\<^sub>c\<nat>\<^sub>c) \<times>\<^sub>f  (mult_uncurried \<circ>\<^sub>c (id\<^sub>c \<nat>\<^sub>c  \<times>\<^sub>f mult_uncurried) \<circ>\<^sub>c \<langle>(left_cart_proj \<nat>\<^sub>c \<nat>\<^sub>c) \<circ>\<^sub>c (left_cart_proj (\<nat>\<^sub>c\<times>\<^sub>c \<nat>\<^sub>c) \<nat>\<^sub>c),
+\<langle>(right_cart_proj \<nat>\<^sub>c \<nat>\<^sub>c) \<circ>\<^sub>c (left_cart_proj (\<nat>\<^sub>c\<times>\<^sub>c \<nat>\<^sub>c) \<nat>\<^sub>c), (right_cart_proj (\<nat>\<^sub>c\<times>\<^sub>c \<nat>\<^sub>c) \<nat>\<^sub>c)\<rangle>\<rangle>)\<^sup>\<sharp>)
+)\<circ>\<^sub>c \<langle>\<langle>a,b\<rangle>,c\<rangle>"
+      using comp_associative by auto
+    also have "... = (add_uncurried \<circ>\<^sub>c \<langle>mult_uncurried \<circ>\<^sub>c (left_cart_proj (\<nat>\<^sub>c\<times>\<^sub>c\<nat>\<^sub>c) (\<nat>\<^sub>c\<^bsup>(\<nat>\<^sub>c\<times>\<^sub>c\<nat>\<^sub>c)\<^esup>))
+\<circ>\<^sub>c ( id\<^sub>c (\<nat>\<^sub>c\<times>\<^sub>c\<nat>\<^sub>c) \<times>\<^sub>f  (mult_uncurried \<circ>\<^sub>c (id\<^sub>c \<nat>\<^sub>c  \<times>\<^sub>f mult_uncurried) \<circ>\<^sub>c \<langle>(left_cart_proj \<nat>\<^sub>c \<nat>\<^sub>c) \<circ>\<^sub>c (left_cart_proj (\<nat>\<^sub>c\<times>\<^sub>c \<nat>\<^sub>c) \<nat>\<^sub>c),
+\<langle>(right_cart_proj \<nat>\<^sub>c \<nat>\<^sub>c) \<circ>\<^sub>c (left_cart_proj (\<nat>\<^sub>c\<times>\<^sub>c \<nat>\<^sub>c) \<nat>\<^sub>c), (right_cart_proj (\<nat>\<^sub>c\<times>\<^sub>c \<nat>\<^sub>c) \<nat>\<^sub>c)\<rangle>\<rangle>)\<^sup>\<sharp>)
+, eval_func \<nat>\<^sub>c (\<nat>\<^sub>c\<times>\<^sub>c\<nat>\<^sub>c)
+\<circ>\<^sub>c ( id\<^sub>c (\<nat>\<^sub>c\<times>\<^sub>c\<nat>\<^sub>c) \<times>\<^sub>f  (mult_uncurried \<circ>\<^sub>c (id\<^sub>c \<nat>\<^sub>c  \<times>\<^sub>f mult_uncurried) \<circ>\<^sub>c \<langle>(left_cart_proj \<nat>\<^sub>c \<nat>\<^sub>c) \<circ>\<^sub>c (left_cart_proj (\<nat>\<^sub>c\<times>\<^sub>c \<nat>\<^sub>c) \<nat>\<^sub>c),
+\<langle>(right_cart_proj \<nat>\<^sub>c \<nat>\<^sub>c) \<circ>\<^sub>c (left_cart_proj (\<nat>\<^sub>c\<times>\<^sub>c \<nat>\<^sub>c) \<nat>\<^sub>c), (right_cart_proj (\<nat>\<^sub>c\<times>\<^sub>c \<nat>\<^sub>c) \<nat>\<^sub>c)\<rangle>\<rangle>)\<^sup>\<sharp>)\<rangle>
+)\<circ>\<^sub>c \<langle>\<langle>a,b\<rangle>,c\<rangle>"
+      apply (subst cfunc_prod_comp[where X ="(\<nat>\<^sub>c\<times>\<^sub>c \<nat>\<^sub>c)\<times>\<^sub>c \<nat>\<^sub>c",
+          where Y = "(\<nat>\<^sub>c\<times>\<^sub>c \<nat>\<^sub>c)\<times>\<^sub>c(\<nat>\<^sub>c\<^bsup>(\<nat>\<^sub>c\<times>\<^sub>c\<nat>\<^sub>c)\<^esup>)", where A= "\<nat>\<^sub>c", where B="\<nat>\<^sub>c"])
+      apply (simp add: cfunc_cross_prod_type id_type multIdxMultp0p0p1p0p1_Sharp_type)
+      using multsigma0_type apply blast
+      using eval_func_type apply force
+      by (simp add: comp_associative)
+    also have "... = (add_uncurried \<circ>\<^sub>c \<langle>mult_uncurried \<circ>\<^sub>c (left_cart_proj (\<nat>\<^sub>c\<times>\<^sub>c\<nat>\<^sub>c) (\<nat>\<^sub>c\<^bsup>(\<nat>\<^sub>c\<times>\<^sub>c\<nat>\<^sub>c)\<^esup>))
+\<circ>\<^sub>c ( id\<^sub>c (\<nat>\<^sub>c\<times>\<^sub>c\<nat>\<^sub>c) \<times>\<^sub>f  (mult_uncurried \<circ>\<^sub>c (id\<^sub>c \<nat>\<^sub>c  \<times>\<^sub>f mult_uncurried) \<circ>\<^sub>c \<langle>(left_cart_proj \<nat>\<^sub>c \<nat>\<^sub>c) \<circ>\<^sub>c (left_cart_proj (\<nat>\<^sub>c\<times>\<^sub>c \<nat>\<^sub>c) \<nat>\<^sub>c),
+\<langle>(right_cart_proj \<nat>\<^sub>c \<nat>\<^sub>c) \<circ>\<^sub>c (left_cart_proj (\<nat>\<^sub>c\<times>\<^sub>c \<nat>\<^sub>c) \<nat>\<^sub>c), (right_cart_proj (\<nat>\<^sub>c\<times>\<^sub>c \<nat>\<^sub>c) \<nat>\<^sub>c)\<rangle>\<rangle>)\<^sup>\<sharp>)
+, 
+  mult_uncurried \<circ>\<^sub>c (id\<^sub>c \<nat>\<^sub>c  \<times>\<^sub>f mult_uncurried) \<circ>\<^sub>c \<langle>(left_cart_proj \<nat>\<^sub>c \<nat>\<^sub>c) \<circ>\<^sub>c (left_cart_proj (\<nat>\<^sub>c\<times>\<^sub>c \<nat>\<^sub>c) \<nat>\<^sub>c),
+\<langle>(right_cart_proj \<nat>\<^sub>c \<nat>\<^sub>c) \<circ>\<^sub>c (left_cart_proj (\<nat>\<^sub>c\<times>\<^sub>c \<nat>\<^sub>c) \<nat>\<^sub>c), (right_cart_proj (\<nat>\<^sub>c\<times>\<^sub>c \<nat>\<^sub>c) \<nat>\<^sub>c)\<rangle>\<rangle>\<rangle>
+)\<circ>\<^sub>c \<langle>\<langle>a,b\<rangle>,c\<rangle>"
+      using multIdxMultp0p0p1p0p1_type transpose_func_def by auto
+    also have "... = 
+(add_uncurried \<circ>\<^sub>c \<langle>mult_uncurried \<circ>\<^sub>c (id\<^sub>c (\<nat>\<^sub>c\<times>\<^sub>c\<nat>\<^sub>c) \<circ>\<^sub>c left_cart_proj (\<nat>\<^sub>c\<times>\<^sub>c\<nat>\<^sub>c) \<nat>\<^sub>c)  
+, 
+  mult_uncurried \<circ>\<^sub>c (id\<^sub>c \<nat>\<^sub>c  \<times>\<^sub>f mult_uncurried) \<circ>\<^sub>c \<langle>(left_cart_proj \<nat>\<^sub>c \<nat>\<^sub>c) \<circ>\<^sub>c (left_cart_proj (\<nat>\<^sub>c\<times>\<^sub>c \<nat>\<^sub>c) \<nat>\<^sub>c),
+\<langle>(right_cart_proj \<nat>\<^sub>c \<nat>\<^sub>c) \<circ>\<^sub>c (left_cart_proj (\<nat>\<^sub>c\<times>\<^sub>c \<nat>\<^sub>c) \<nat>\<^sub>c), (right_cart_proj (\<nat>\<^sub>c\<times>\<^sub>c \<nat>\<^sub>c) \<nat>\<^sub>c)\<rangle>\<rangle>\<rangle>
+)\<circ>\<^sub>c \<langle>\<langle>a,b\<rangle>,c\<rangle>"
+      by (smt id_type left_cart_proj_cfunc_cross_prod multIdxMultp0p0p1p0p1_Sharp_type)
+    also have "... = 
+     (add_uncurried \<circ>\<^sub>c \<langle>mult_uncurried \<circ>\<^sub>c (id\<^sub>c (\<nat>\<^sub>c\<times>\<^sub>c\<nat>\<^sub>c) \<circ>\<^sub>c left_cart_proj (\<nat>\<^sub>c\<times>\<^sub>c\<nat>\<^sub>c) \<nat>\<^sub>c)  
+, 
+  mult_uncurried  \<circ>\<^sub>c
+ \<langle>id\<^sub>c \<nat>\<^sub>c \<circ>\<^sub>c  (left_cart_proj \<nat>\<^sub>c \<nat>\<^sub>c) \<circ>\<^sub>c (left_cart_proj (\<nat>\<^sub>c\<times>\<^sub>c \<nat>\<^sub>c) \<nat>\<^sub>c),
+mult_uncurried \<circ>\<^sub>c \<langle>(right_cart_proj \<nat>\<^sub>c \<nat>\<^sub>c) \<circ>\<^sub>c (left_cart_proj (\<nat>\<^sub>c\<times>\<^sub>c \<nat>\<^sub>c) \<nat>\<^sub>c), (right_cart_proj (\<nat>\<^sub>c\<times>\<^sub>c \<nat>\<^sub>c) \<nat>\<^sub>c)\<rangle>
+\<rangle>
+\<rangle>
+)\<circ>\<^sub>c \<langle>\<langle>a,b\<rangle>,c\<rangle>"
+      using cfunc_cross_prod_comp_cfunc_prod id_type mult_uncurried_type p0rho0_type p1rho0rho1_type by fastforce
+    also have "... = add_uncurried \<circ>\<^sub>c 
+\<langle>mult_uncurried \<circ>\<^sub>c (left_cart_proj (\<nat>\<^sub>c\<times>\<^sub>c\<nat>\<^sub>c) \<nat>\<^sub>c)  
+, 
+  mult_uncurried  \<circ>\<^sub>c \<langle>(left_cart_proj \<nat>\<^sub>c \<nat>\<^sub>c) \<circ>\<^sub>c (left_cart_proj (\<nat>\<^sub>c\<times>\<^sub>c \<nat>\<^sub>c) \<nat>\<^sub>c),
+mult_uncurried \<circ>\<^sub>c \<langle>(right_cart_proj \<nat>\<^sub>c \<nat>\<^sub>c) \<circ>\<^sub>c (left_cart_proj (\<nat>\<^sub>c\<times>\<^sub>c \<nat>\<^sub>c) \<nat>\<^sub>c), (right_cart_proj (\<nat>\<^sub>c\<times>\<^sub>c \<nat>\<^sub>c) \<nat>\<^sub>c)\<rangle>
+\<rangle>
+\<rangle>
+\<circ>\<^sub>c \<langle>\<langle>a,b\<rangle>,c\<rangle>"
+      by (smt comp_associative id_left_unit2 id_right_unit2 mult_uncurried_type p0rho0_type)
+    also have "... = add_uncurried \<circ>\<^sub>c 
+\<langle>mult_uncurried \<circ>\<^sub>c (left_cart_proj (\<nat>\<^sub>c\<times>\<^sub>c\<nat>\<^sub>c) \<nat>\<^sub>c)  
+\<circ>\<^sub>c \<langle>\<langle>a,b\<rangle>,c\<rangle>
+,
+  mult_uncurried  \<circ>\<^sub>c \<langle>(left_cart_proj \<nat>\<^sub>c \<nat>\<^sub>c) \<circ>\<^sub>c (left_cart_proj (\<nat>\<^sub>c\<times>\<^sub>c \<nat>\<^sub>c) \<nat>\<^sub>c),
+mult_uncurried \<circ>\<^sub>c \<langle>(right_cart_proj \<nat>\<^sub>c \<nat>\<^sub>c) \<circ>\<^sub>c (left_cart_proj (\<nat>\<^sub>c\<times>\<^sub>c \<nat>\<^sub>c) \<nat>\<^sub>c), (right_cart_proj (\<nat>\<^sub>c\<times>\<^sub>c \<nat>\<^sub>c) \<nat>\<^sub>c)\<rangle>
+\<rangle>
+\<circ>\<^sub>c \<langle>\<langle>a,b\<rangle>,c\<rangle> \<rangle>"
+      apply (subst cfunc_prod_comp[where X = "one", where Y = "(\<nat>\<^sub>c\<times>\<^sub>c \<nat>\<^sub>c)\<times>\<^sub>c\<nat>\<^sub>c",
+            where A = "\<nat>\<^sub>c", where B= "\<nat>\<^sub>c"])
+      using abc_type apply blast
+      using comp_type left_cart_proj_type mult_uncurried_type apply blast
+      apply (smt cfunc_cross_prod_comp_cfunc_prod id_left_unit2 id_type multIdxMultp0p0p1p0p1_type mult_uncurried_type p0rho0_type p1rho0rho1_type)
+      by (simp add: comp_associative)
+    also have "... =add_uncurried \<circ>\<^sub>c 
+\<langle>mult_uncurried \<circ>\<^sub>c (left_cart_proj (\<nat>\<^sub>c\<times>\<^sub>c\<nat>\<^sub>c) \<nat>\<^sub>c)  
+\<circ>\<^sub>c \<langle>\<langle>a,b\<rangle>,c\<rangle>
+,
+  mult_uncurried  \<circ>\<^sub>c \<langle>(left_cart_proj \<nat>\<^sub>c \<nat>\<^sub>c) \<circ>\<^sub>c (left_cart_proj (\<nat>\<^sub>c\<times>\<^sub>c \<nat>\<^sub>c) \<nat>\<^sub>c) \<circ>\<^sub>c \<langle>\<langle>a,b\<rangle>,c\<rangle>
+,
+mult_uncurried \<circ>\<^sub>c \<langle>(right_cart_proj \<nat>\<^sub>c \<nat>\<^sub>c) \<circ>\<^sub>c (left_cart_proj (\<nat>\<^sub>c\<times>\<^sub>c \<nat>\<^sub>c) \<nat>\<^sub>c), (right_cart_proj (\<nat>\<^sub>c\<times>\<^sub>c \<nat>\<^sub>c) \<nat>\<^sub>c)\<rangle>
+\<circ>\<^sub>c \<langle>\<langle>a,b\<rangle>,c\<rangle>
+\<rangle>
+ \<rangle>"
+      apply (subst cfunc_prod_comp [where X = "one", where Y = "(\<nat>\<^sub>c\<times>\<^sub>c \<nat>\<^sub>c)\<times>\<^sub>c\<nat>\<^sub>c",
+            where  A = "\<nat>\<^sub>c", where B = "\<nat>\<^sub>c"])
+      using abc_type apply blast
+      using p0rho0_type apply fastforce
+      using comp_type mult_uncurried_type p1rho0rho1_type apply blast
+      by (simp add: comp_associative)
+    also have "... = add_uncurried \<circ>\<^sub>c 
+\<langle>mult_uncurried \<circ>\<^sub>c (left_cart_proj (\<nat>\<^sub>c\<times>\<^sub>c\<nat>\<^sub>c) \<nat>\<^sub>c)  
+\<circ>\<^sub>c \<langle>\<langle>a,b\<rangle>,c\<rangle>
+,
+  mult_uncurried  \<circ>\<^sub>c \<langle>(left_cart_proj \<nat>\<^sub>c \<nat>\<^sub>c) \<circ>\<^sub>c (left_cart_proj (\<nat>\<^sub>c\<times>\<^sub>c \<nat>\<^sub>c) \<nat>\<^sub>c) \<circ>\<^sub>c \<langle>\<langle>a,b\<rangle>,c\<rangle>
+,
+mult_uncurried \<circ>\<^sub>c \<langle>(right_cart_proj \<nat>\<^sub>c \<nat>\<^sub>c) \<circ>\<^sub>c (left_cart_proj (\<nat>\<^sub>c\<times>\<^sub>c \<nat>\<^sub>c) \<nat>\<^sub>c) \<circ>\<^sub>c \<langle>\<langle>a,b\<rangle>,c\<rangle>
+, (right_cart_proj (\<nat>\<^sub>c\<times>\<^sub>c \<nat>\<^sub>c) \<nat>\<^sub>c) \<circ>\<^sub>c \<langle>\<langle>a,b\<rangle>,c\<rangle>  \<rangle>
+\<rangle>
+ \<rangle>"
+      by (smt abc_type cfunc_prod_comp comp_associative p1rho0_type right_cart_proj_type)
+    also have "... = add_uncurried \<circ>\<^sub>c 
+\<langle>mult_uncurried \<circ>\<^sub>c 
+ \<langle>a,b\<rangle>
+,
+  mult_uncurried  \<circ>\<^sub>c \<langle>(left_cart_proj \<nat>\<^sub>c \<nat>\<^sub>c) \<circ>\<^sub>c \<langle>a,b\<rangle>
+,
+mult_uncurried \<circ>\<^sub>c \<langle>(right_cart_proj \<nat>\<^sub>c \<nat>\<^sub>c) \<circ>\<^sub>c  \<langle>a,b\<rangle>
+, (right_cart_proj (\<nat>\<^sub>c\<times>\<^sub>c \<nat>\<^sub>c) \<nat>\<^sub>c) \<circ>\<^sub>c \<langle>\<langle>a,b\<rangle>,c\<rangle>  \<rangle>
+\<rangle>
+ \<rangle>"
+      using ab_type assms(3) left_cart_proj_cfunc_prod by auto
+    also have "... = add_uncurried \<circ>\<^sub>c 
+\<langle>mult_uncurried \<circ>\<^sub>c \<langle>a,b\<rangle> ,mult_uncurried  \<circ>\<^sub>c \<langle>a, mult_uncurried \<circ>\<^sub>c \<langle>b, c \<rangle>\<rangle>\<rangle>"
+      using ab_type assms left_cart_proj_cfunc_prod right_cart_proj_cfunc_prod by auto
+    also have "... =  (a \<cdot>\<^sub>\<nat> b) +\<^sub>\<nat> a \<cdot>\<^sub>\<nat> (b \<cdot>\<^sub>\<nat> c)"
+      by (simp add: add_def mult_def)
+    also have "... = a \<cdot>\<^sub>\<nat> b  +\<^sub>\<nat> (b \<cdot>\<^sub>\<nat> c) \<cdot>\<^sub>\<nat> a"
+      oops
+*)
+
+  oops
+
+*)
+
+
+(* Don't forget to do Right Distributivity *)
+
+
+lemma mult_right_distributivity:
+  assumes "a \<in>\<^sub>c  \<nat>\<^sub>c"  "b\<in>\<^sub>c  \<nat>\<^sub>c"  "c\<in>\<^sub>c  \<nat>\<^sub>c"
+  shows "a \<cdot>\<^sub>\<nat> ( b +\<^sub>\<nat> c)   = (a \<cdot>\<^sub>\<nat> b) +\<^sub>\<nat>  (a \<cdot>\<^sub>\<nat> c)"
+  oops
+
+
+
+(*Defining exponentiation on N*)
+
+definition exp_curried :: "cfunc" where
+   "exp_curried = (THE w. w: \<nat>\<^sub>c \<rightarrow>  \<nat>\<^sub>c\<^bsup>\<nat>\<^sub>c\<^esup> \<and>
+   triangle_commutes one \<nat>\<^sub>c  (\<nat>\<^sub>c\<^bsup>\<nat>\<^sub>c\<^esup>) zero w ((successor \<circ>\<^sub>c zero \<circ>\<^sub>c right_cart_proj \<nat>\<^sub>c one)\<^sup>\<sharp>) \<and>
+   square_commutes \<nat>\<^sub>c  (\<nat>\<^sub>c\<^bsup>\<nat>\<^sub>c\<^esup>) \<nat>\<^sub>c (\<nat>\<^sub>c\<^bsup>\<nat>\<^sub>c\<^esup>) w ((mult_uncurried \<circ>\<^sub>c\<langle>left_cart_proj \<nat>\<^sub>c (\<nat>\<^sub>c\<^bsup>\<nat>\<^sub>c\<^esup>),eval_func \<nat>\<^sub>c \<nat>\<^sub>c\<rangle>)\<^sup>\<sharp>) successor w)"
+
+lemma exp_curried_property: "(exp_curried: \<nat>\<^sub>c \<rightarrow>  \<nat>\<^sub>c\<^bsup>\<nat>\<^sub>c\<^esup> \<and>
+   triangle_commutes one \<nat>\<^sub>c  (\<nat>\<^sub>c\<^bsup>\<nat>\<^sub>c\<^esup>) zero exp_curried ((successor \<circ>\<^sub>c zero \<circ>\<^sub>c right_cart_proj \<nat>\<^sub>c one)\<^sup>\<sharp>) \<and>
+   square_commutes \<nat>\<^sub>c  (\<nat>\<^sub>c\<^bsup>\<nat>\<^sub>c\<^esup>) \<nat>\<^sub>c (\<nat>\<^sub>c\<^bsup>\<nat>\<^sub>c\<^esup>) exp_curried ((mult_uncurried \<circ>\<^sub>c\<langle>left_cart_proj \<nat>\<^sub>c (\<nat>\<^sub>c\<^bsup>\<nat>\<^sub>c\<^esup>),eval_func \<nat>\<^sub>c \<nat>\<^sub>c\<rangle>)\<^sup>\<sharp>) successor exp_curried)"
+  unfolding exp_curried_def
+proof (rule theI')
+  have q_type: "((successor \<circ>\<^sub>c zero \<circ>\<^sub>c right_cart_proj \<nat>\<^sub>c one)\<^sup>\<sharp>) :  one \<rightarrow>  \<nat>\<^sub>c\<^bsup>\<nat>\<^sub>c\<^esup>"
+    by (meson comp_type right_cart_proj_type successor_type transpose_func_def zero_type)
+  have f_type: "((mult_uncurried \<circ>\<^sub>c\<langle>left_cart_proj \<nat>\<^sub>c (\<nat>\<^sub>c\<^bsup>\<nat>\<^sub>c\<^esup>),eval_func \<nat>\<^sub>c \<nat>\<^sub>c\<rangle>)\<^sup>\<sharp>) : (\<nat>\<^sub>c\<^bsup>\<nat>\<^sub>c\<^esup>) \<rightarrow> (\<nat>\<^sub>c\<^bsup>\<nat>\<^sub>c\<^esup>)"
+    using add_uncurried_type cfunc_type_def codomain_comp compatible_comp_ETCS_func domain_comp f_mult_flat_type mult_uncurried_type transpose_func_def by auto
+  show "\<exists>!x. x : \<nat>\<^sub>c \<rightarrow> \<nat>\<^sub>c\<^bsup>\<nat>\<^sub>c\<^esup> \<and>
+         triangle_commutes one \<nat>\<^sub>c (\<nat>\<^sub>c\<^bsup>\<nat>\<^sub>c\<^esup>) zero x
+          ((successor \<circ>\<^sub>c zero \<circ>\<^sub>c right_cart_proj \<nat>\<^sub>c one)\<^sup>\<sharp>) \<and>
+         square_commutes \<nat>\<^sub>c (\<nat>\<^sub>c\<^bsup>\<nat>\<^sub>c\<^esup>) \<nat>\<^sub>c (\<nat>\<^sub>c\<^bsup>\<nat>\<^sub>c\<^esup>) x
+          ((mult_uncurried \<circ>\<^sub>c \<langle>left_cart_proj \<nat>\<^sub>c (\<nat>\<^sub>c\<^bsup>\<nat>\<^sub>c\<^esup>),eval_func \<nat>\<^sub>c \<nat>\<^sub>c\<rangle>)\<^sup>\<sharp>)
+          successor x"
+    by (simp add: f_type natural_number_object_property q_type)
+qed
+
+lemma exp_curried_type: "exp_curried:  \<nat>\<^sub>c \<rightarrow>  \<nat>\<^sub>c\<^bsup>\<nat>\<^sub>c\<^esup>"
+  by (simp add: exp_curried_property)
+ 
+lemma exp_curried_0_eq: "exp_curried \<circ>\<^sub>c zero = ((successor \<circ>\<^sub>c zero \<circ>\<^sub>c right_cart_proj \<nat>\<^sub>c one)\<^sup>\<sharp>)"
+  using exp_curried_property triangle_commutes_def by blast
+
+lemma exp_curried_comp_succ_eq: "exp_curried \<circ>\<^sub>c successor = ((mult_uncurried \<circ>\<^sub>c\<langle>left_cart_proj \<nat>\<^sub>c (\<nat>\<^sub>c\<^bsup>\<nat>\<^sub>c\<^esup>),eval_func \<nat>\<^sub>c \<nat>\<^sub>c\<rangle>)\<^sup>\<sharp>) \<circ>\<^sub>c exp_curried"
+  using exp_curried_property square_commutes_def by auto
+
+definition exp_uncurried :: "cfunc"
+  where "exp_uncurried = eval_func  \<nat>\<^sub>c \<nat>\<^sub>c \<circ>\<^sub>c (id \<nat>\<^sub>c \<times>\<^sub>f exp_curried)"
+
+lemma exp_uncurried_type: "exp_uncurried:  \<nat>\<^sub>c\<times>\<^sub>c\<nat>\<^sub>c \<rightarrow>  \<nat>\<^sub>c"
+  unfolding exp_uncurried_def
+proof - 
+  have "id \<nat>\<^sub>c \<times>\<^sub>f exp_curried : \<nat>\<^sub>c\<times>\<^sub>c\<nat>\<^sub>c \<rightarrow>  \<nat>\<^sub>c\<times>\<^sub>c(\<nat>\<^sub>c\<^bsup>\<nat>\<^sub>c\<^esup>)"
+    by (simp add: exp_curried_property cfunc_cross_prod_type id_type)
+  then show "eval_func \<nat>\<^sub>c \<nat>\<^sub>c \<circ>\<^sub>c id\<^sub>c \<nat>\<^sub>c \<times>\<^sub>f exp_curried : \<nat>\<^sub>c \<times>\<^sub>c \<nat>\<^sub>c \<rightarrow> \<nat>\<^sub>c"
+    using comp_type eval_func_type by blast
+qed
+
+lemma exp_uncurried_apply:
+  assumes "m : X \<rightarrow> \<nat>\<^sub>c" "n : X \<rightarrow> \<nat>\<^sub>c"
+  shows "exp_uncurried \<circ>\<^sub>c \<langle>m, n\<rangle> = eval_func  \<nat>\<^sub>c \<nat>\<^sub>c \<circ>\<^sub>c \<langle>m, exp_curried \<circ>\<^sub>c n\<rangle>"
+  by (smt exp_curried_property exp_uncurried_def assms cfunc_cross_prod_comp_cfunc_prod comp_associative id_left_unit2 id_type)
+
+
+definition exp :: "cfunc \<Rightarrow> cfunc \<Rightarrow> cfunc" (infixl "^\<^sub>\<nat>" 75)
+  where "m ^\<^sub>\<nat> n = exp_uncurried\<circ>\<^sub>c\<langle>m, n\<rangle>"
+
+lemma exp_def2:
+  assumes "m\<in>\<^sub>c  \<nat>\<^sub>c" "n\<in>\<^sub>c  \<nat>\<^sub>c"
+  shows "m ^\<^sub>\<nat> n = eval_func  \<nat>\<^sub>c \<nat>\<^sub>c \<circ>\<^sub>c \<langle>m, exp_curried \<circ>\<^sub>c n\<rangle>"
+  unfolding exp_def exp_uncurried_def
+  by (smt exp_curried_type assms cfunc_cross_prod_comp_cfunc_prod cfunc_type_def comp_associative id_left_unit id_type)
+
+
+
+lemma exp_apply1:
+  assumes "m \<in>\<^sub>c \<nat>\<^sub>c" "n\<in>\<^sub>c \<nat>\<^sub>c"
+  shows "m ^\<^sub>\<nat> n = exp_uncurried \<circ>\<^sub>c \<langle>m \<circ>\<^sub>c \<beta>\<^bsub>\<nat>\<^sub>c\<^esub>, id \<nat>\<^sub>c\<rangle>\<circ>\<^sub>c n"
+  unfolding add_def 
+proof - 
+  have fact1: "m \<circ>\<^sub>c \<beta>\<^bsub>\<nat>\<^sub>c\<^esub>:\<nat>\<^sub>c \<rightarrow> \<nat>\<^sub>c"
+    using assms(1) comp_type terminal_func_type by blast
+  have "exp_uncurried \<circ>\<^sub>c \<langle>m,n\<rangle> = exp_uncurried \<circ>\<^sub>c \<langle>m \<circ>\<^sub>c id one  ,id \<nat>\<^sub>c \<circ>\<^sub>c n\<rangle>"
+    by (metis assms cfunc_type_def id_left_unit id_right_unit)
+  also have "... = exp_uncurried \<circ>\<^sub>c \<langle>m \<circ>\<^sub>c (\<beta>\<^bsub>\<nat>\<^sub>c\<^esub> \<circ>\<^sub>c n)  ,id \<nat>\<^sub>c \<circ>\<^sub>c n\<rangle>"
+    by (metis assms(2) comp_type id_type one_unique_element terminal_func_type)
+  also have "... = exp_uncurried \<circ>\<^sub>c \<langle>(m \<circ>\<^sub>c \<beta>\<^bsub>\<nat>\<^sub>c\<^esub>) \<circ>\<^sub>c n  ,id \<nat>\<^sub>c \<circ>\<^sub>c n\<rangle>"
+    using comp_associative by auto
+  also have "... = exp_uncurried \<circ>\<^sub>c \<langle>m \<circ>\<^sub>c \<beta>\<^bsub>\<nat>\<^sub>c\<^esub>, id \<nat>\<^sub>c\<rangle>\<circ>\<^sub>c n"
+    using assms(2) cfunc_prod_comp fact1 id_type by fastforce
+  then show ?thesis
+    by (simp add: calculation exp_def)
+qed
+
+
+
+lemma exp_apply1_left:
+  assumes "m \<in>\<^sub>c \<nat>\<^sub>c" "n\<in>\<^sub>c \<nat>\<^sub>c"
+  shows "m ^\<^sub>\<nat> n = exp_uncurried \<circ>\<^sub>c \<langle>id \<nat>\<^sub>c, n \<circ>\<^sub>c \<beta>\<^bsub>\<nat>\<^sub>c\<^esub>\<rangle>\<circ>\<^sub>c m"
+  unfolding add_def 
+proof - 
+  have fact1: "n \<circ>\<^sub>c \<beta>\<^bsub>\<nat>\<^sub>c\<^esub>:\<nat>\<^sub>c \<rightarrow> \<nat>\<^sub>c"
+    using assms(2) comp_type terminal_func_type by blast
+  have "exp_uncurried \<circ>\<^sub>c \<langle>m,n\<rangle> = exp_uncurried \<circ>\<^sub>c \<langle>id \<nat>\<^sub>c \<circ>\<^sub>c m, n \<circ>\<^sub>c id one\<rangle>"
+    by (metis assms cfunc_type_def id_left_unit id_right_unit)
+  also have "... = exp_uncurried \<circ>\<^sub>c \<langle>id \<nat>\<^sub>c \<circ>\<^sub>c m, n \<circ>\<^sub>c (\<beta>\<^bsub>\<nat>\<^sub>c\<^esub> \<circ>\<^sub>c m)\<rangle>"
+    by (metis assms(1) comp_type id_type one_unique_element terminal_func_type)
+  also have "... = exp_uncurried \<circ>\<^sub>c \<langle>id \<nat>\<^sub>c \<circ>\<^sub>c m, (n \<circ>\<^sub>c \<beta>\<^bsub>\<nat>\<^sub>c\<^esub>) \<circ>\<^sub>c m\<rangle>"
+    using comp_associative by auto
+  also have "... = exp_uncurried \<circ>\<^sub>c \<langle>id \<nat>\<^sub>c, n \<circ>\<^sub>c \<beta>\<^bsub>\<nat>\<^sub>c\<^esub> \<rangle> \<circ>\<^sub>c m"
+    using assms(1) cfunc_prod_comp fact1 id_type by fastforce
+  then show ?thesis
+    by (simp add: calculation exp_def)
+qed
+
+lemma s0proj_type: "successor \<circ>\<^sub>c zero \<circ>\<^sub>c (right_cart_proj \<nat>\<^sub>c one): \<nat>\<^sub>c \<times>\<^sub>c one \<rightarrow> \<nat>\<^sub>c"
+    using comp_type right_cart_proj_type successor_type zero_type by blast
+lemma s0projSharp_type: "(successor \<circ>\<^sub>c zero \<circ>\<^sub>c (right_cart_proj \<nat>\<^sub>c one))\<^sup>\<sharp>: one \<rightarrow> \<nat>\<^sub>c\<^bsup>\<nat>\<^sub>c\<^esup>"
+  by (simp add: s0proj_type transpose_func_def)
+
+
+lemma exp_respects_Zero_Left:
+  assumes "n \<in>\<^sub>c  \<nat>\<^sub>c"
+  shows "n ^\<^sub>\<nat> zero = successor \<circ>\<^sub>c zero"
+proof -
+  have "n ^\<^sub>\<nat> zero =  eval_func  \<nat>\<^sub>c \<nat>\<^sub>c \<circ>\<^sub>c \<langle>n, exp_curried \<circ>\<^sub>c zero\<rangle>"
+    by (simp add: assms exp_def2 zero_type)
+  also have "... = eval_func  \<nat>\<^sub>c \<nat>\<^sub>c \<circ>\<^sub>c  \<langle>n,((successor \<circ>\<^sub>c zero \<circ>\<^sub>c right_cart_proj \<nat>\<^sub>c one)\<^sup>\<sharp>)\<rangle>"
+    by (simp add: exp_curried_0_eq)
+  also have "... = eval_func  \<nat>\<^sub>c \<nat>\<^sub>c \<circ>\<^sub>c  \<langle>id\<^sub>c \<nat>\<^sub>c \<circ>\<^sub>c n,((successor \<circ>\<^sub>c zero \<circ>\<^sub>c right_cart_proj \<nat>\<^sub>c one)\<^sup>\<sharp>) \<circ>\<^sub>c id\<^sub>c one\<rangle>"
+    by (metis assms comp_associative exp_curried_0_eq id_left_unit2 id_right_unit2 zero_type)
+  also have "... =  eval_func  \<nat>\<^sub>c \<nat>\<^sub>c \<circ>\<^sub>c (id\<^sub>c \<nat>\<^sub>c \<times>\<^sub>f ((successor \<circ>\<^sub>c zero \<circ>\<^sub>c right_cart_proj \<nat>\<^sub>c one)\<^sup>\<sharp>)) \<circ>\<^sub>c \<langle>n,id\<^sub>c one\<rangle>" 
+    using assms exp_curried_property triangle_commutes_def id_type
+    by (smt cfunc_cross_prod_comp_cfunc_prod)
+  also have "... = successor \<circ>\<^sub>c zero \<circ>\<^sub>c right_cart_proj \<nat>\<^sub>c one \<circ>\<^sub>c \<langle>n,id\<^sub>c one\<rangle>"
+    using comp_associative s0proj_type transpose_func_def by auto
+  also have "... = successor \<circ>\<^sub>c zero \<circ>\<^sub>c id\<^sub>c one"
+    using assms id_type right_cart_proj_cfunc_prod by fastforce
+  also have "... =  successor \<circ>\<^sub>c zero"
+    using id_right_unit2 zero_type by auto
+  then show ?thesis
+    using calculation by auto
+qed
+
+(*Notice, in particular that 0^0 = 1*)
+
+
+lemma exp_respects_one_right:
+  assumes "n \<in>\<^sub>c  \<nat>\<^sub>c"
+  shows "n ^\<^sub>\<nat> (successor \<circ>\<^sub>c zero) = n" 
+proof -
+  have "n ^\<^sub>\<nat> (successor \<circ>\<^sub>c zero) =  eval_func  \<nat>\<^sub>c \<nat>\<^sub>c \<circ>\<^sub>c \<langle>n, exp_curried \<circ>\<^sub>c(successor \<circ>\<^sub>c zero) \<rangle>"
+    using assms comp_type exp_def2 successor_type zero_type by blast
+  also have "... = eval_func  \<nat>\<^sub>c \<nat>\<^sub>c \<circ>\<^sub>c \<langle>n, ((mult_uncurried \<circ>\<^sub>c\<langle>left_cart_proj \<nat>\<^sub>c (\<nat>\<^sub>c\<^bsup>\<nat>\<^sub>c\<^esup>),eval_func \<nat>\<^sub>c \<nat>\<^sub>c\<rangle>)\<^sup>\<sharp>) \<circ>\<^sub>cexp_curried \<circ>\<^sub>c zero \<rangle>"
+    using comp_associative exp_curried_comp_succ_eq by auto
+  also have "... = eval_func  \<nat>\<^sub>c \<nat>\<^sub>c \<circ>\<^sub>c \<langle>n, ((mult_uncurried \<circ>\<^sub>c\<langle>left_cart_proj \<nat>\<^sub>c (\<nat>\<^sub>c\<^bsup>\<nat>\<^sub>c\<^esup>),eval_func \<nat>\<^sub>c \<nat>\<^sub>c\<rangle>)\<^sup>\<sharp>) \<circ>\<^sub>c ((successor \<circ>\<^sub>c zero \<circ>\<^sub>c right_cart_proj \<nat>\<^sub>c one)\<^sup>\<sharp>)\<rangle>"
+    by (simp add: exp_curried_0_eq)
+  also have "... = eval_func  \<nat>\<^sub>c \<nat>\<^sub>c \<circ>\<^sub>c \<langle>id\<^sub>c \<nat>\<^sub>c \<circ>\<^sub>c n, ((mult_uncurried \<circ>\<^sub>c\<langle>left_cart_proj \<nat>\<^sub>c (\<nat>\<^sub>c\<^bsup>\<nat>\<^sub>c\<^esup>),eval_func \<nat>\<^sub>c \<nat>\<^sub>c\<rangle>)\<^sup>\<sharp>) \<circ>\<^sub>c ((successor \<circ>\<^sub>c zero \<circ>\<^sub>c right_cart_proj \<nat>\<^sub>c one)\<^sup>\<sharp>)\<rangle>"
+    using assms id_left_unit2 by auto
+  also have "... =  eval_func  \<nat>\<^sub>c \<nat>\<^sub>c \<circ>\<^sub>c (id\<^sub>c \<nat>\<^sub>c \<times>\<^sub>f ((mult_uncurried \<circ>\<^sub>c\<langle>left_cart_proj \<nat>\<^sub>c (\<nat>\<^sub>c\<^bsup>\<nat>\<^sub>c\<^esup>),eval_func \<nat>\<^sub>c \<nat>\<^sub>c\<rangle>)\<^sup>\<sharp>)) \<circ>\<^sub>c \<langle>n,((successor \<circ>\<^sub>c zero \<circ>\<^sub>c right_cart_proj \<nat>\<^sub>c one)\<^sup>\<sharp>)\<rangle>"
+    by (smt assms cfunc_cross_prod_comp_cfunc_prod exp_curried_property id_type square_commutes_def triangle_commutes_def)
+  also have "... = mult_uncurried \<circ>\<^sub>c\<langle>left_cart_proj \<nat>\<^sub>c (\<nat>\<^sub>c\<^bsup>\<nat>\<^sub>c\<^esup>),eval_func \<nat>\<^sub>c \<nat>\<^sub>c\<rangle> \<circ>\<^sub>c \<langle>n,((successor \<circ>\<^sub>c zero \<circ>\<^sub>c right_cart_proj \<nat>\<^sub>c one)\<^sup>\<sharp>)\<rangle>"
+    using add_uncurried_type cfunc_type_def codomain_comp comp_associative compatible_comp_ETCS_func domain_comp f_mult_flat_type mult_uncurried_type transpose_func_def by auto
+  also have "... = mult_uncurried \<circ>\<^sub>c
+\<langle>left_cart_proj \<nat>\<^sub>c (\<nat>\<^sub>c\<^bsup>\<nat>\<^sub>c\<^esup>)
+\<circ>\<^sub>c \<langle>n,((successor \<circ>\<^sub>c zero \<circ>\<^sub>c right_cart_proj \<nat>\<^sub>c one)\<^sup>\<sharp>)\<rangle>,
+eval_func \<nat>\<^sub>c \<nat>\<^sub>c 
+\<circ>\<^sub>c \<langle>n,((successor \<circ>\<^sub>c zero \<circ>\<^sub>c right_cart_proj \<nat>\<^sub>c one)\<^sup>\<sharp>)\<rangle> \<rangle> "
+    using assms cfunc_prod_type s0projSharp_type left_cart_proj_type eval_func_type
+    by (metis cfunc_prod_comp)
+  also have "... =  mult_uncurried \<circ>\<^sub>c
+\<langle>n ,eval_func \<nat>\<^sub>c \<nat>\<^sub>c \<circ>\<^sub>c \<langle>n,((successor \<circ>\<^sub>c zero \<circ>\<^sub>c right_cart_proj \<nat>\<^sub>c one)\<^sup>\<sharp>)\<rangle> \<rangle> "
+    using assms left_cart_proj_cfunc_prod s0projSharp_type by auto
+  also have "... = mult_uncurried \<circ>\<^sub>c
+\<langle>n ,eval_func \<nat>\<^sub>c \<nat>\<^sub>c \<circ>\<^sub>c \<langle>id\<^sub>c \<nat>\<^sub>c \<circ>\<^sub>c n,((successor \<circ>\<^sub>c zero \<circ>\<^sub>c right_cart_proj \<nat>\<^sub>c one)\<^sup>\<sharp>) \<circ>\<^sub>c id\<^sub>c one  \<rangle> \<rangle> "
+    using assms id_left_unit2 id_right_unit2 s0projSharp_type by auto
+  also have "... = mult_uncurried \<circ>\<^sub>c
+\<langle>n ,eval_func \<nat>\<^sub>c \<nat>\<^sub>c \<circ>\<^sub>c (id\<^sub>c \<nat>\<^sub>c \<times>\<^sub>f ((successor \<circ>\<^sub>c zero \<circ>\<^sub>c right_cart_proj \<nat>\<^sub>c one)\<^sup>\<sharp>))\<circ>\<^sub>c \<langle>n, id\<^sub>c one  \<rangle> \<rangle> "
+    by (smt assms cfunc_cross_prod_comp_cfunc_prod id_type s0projSharp_type)
+  also have "... = mult_uncurried \<circ>\<^sub>c \<langle>n ,successor \<circ>\<^sub>c zero \<circ>\<^sub>c right_cart_proj \<nat>\<^sub>c one \<circ>\<^sub>c \<langle>n, id\<^sub>c one  \<rangle>\<rangle>"
+    using comp_associative flat_cancels_sharp inv_transpose_func_def2 s0projSharp_type s0proj_type by fastforce
+  also have "... = mult_uncurried \<circ>\<^sub>c \<langle>n ,successor \<circ>\<^sub>c zero \<circ>\<^sub>c id\<^sub>c one \<rangle>"
+    by (metis (no_types) assms id_type right_cart_proj_cfunc_prod)
+  also have "... = n"
+    using assms id_right_unit2 mult_def s0_is_right_id zero_type by auto
+  then show ?thesis
+    using calculation by auto
+qed
+
+ lemma exp_respects_one_right:
+   assumes "n \<in>\<^sub>c  \<nat>\<^sub>c"
+   shows "zero ^\<^sub>\<nat> (successor \<circ>\<^sub>c n) = zero" 
+ proof - 
+   have zbz: "zero \<circ>\<^sub>c \<beta>\<^bsub>\<nat>\<^sub>c\<^esub> \<circ>\<^sub>c zero = zero"
+     using comp_associative successor_type terminal_func_comp zero_beta_succ_mEqs0 zero_type by auto
+   have Exp0betaSucc0Eqs0: "exp_uncurried \<circ>\<^sub>c \<langle>zero \<circ>\<^sub>c \<beta>\<^bsub>\<nat>\<^sub>c\<^esub>, successor\<rangle> \<circ>\<^sub>c zero = zero"
+     by (smt cfunc_prod_comp comp_associative exp_def exp_respects_one_right successor_type terminal_func_comp zbz zero_beta_N_succ_type zero_type)
+   have zbsn: "(zero \<circ>\<^sub>c \<beta>\<^bsub>\<nat>\<^sub>c\<^esub> \<circ>\<^sub>c successor)\<circ>\<^sub>c n  = zero"
+     by (metis assms comp_associative successor_type terminal_func_comp zbz zero_type)
+   have zbzbn: "(zero \<circ>\<^sub>c \<beta>\<^bsub>\<nat>\<^sub>c\<^esub>)\<circ>\<^sub>c(zero \<circ>\<^sub>c \<beta>\<^bsub>\<nat>\<^sub>c\<^esub>)\<circ>\<^sub>c n = zero"
+     using comp_associative successor_type terminal_func_comp zbsn zbz by auto
+
+   have square_el: "(exp_uncurried \<circ>\<^sub>c \<langle>zero \<circ>\<^sub>c \<beta>\<^bsub>\<nat>\<^sub>c\<^esub>, successor\<rangle> \<circ>\<^sub>c successor)\<circ>\<^sub>c n = zero \<circ>\<^sub>c \<beta>\<^bsub>\<nat>\<^sub>c\<^esub> \<circ>\<^sub>c exp_uncurried \<circ>\<^sub>c \<langle>zero \<circ>\<^sub>c \<beta>\<^bsub>\<nat>\<^sub>c\<^esub>,successor\<rangle>"
+   proof - 
+     have "(exp_uncurried \<circ>\<^sub>c \<langle>zero \<circ>\<^sub>c \<beta>\<^bsub>\<nat>\<^sub>c\<^esub>, successor\<rangle> \<circ>\<^sub>c successor)\<circ>\<^sub>c n = 
+     eval_func \<nat>\<^sub>c \<nat>\<^sub>c  \<circ>\<^sub>c \<langle>zero \<circ>\<^sub>c \<beta>\<^bsub>\<nat>\<^sub>c\<^esub>, exp_curried \<circ>\<^sub>c successor \<rangle> \<circ>\<^sub>c successor \<circ>\<^sub>c n"
+       using comp_associative exp_uncurried_apply successor_type terminal_func_comp zero_beta_N_succ_type by auto
+     also have "... =  eval_func \<nat>\<^sub>c \<nat>\<^sub>c  \<circ>\<^sub>c 
+\<langle>zero \<circ>\<^sub>c \<beta>\<^bsub>\<nat>\<^sub>c\<^esub>, ((mult_uncurried \<circ>\<^sub>c\<langle>left_cart_proj \<nat>\<^sub>c (\<nat>\<^sub>c\<^bsup>\<nat>\<^sub>c\<^esup>),eval_func \<nat>\<^sub>c \<nat>\<^sub>c\<rangle>)\<^sup>\<sharp>) \<circ>\<^sub>c exp_curried\<rangle> \<circ>\<^sub>c successor \<circ>\<^sub>c n"
+       using exp_curried_comp_succ_eq by auto
+     also have "... = eval_func \<nat>\<^sub>c \<nat>\<^sub>c  \<circ>\<^sub>c 
+\<langle>id\<^sub>c\<nat>\<^sub>c \<circ>\<^sub>c  zero \<circ>\<^sub>c \<beta>\<^bsub>\<nat>\<^sub>c\<^esub>, ((mult_uncurried \<circ>\<^sub>c\<langle>left_cart_proj \<nat>\<^sub>c (\<nat>\<^sub>c\<^bsup>\<nat>\<^sub>c\<^esup>),eval_func \<nat>\<^sub>c \<nat>\<^sub>c\<rangle>)\<^sup>\<sharp>) \<circ>\<^sub>c exp_curried\<rangle> \<circ>\<^sub>c successor \<circ>\<^sub>c n"
+       using id_left_unit2 successor_type terminal_func_comp zero_beta_N_succ_type by auto
+     also have "... =  eval_func \<nat>\<^sub>c \<nat>\<^sub>c  \<circ>\<^sub>c  (id\<^sub>c\<nat>\<^sub>c \<times>\<^sub>f ((mult_uncurried \<circ>\<^sub>c\<langle>left_cart_proj \<nat>\<^sub>c (\<nat>\<^sub>c\<^bsup>\<nat>\<^sub>c\<^esup>),eval_func \<nat>\<^sub>c \<nat>\<^sub>c\<rangle>)\<^sup>\<sharp>)) 
+\<circ>\<^sub>c \<langle>zero \<circ>\<^sub>c \<beta>\<^bsub>\<nat>\<^sub>c\<^esub>, exp_curried\<rangle> \<circ>\<^sub>c successor \<circ>\<^sub>c n"
+       by (smt cfunc_cross_prod_comp_cfunc_prod comp_associative exp_curried_property id_type square_commutes_def terminal_func_comp zero_beta_N_succ_type)
+     also have "... = (mult_uncurried \<circ>\<^sub>c\<langle>left_cart_proj \<nat>\<^sub>c (\<nat>\<^sub>c\<^bsup>\<nat>\<^sub>c\<^esup>),eval_func \<nat>\<^sub>c \<nat>\<^sub>c\<rangle> \<circ>\<^sub>c \<langle>zero \<circ>\<^sub>c \<beta>\<^bsub>\<nat>\<^sub>c\<^esub>, exp_curried\<rangle>) \<circ>\<^sub>c successor \<circ>\<^sub>c n"
+       using add_uncurried_type cfunc_type_def codomain_comp comp_associative compatible_comp_ETCS_func domain_comp f_mult_flat_type mult_uncurried_type transpose_func_def by auto
+     also have "... =  (mult_uncurried \<circ>\<^sub>c\<langle>left_cart_proj \<nat>\<^sub>c (\<nat>\<^sub>c\<^bsup>\<nat>\<^sub>c\<^esup>)\<circ>\<^sub>c \<langle>zero \<circ>\<^sub>c \<beta>\<^bsub>\<nat>\<^sub>c\<^esub>, exp_curried\<rangle> ,eval_func \<nat>\<^sub>c \<nat>\<^sub>c \<circ>\<^sub>c \<langle>zero \<circ>\<^sub>c \<beta>\<^bsub>\<nat>\<^sub>c\<^esub>, exp_curried\<rangle> \<rangle>) \<circ>\<^sub>c successor \<circ>\<^sub>c n"
+       apply(subst cfunc_prod_comp[where X = "\<nat>\<^sub>c", where Y = "\<nat>\<^sub>c \<times>\<^sub>c(\<nat>\<^sub>c\<^bsup>\<nat>\<^sub>c\<^esup>)", where A= "\<nat>\<^sub>c", where B="\<nat>\<^sub>c"])
+       apply (simp add: cfunc_prod_type exp_curried_property zero_betaN_type)
+       apply (simp add: left_cart_proj_type)
+       using eval_func_type apply blast
+       by simp
+     also have "... = (mult_uncurried \<circ>\<^sub>c\<langle>left_cart_proj \<nat>\<^sub>c (\<nat>\<^sub>c\<^bsup>\<nat>\<^sub>c\<^esup>)\<circ>\<^sub>c \<langle>zero \<circ>\<^sub>c \<beta>\<^bsub>\<nat>\<^sub>c\<^esub>, exp_curried\<rangle> ,eval_func \<nat>\<^sub>c \<nat>\<^sub>c \<circ>\<^sub>c \<langle>id\<^sub>c\<nat>\<^sub>c \<circ>\<^sub>c zero \<circ>\<^sub>c \<beta>\<^bsub>\<nat>\<^sub>c\<^esub>, exp_curried \<circ>\<^sub>c id\<^sub>c\<nat>\<^sub>c\<rangle> \<rangle>) \<circ>\<^sub>c successor \<circ>\<^sub>c n"
+       using exp_curried_type id_left_unit2 id_right_unit2 successor_type terminal_func_comp zero_beta_N_succ_type by auto
+     also have "... = (mult_uncurried \<circ>\<^sub>c\<langle>left_cart_proj \<nat>\<^sub>c (\<nat>\<^sub>c\<^bsup>\<nat>\<^sub>c\<^esup>)\<circ>\<^sub>c \<langle>zero \<circ>\<^sub>c \<beta>\<^bsub>\<nat>\<^sub>c\<^esub>, exp_curried\<rangle> ,eval_func \<nat>\<^sub>c \<nat>\<^sub>c \<circ>\<^sub>c (id\<^sub>c\<nat>\<^sub>c \<times>\<^sub>f exp_curried) \<circ>\<^sub>c  \<langle> zero \<circ>\<^sub>c \<beta>\<^bsub>\<nat>\<^sub>c\<^esub>,  id\<^sub>c\<nat>\<^sub>c\<rangle> \<rangle>) \<circ>\<^sub>c successor \<circ>\<^sub>c n"
+       by (smt cfunc_cross_prod_comp_cfunc_prod exp_curried_property id_type successor_type terminal_func_comp zero_beta_N_succ_type)
+     also have "... = (mult_uncurried \<circ>\<^sub>c\<langle>zero \<circ>\<^sub>c \<beta>\<^bsub>\<nat>\<^sub>c\<^esub>,eval_func \<nat>\<^sub>c \<nat>\<^sub>c \<circ>\<^sub>c (id\<^sub>c\<nat>\<^sub>c \<times>\<^sub>f exp_curried) \<circ>\<^sub>c  \<langle>zero \<circ>\<^sub>c \<beta>\<^bsub>\<nat>\<^sub>c\<^esub>,  id\<^sub>c\<nat>\<^sub>c\<rangle> \<rangle>) \<circ>\<^sub>c successor \<circ>\<^sub>c n"
+       by (metis (no_types) exp_curried_property left_cart_proj_cfunc_prod zero_betaN_type)
+     also have "... = (mult_uncurried \<circ>\<^sub>c\<langle>zero \<circ>\<^sub>c \<beta>\<^bsub>\<nat>\<^sub>c\<^esub>, exp_uncurried \<circ>\<^sub>c \<langle>zero \<circ>\<^sub>c \<beta>\<^bsub>\<nat>\<^sub>c\<^esub>,  id\<^sub>c\<nat>\<^sub>c\<rangle> \<rangle>)\<circ>\<^sub>c successor \<circ>\<^sub>c n"
+       by (simp add: comp_associative exp_uncurried_def)
+     also have "... = zero \<circ>\<^sub>c \<beta>\<^bsub>\<nat>\<^sub>c\<^esub> \<circ>\<^sub>c successor \<circ>\<^sub>c n"
+       oops
+
+(*
+lemma exp_respects_one_left:
+   assumes "n \<in>\<^sub>c  \<nat>\<^sub>c"
+   shows "(successor \<circ>\<^sub>c zero)^\<^sub>\<nat> n = (successor \<circ>\<^sub>c zero)" 
+proof - 
+  have s0b0Eqs0: "((successor \<circ>\<^sub>c zero)\<circ>\<^sub>c \<beta>\<^bsub>\<nat>\<^sub>c\<^esub>) \<circ>\<^sub>c zero = (successor \<circ>\<^sub>c zero)"
+    by (metis comp_associative successor_type terminal_func_comp zero_beta_succ_mEqs0 zero_type)
+  have ExpS0b1z: "(exp_uncurried \<circ>\<^sub>c \<langle>(successor \<circ>\<^sub>c zero)\<circ>\<^sub>c \<beta>\<^bsub>\<nat>\<^sub>c\<^esub>, id\<^sub>c\<nat>\<^sub>c\<rangle>) \<circ>\<^sub>c zero = (successor \<circ>\<^sub>c zero)"
+    by (metis (no_types, hide_lams) cfunc_type_def comp_associative compatible_comp_ETCS_func exp_apply1 exp_respects_Zero_Left s0b_type zero_type)
+  have szbs_n: "(((successor \<circ>\<^sub>c zero)\<circ>\<^sub>c \<beta>\<^bsub>\<nat>\<^sub>c\<^esub>) \<circ>\<^sub>c successor) \<circ>\<^sub>c  n = ((successor \<circ>\<^sub>c zero)\<circ>\<^sub>c \<beta>\<^bsub>\<nat>\<^sub>c\<^esub>) \<circ>\<^sub>c  n"
+    by (metis comp_associative successor_type terminal_func_comp)
+  have expSzbIdsnEqsIdExpS0bIdn: "(exp_uncurried \<circ>\<^sub>c \<langle>successor \<circ>\<^sub>c zero\<circ>\<^sub>c \<beta>\<^bsub>\<nat>\<^sub>c\<^esub>, id\<^sub>c\<nat>\<^sub>c\<rangle>) \<circ>\<^sub>c (successor \<circ>\<^sub>c n)
+                                   = (id\<^sub>c\<nat>\<^sub>c \<circ>\<^sub>c exp_uncurried \<circ>\<^sub>c \<langle>successor \<circ>\<^sub>c zero\<circ>\<^sub>c \<beta>\<^bsub>\<nat>\<^sub>c\<^esub>, id\<^sub>c\<nat>\<^sub>c\<rangle>)\<circ>\<^sub>c n"
+  (*
+  proof -
+
+    have s0_type: "successor \<circ>\<^sub>c zero : one \<rightarrow> \<nat>\<^sub>c"
+      using successor_type zero_type by auto
+    have sn_type: "successor \<circ>\<^sub>c n : one \<rightarrow> \<nat>\<^sub>c"
+      by (meson assms comp_type successor_type)
+    have "(exp_uncurried \<circ>\<^sub>c \<langle>successor \<circ>\<^sub>c zero\<circ>\<^sub>c \<beta>\<^bsub>\<nat>\<^sub>c\<^esub>, id\<^sub>c\<nat>\<^sub>c\<rangle>) \<circ>\<^sub>c (successor \<circ>\<^sub>c n) =exp_uncurried \<circ>\<^sub>c \<langle>successor \<circ>\<^sub>c zero\<circ>\<^sub>c \<beta>\<^bsub>\<nat>\<^sub>c\<^esub>, id\<^sub>c\<nat>\<^sub>c\<rangle> \<circ>\<^sub>c (successor \<circ>\<^sub>c n)"
+      by (simp add: comp_associative)
+    also have "... = exp_uncurried \<circ>\<^sub>c \<langle>successor \<circ>\<^sub>c zero\<circ>\<^sub>c \<beta>\<^bsub>\<nat>\<^sub>c\<^esub> \<circ>\<^sub>c (successor \<circ>\<^sub>c n),  successor \<circ>\<^sub>c n\<rangle>"
+      by (smt assms cfunc_prod_comp comp_associative id_left_unit2 id_type s0b_type successor_type terminal_func_comp)
+    also have "... =  exp_uncurried \<circ>\<^sub>c \<langle>successor \<circ>\<^sub>c zero, successor \<circ>\<^sub>c n\<rangle>"
+      using assms zero_beta_succ_mEqs0 by auto
+    also have "... = eval_func \<nat>\<^sub>c \<nat>\<^sub>c  \<circ>\<^sub>c (id\<^sub>c\<nat>\<^sub>c \<times>\<^sub>f exp_curried) \<circ>\<^sub>c \<langle>successor \<circ>\<^sub>c zero, successor \<circ>\<^sub>c n\<rangle>"
+      by (simp add: comp_associative exp_uncurried_def)
+    also have "... = eval_func \<nat>\<^sub>c \<nat>\<^sub>c  \<circ>\<^sub>c (id\<^sub>c\<nat>\<^sub>c \<times>\<^sub>f (id\<^sub>c(\<nat>\<^sub>c\<^bsup>\<nat>\<^sub>c\<^esup>) \<circ>\<^sub>c exp_curried)) \<circ>\<^sub>c \<langle>successor \<circ>\<^sub>c zero, successor \<circ>\<^sub>c n\<rangle>"
+      using exp_curried_property id_left_unit2 by auto
+    also have "... = eval_func \<nat>\<^sub>c \<nat>\<^sub>c  \<circ>\<^sub>c (id\<^sub>c\<nat>\<^sub>c \<times>\<^sub>f id\<^sub>c(\<nat>\<^sub>c\<^bsup>\<nat>\<^sub>c\<^esup>)) \<circ>\<^sub>c \<langle>successor \<circ>\<^sub>c zero, exp_curried \<circ>\<^sub>c successor \<circ>\<^sub>c n\<rangle>"
+      by (metis \<open>eval_func \<nat>\<^sub>c \<nat>\<^sub>c \<circ>\<^sub>c (id\<^sub>c \<nat>\<^sub>c \<times>\<^sub>f exp_curried) \<circ>\<^sub>c \<langle>successor \<circ>\<^sub>c zero,successor \<circ>\<^sub>c n\<rangle> = eval_func \<nat>\<^sub>c \<nat>\<^sub>c \<circ>\<^sub>c (id\<^sub>c \<nat>\<^sub>c \<times>\<^sub>f id\<^sub>c (\<nat>\<^sub>c\<^bsup>\<nat>\<^sub>c\<^esup>) \<circ>\<^sub>c exp_curried) \<circ>\<^sub>c \<langle>successor \<circ>\<^sub>c zero,successor \<circ>\<^sub>c n\<rangle>\<close> \<open>exp_uncurried \<circ>\<^sub>c \<langle>successor \<circ>\<^sub>c zero,successor \<circ>\<^sub>c n\<rangle> = eval_func \<nat>\<^sub>c \<nat>\<^sub>c \<circ>\<^sub>c (id\<^sub>c \<nat>\<^sub>c \<times>\<^sub>f exp_curried) \<circ>\<^sub>c \<langle>successor \<circ>\<^sub>c zero,successor \<circ>\<^sub>c n\<rangle>\<close> comp_associative eval_func_type exp_uncurried_apply id_cross_prod id_right_unit2 s0_type sn_type)
+    also have "... =  eval_func \<nat>\<^sub>c \<nat>\<^sub>c  \<circ>\<^sub>c (id\<^sub>c\<nat>\<^sub>c \<times>\<^sub>f id\<^sub>c(\<nat>\<^sub>c\<^bsup>\<nat>\<^sub>c\<^esup>)) \<circ>\<^sub>c \<langle>successor \<circ>\<^sub>c zero, ((mult_uncurried \<circ>\<^sub>c\<langle>left_cart_proj \<nat>\<^sub>c (\<nat>\<^sub>c\<^bsup>\<nat>\<^sub>c\<^esup>),eval_func \<nat>\<^sub>c \<nat>\<^sub>c\<rangle>)\<^sup>\<sharp>)     \<circ>\<^sub>c  exp_curried  \<circ>\<^sub>c n\<rangle>"
+      by (simp add: comp_associative exp_curried_comp_succ_eq)
+    also have "... =  eval_func \<nat>\<^sub>c \<nat>\<^sub>c  \<circ>\<^sub>c (id\<^sub>c\<nat>\<^sub>c \<times>\<^sub>f (id\<^sub>c(\<nat>\<^sub>c\<^bsup>\<nat>\<^sub>c\<^esup>) \<circ>\<^sub>c ((mult_uncurried \<circ>\<^sub>c\<langle>left_cart_proj \<nat>\<^sub>c (\<nat>\<^sub>c\<^bsup>\<nat>\<^sub>c\<^esup>),eval_func \<nat>\<^sub>c \<nat>\<^sub>c\<rangle>)\<^sup>\<sharp>) ) ) \<circ>\<^sub>c \<langle>successor \<circ>\<^sub>c zero,    exp_curried  \<circ>\<^sub>c n\<rangle>"
+      oops
+    *)
+*)
+
+lemma exp_respects_successor:
+   assumes "m \<in>\<^sub>c  \<nat>\<^sub>c" "n \<in>\<^sub>c  \<nat>\<^sub>c"
+   shows "m^\<^sub>\<nat>(successor \<circ>\<^sub>c n) = m \<cdot>\<^sub>\<nat> (m^\<^sub>\<nat> n) "
+proof - 
+  have "m^\<^sub>\<nat>(successor \<circ>\<^sub>c n) = exp_uncurried \<circ>\<^sub>c \<langle>m,successor \<circ>\<^sub>c n\<rangle>"
+    by (simp add: exp_def)
+  also have "... = eval_func \<nat>\<^sub>c \<nat>\<^sub>c  \<circ>\<^sub>c (id\<^sub>c \<nat>\<^sub>c \<times>\<^sub>f exp_curried) \<circ>\<^sub>c  \<langle>m,successor \<circ>\<^sub>c n\<rangle>"
+    by (simp add: comp_associative exp_uncurried_def)
+  also have "... = eval_func \<nat>\<^sub>c \<nat>\<^sub>c  \<circ>\<^sub>c (id\<^sub>c \<nat>\<^sub>c \<times>\<^sub>f exp_curried) \<circ>\<^sub>c  \<langle>id\<^sub>c \<nat>\<^sub>c \<circ>\<^sub>c m,successor \<circ>\<^sub>c n\<rangle>"
+    using assms(1) id_left_unit2 by auto
+  also have "... = eval_func \<nat>\<^sub>c \<nat>\<^sub>c  \<circ>\<^sub>c (id\<^sub>c \<nat>\<^sub>c \<circ>\<^sub>c id\<^sub>c \<nat>\<^sub>c \<times>\<^sub>f exp_curried \<circ>\<^sub>c successor) \<circ>\<^sub>c  \<langle>m, n\<rangle>"
+    apply (subst cfunc_cross_prod_comp_cfunc_prod[where A = one, where W ="\<nat>\<^sub>c", 
+          where X ="\<nat>\<^sub>c",  where Y ="\<nat>\<^sub>c", where Z = "\<nat>\<^sub>c\<^bsup>\<nat>\<^sub>c\<^esup>"])
+    using assms(1) id_left_unit2 apply auto[1]
+    using assms(2) comp_type successor_type apply blast
+    using id_type apply auto[1]
+    apply (simp add: exp_curried_type)
+    oops
 
 
 
